IOTickTock/IOTickTock_Deadline.thy
@@ -1,0 +1,1910 @@
+theory IOTickTock_Deadline
+  imports IOTickTock_Core "TickTock-FL.TickTock_Pri"
+begin
+
+section \<open>Preliminary Lemmas\<close>
+
+lemma filter_tocks_refusal_no_mid_event: "\<And>s. filter_tocks p @ [[Y]\<^sub>R] \<noteq> s @ [Event e]\<^sub>E # \<sigma>"
+  by (induct p rule:filter_tocks.induct, auto simp add: notin_tocks Cons_eq_append_conv)
+
+lemma RenamingTT_init_event:
+  "inj f \<Longrightarrow> {t. [Event (f e)]\<^sub>E # t \<in> RenamingTT P f} = RenamingTT {t. [Event e]\<^sub>E # t \<in> P} f"
+  unfolding RenamingTT_def inj_def by (auto, case_tac xa rule:ttWF.cases, auto, force)
+
+lemma RenamingTT_init_tock: "{\<sigma>. [X]\<^sub>R # [Tock]\<^sub>E # \<sigma> \<in> RenamingTT P f}
+          = RenamingTT {\<sigma>. [(lift_renaming_func f) -` X]\<^sub>R # [Tock]\<^sub>E # \<sigma> \<in> P} f"
+  unfolding RenamingTT_def by (auto, case_tac xa rule:ttWF.cases, auto, force)
+
+lemma lift_renaming_func_image_inverse:
+  "inj f \<Longrightarrow> lift_renaming_func f -` lift_renaming_func f ` X = X"
+  unfolding image_def vimage_def inj_def by (auto, case_tac x, auto, (case_tac xa, auto)+)
+
+lemma rename_trace_nonempty: "inj f \<Longrightarrow> \<exists>x. x \<in> rename_trace f t"
+  apply (induct f t rule:rename_trace.induct, auto)
+  by (rule_tac x="lift_renaming_func f ` X" in exI, auto simp add: lift_renaming_func_image_inverse)
+
+lemma RenamingTT_init_tock2:
+  "inj f \<Longrightarrow>
+    {\<sigma>. [(lift_renaming_func f) ` X]\<^sub>R # [Tock]\<^sub>E # \<sigma> \<in> RenamingTT P f} = RenamingTT {\<sigma>. [X]\<^sub>R # [Tock]\<^sub>E # \<sigma> \<in> P} f"
+  unfolding  RenamingTT_def using lift_renaming_func_image_inverse
+  by (auto, case_tac xa rule:ttWF.cases, auto, fastforce, rule_tac x="[X]\<^sub>R # [Tock]\<^sub>E # xa" in bexI, auto)
+
+lemma TimeSyncInterruptTT_PrefixTT_init_event: "e \<noteq> f \<Longrightarrow> {t. [Event e]\<^sub>E # t \<in> P \<triangle>\<^sub>T f \<rightarrow>\<^sub>C Q} = {t. [Event e]\<^sub>E # t \<in> P} \<triangle>\<^sub>T f \<rightarrow>\<^sub>C Q"
+  unfolding TimeSyncInterruptTT_def
+proof (safe, simp_all)
+  fix p x
+  show "p @ [[Tick]\<^sub>E] \<in> P \<Longrightarrow> filter_tocks p \<in> f \<rightarrow>\<^sub>C Q \<Longrightarrow> [Event e]\<^sub>E # x = p @ [[Tick]\<^sub>E] \<Longrightarrow>
+      \<exists>p. [Event e]\<^sub>E # p @ [[Tick]\<^sub>E] \<in> P \<and> filter_tocks p \<in> f \<rightarrow>\<^sub>C Q \<and> x = p @ [[Tick]\<^sub>E]"
+    by (case_tac p rule:ttWF.cases, simp_all)
+next
+  fix x p X Y Z
+  assume "p @ [[X]\<^sub>R] \<in> P" "filter_tocks p @ [[Y]\<^sub>R] \<in> f \<rightarrow>\<^sub>C Q" "Z \<subseteq> X \<union> Y" "{e \<in> X. e \<noteq> Tock} = {e \<in> Y. e \<noteq> Tock}" "[Event e]\<^sub>E # x = p @ [[Z]\<^sub>R]"
+  then show "\<forall>p X. [Event e]\<^sub>E # p @ [[X]\<^sub>R] \<in> P \<longrightarrow>
+             (\<forall>Y. {e \<in> X. e \<noteq> Tock} = {e \<in> Y. e \<noteq> Tock} \<longrightarrow> filter_tocks p @ [[Y]\<^sub>R] \<in> f \<rightarrow>\<^sub>C Q \<longrightarrow> (\<forall>Z\<subseteq>X \<union> Y. x \<noteq> p @ [[Z]\<^sub>R])) \<Longrightarrow>
+       [Event e]\<^sub>E # x = p @ [[Z]\<^sub>R] \<Longrightarrow> \<exists>p. [Event e]\<^sub>E # p @ [[Tick]\<^sub>E] \<in> P \<and> filter_tocks p \<in> f \<rightarrow>\<^sub>C Q \<and> x = p @ [[Tick]\<^sub>E]"
+    by (case_tac p rule:ttWF.cases, simp_all, blast)
+next
+  fix x p q2
+  assume p_in_P: "p \<in> P" and filter_tocks_p_q2_in_PrefixTT_Q: "filter_tocks p @ q2 \<in> f \<rightarrow>\<^sub>C Q"
+  assume p_no_end_tick: "\<forall>p'. p \<noteq> p' @ [[Tick]\<^sub>E]" and p_no_end_refusal: "\<forall>p' Y. p \<noteq> p' @ [[Y]\<^sub>R]"
+  assume q2_no_init_refusal: "\<forall>q' Y. q2 \<noteq> [Y]\<^sub>R # q'"
+  assume e_x_eq_p_q2: "[Event e]\<^sub>E # x = p @ q2"
+  assume e_neq_f: "e \<noteq> f"
+
+  have "(\<exists>p'. p = [Event e]\<^sub>E # p') \<or> p = []"
+    using e_x_eq_p_q2 by (case_tac p rule:ttWF.cases, simp_all)
+  then have "\<exists>p'. p = [Event e]\<^sub>E # p'"
+    using e_x_eq_p_q2 filter_tocks_p_q2_in_PrefixTT_Q unfolding PrefixTT_def apply (auto simp add: notin_tocks)
+    apply (metis (no_types, lifting) Cons_eq_append_conv list.inject start_event_notin_tocks ttobs.distinct(1))
+    by (metis (no_types, lifting) Cons_eq_append_conv e_neq_f list.inject start_event_notin_tocks ttevent.inject ttobs.inject(1))
+  then show "\<forall>p. [Event e]\<^sub>E # p \<in> P \<longrightarrow>
+           (\<exists>p'. p = p' @ [[Tick]\<^sub>E]) \<or>
+           (\<exists>p' Y. p = p' @ [[Y]\<^sub>R]) \<or> (\<forall>q2. filter_tocks p @ q2 \<in> f \<rightarrow>\<^sub>C Q \<longrightarrow> (\<exists>q' Y. q2 = [Y]\<^sub>R # q') \<or> x \<noteq> p @ q2) \<Longrightarrow>
+      \<exists>p. [Event e]\<^sub>E # p @ [[Tick]\<^sub>E] \<in> P \<and> filter_tocks p \<in> f \<rightarrow>\<^sub>C Q \<and> x = p @ [[Tick]\<^sub>E]"
+    by (metis append_Cons e_x_eq_p_q2 filter_tocks.simps(3) filter_tocks_p_q2_in_PrefixTT_Q
+        list.inject p_in_P p_no_end_refusal p_no_end_tick q2_no_init_refusal)
+next
+  fix p X Y Z
+  show " \<forall>pa X. pa @ [[X]\<^sub>R] \<in> P \<longrightarrow> (\<forall>Y. {e \<in> X. e \<noteq> Tock} = {e \<in> Y. e \<noteq> Tock} \<longrightarrow> Z \<subseteq> X \<union> Y \<longrightarrow> filter_tocks pa @ [[Y]\<^sub>R] \<in> f \<rightarrow>\<^sub>C Q \<longrightarrow> [Event e]\<^sub>E # p \<noteq> pa) \<Longrightarrow>
+       [Event e]\<^sub>E # p @ [[X]\<^sub>R] \<in> P \<Longrightarrow> filter_tocks p @ [[Y]\<^sub>R] \<in> f \<rightarrow>\<^sub>C Q \<Longrightarrow> Z \<subseteq> X \<union> Y \<Longrightarrow> {e \<in> X. e \<noteq> Tock} = {e \<in> Y. e \<noteq> Tock} \<Longrightarrow> False"
+    by (metis (no_types, lifting) append_Cons filter_tocks.simps(3))
+next
+  fix p q2
+  assume "[Event e]\<^sub>E # p \<in> P" "\<forall>p'. p \<noteq> p' @ [[Tick]\<^sub>E]" "\<forall>p' Y. p \<noteq> p' @ [[Y]\<^sub>R]" "filter_tocks p @ q2 \<in> f \<rightarrow>\<^sub>C Q" "\<forall>q' Y. q2 \<noteq> [Y]\<^sub>R # q'"
+  then show "\<forall>pa. pa \<in> P \<longrightarrow> (\<exists>p'. pa = p' @ [[Tick]\<^sub>E]) \<or> (\<exists>p' Y. pa = p' @ [[Y]\<^sub>R]) \<or>
+            (\<forall>q2a. filter_tocks pa @ q2a \<in> f \<rightarrow>\<^sub>C Q \<longrightarrow> (\<exists>q' Y. q2a = [Y]\<^sub>R # q') \<or> [Event e]\<^sub>E # p @ q2 \<noteq> pa @ q2a) \<Longrightarrow>
+        \<exists>pa. pa @ [[Tick]\<^sub>E] \<in> P \<and> filter_tocks pa \<in> f \<rightarrow>\<^sub>C Q \<and> [Event e]\<^sub>E # p @ q2 = pa @ [[Tick]\<^sub>E]"
+    by (erule_tac x="[Event e]\<^sub>E # p" in allE, auto simp add: Cons_eq_append_conv)
+qed
+
+lemma TimeSyncInterruptTT_PrefixTT_init_tock:
+  "\<forall>x\<in>P. ttWF x \<Longrightarrow> Event f \<notin> X \<Longrightarrow> {t. [X]\<^sub>R # [Tock]\<^sub>E # t \<in> P \<triangle>\<^sub>T f \<rightarrow>\<^sub>C Q} = {t. [X]\<^sub>R # [Tock]\<^sub>E # t \<in> P} \<triangle>\<^sub>T f \<rightarrow>\<^sub>C Q"
+  unfolding TimeSyncInterruptTT_def
+proof (safe, simp_all)
+  fix x p
+  show "p @ [[Tick]\<^sub>E] \<in> P \<Longrightarrow> filter_tocks p \<in> f \<rightarrow>\<^sub>C Q \<Longrightarrow> [X]\<^sub>R # [Tock]\<^sub>E # x = p @ [[Tick]\<^sub>E] \<Longrightarrow>
+      \<exists>p. [X]\<^sub>R # [Tock]\<^sub>E # p @ [[Tick]\<^sub>E] \<in> P \<and> filter_tocks p \<in> f \<rightarrow>\<^sub>C Q \<and> x = p @ [[Tick]\<^sub>E]"
+    unfolding PrefixTT_def apply (cases p rule:ttWF.cases, auto)
+    apply (meson list.inject list.simps(3) tocks.simps)
+    apply (metis end_refusal_notin_tocks filter_tocks.simps(1) filter_tocks_in_tocks)
+    apply (meson list.inject list.simps(3) tocks.simps)
+    by (metis append.left_neutral append_Cons filter_tocks.simps(1) filter_tocks_in_tocks mid_event_notin_tocks)
+next
+  fix x p Xa Y Z
+  assume "p @ [[Xa]\<^sub>R] \<in> P" "filter_tocks p @ [[Y]\<^sub>R] \<in> f \<rightarrow>\<^sub>C Q" "Z \<subseteq> Xa \<union> Y"
+    "{e \<in> Xa. e \<noteq> Tock} = {e \<in> Y. e \<noteq> Tock}" "[X]\<^sub>R # [Tock]\<^sub>E # x = p @ [[Z]\<^sub>R]"
+  then show "\<forall>p Xa. [X]\<^sub>R # [Tock]\<^sub>E # p @ [[Xa]\<^sub>R] \<in> P \<longrightarrow> (\<forall>Y. {e \<in> Xa. e \<noteq> Tock} = {e \<in> Y. e \<noteq> Tock} \<longrightarrow>
+        filter_tocks p @ [[Y]\<^sub>R] \<in> f \<rightarrow>\<^sub>C Q \<longrightarrow> (\<forall>Z\<subseteq>Xa \<union> Y. x \<noteq> p @ [[Z]\<^sub>R])) \<Longrightarrow>
+      \<exists>p. [X]\<^sub>R # [Tock]\<^sub>E # p @ [[Tick]\<^sub>E] \<in> P \<and> filter_tocks p \<in> f \<rightarrow>\<^sub>C Q \<and> x = p @ [[Tick]\<^sub>E]"
+    apply (cases p rule:ttWF.cases, safe, simp_all)
+    apply (erule_tac x=\<sigma> in allE, erule_tac x=Xa in allE, safe, simp_all)
+    apply (erule_tac x=Y in allE, safe)
+    unfolding PrefixTT_def apply safe apply simp_all
+    using in_tocks_last apply fastforce
+    using tocks.cases apply force
+    using in_tocks_last apply fastforce
+    apply (metis (no_types, hide_lams) append.left_neutral append_Cons append_assoc filter_tocks.simps(1)
+           filter_tocks_end_ref_tock filter_tocks_in_tocks mid_event_notin_tocks)
+    by blast+
+next
+  fix x p q2
+  assume " p \<in> P" "\<forall>p'. p \<noteq> p' @ [[Tick]\<^sub>E]" "\<forall>p' Y. p \<noteq> p' @ [[Y]\<^sub>R]" "filter_tocks p @ q2 \<in> f \<rightarrow>\<^sub>C Q" "\<forall>q' Y. q2 \<noteq> [Y]\<^sub>R # q'" "[X]\<^sub>R # [Tock]\<^sub>E # x = p @ q2"
+  then show "\<forall>p. [X]\<^sub>R # [Tock]\<^sub>E # p \<in> P \<longrightarrow>
+           (\<exists>p'. p = p' @ [[Tick]\<^sub>E]) \<or>
+           (\<exists>p' Y. p = p' @ [[Y]\<^sub>R]) \<or> (\<forall>q2. filter_tocks p @ q2 \<in> f \<rightarrow>\<^sub>C Q \<longrightarrow> (\<exists>q' Y. q2 = [Y]\<^sub>R # q') \<or> x \<noteq> p @ q2) \<Longrightarrow>
+       \<exists>p. [X]\<^sub>R # [Tock]\<^sub>E # p @ [[Tick]\<^sub>E] \<in> P \<and> filter_tocks p \<in> f \<rightarrow>\<^sub>C Q \<and> x = p @ [[Tick]\<^sub>E]"
+    apply (cases p rule:ttWF.cases, safe, simp_all, blast)
+    apply (erule_tac x=\<sigma> in allE, auto, erule_tac x=q2 in allE, auto, erule_tac x=q2 in allE, auto)
+    unfolding PrefixTT_def apply safe apply simp_all
+    apply (meson list.inject list.simps(3) tocks.simps)
+    apply (smt append_butlast_last_id butlast.simps(2) butlast_snoc last.simps last_snoc list.distinct(1) list.inject tocks.cases)
+    apply (meson list.inject list.simps(3) tocks.simps)
+    apply (smt append_Cons filter_tocks.simps(1) filter_tocks_in_tocks list.inject self_append_conv2 start_event_notin_tocks tocks.cases)
+    using \<open>\<forall>q' Y. q2 \<noteq> [Y]\<^sub>R # q'\<close> by blast+
+next
+  fix p
+  assume P_wf: "Ball P ttWF" "[X]\<^sub>R # [Tock]\<^sub>E # p @ [[Tick]\<^sub>E] \<in> P"
+  then have "Tock \<notin> X"
+    using ttWF.simps(5) by blast
+  then show "Event f \<notin> X \<Longrightarrow> filter_tocks p \<in> f \<rightarrow>\<^sub>C Q \<Longrightarrow> [X]\<^sub>R # [Tock]\<^sub>E # filter_tocks p \<in> f \<rightarrow>\<^sub>C Q"
+    unfolding PrefixTT_def apply auto
+    apply (erule_tac x="[X]\<^sub>R # [Tock]\<^sub>E # filter_tocks p" in ballE, auto)
+    apply (smt Ball_Collect tocks.tock_insert_in_tocks)
+    apply (metis end_refusal_notin_tocks filter_tocks_in_tocks)
+    apply (erule_tac x="[X]\<^sub>R # [Tock]\<^sub>E # filter_tocks p" in ballE, auto)
+    apply (smt Ball_Collect tocks.tock_insert_in_tocks)
+    by (metis append.left_neutral append_Cons filter_tocks_in_tocks mid_event_notin_tocks)
+next
+  fix p Xa Y Z
+  assume " Ball P ttWF" "Event f \<notin> X" "[X]\<^sub>R # [Tock]\<^sub>E # p @ [[Xa]\<^sub>R] \<in> P" "filter_tocks p @ [[Y]\<^sub>R] \<in> f \<rightarrow>\<^sub>C Q"
+    "Z \<subseteq> Xa \<union> Y" "{e \<in> Xa. e \<noteq> Tock} = {e \<in> Y. e \<noteq> Tock}"
+  then show "\<forall>pa Xa. pa @ [[Xa]\<^sub>R] \<in> P \<longrightarrow> (\<forall>Y. {e \<in> Xa. e \<noteq> Tock} = {e \<in> Y. e \<noteq> Tock} \<longrightarrow> Z \<subseteq> Xa \<union> Y \<longrightarrow>
+      filter_tocks pa @ [[Y]\<^sub>R] \<in> f \<rightarrow>\<^sub>C Q \<longrightarrow> [X]\<^sub>R # [Tock]\<^sub>E # p \<noteq> pa) \<Longrightarrow> False"
+    apply (erule_tac x="[X]\<^sub>R # [Tock]\<^sub>E # p" in allE)
+    apply (erule_tac x="Xa" in allE, safe, simp_all)
+    apply (erule_tac x="Y" in allE, simp)
+    unfolding PrefixTT_def apply (safe, simp_all add: notin_tocks)
+    apply (erule_tac x="[X]\<^sub>R # [Tock]\<^sub>E # filter_tocks p" in ballE, safe, simp_all)
+    apply (smt Ball_Collect tocks.tock_insert_in_tocks ttWF.simps(5))
+    apply (smt Ball_Collect tocks.tock_insert_in_tocks ttWF.simps(5))
+    by (metis append.left_neutral append_Cons append_assoc filter_tocks_end_ref_tock filter_tocks_in_tocks mid_event_notin_tocks)
+next
+  fix p q2
+  assume "Ball P ttWF" "Event f \<notin> X" "[X]\<^sub>R # [Tock]\<^sub>E # p \<in> P" "\<forall>p'. p \<noteq> p' @ [[Tick]\<^sub>E]"
+    "\<forall>p' Y. p \<noteq> p' @ [[Y]\<^sub>R]" "filter_tocks p @ q2 \<in> f \<rightarrow>\<^sub>C Q" "\<forall>q' Y. q2 \<noteq> [Y]\<^sub>R # q'"
+  then show "\<forall>pa. pa \<in> P \<longrightarrow>
+            (\<exists>p'. pa = p' @ [[Tick]\<^sub>E]) \<or>
+            (\<exists>p' Y. pa = p' @ [[Y]\<^sub>R]) \<or>
+            (\<forall>q2a. filter_tocks pa @ q2a \<in> f \<rightarrow>\<^sub>C Q \<longrightarrow> (\<exists>q' Y. q2a = [Y]\<^sub>R # q') \<or> [X]\<^sub>R # [Tock]\<^sub>E # p @ q2 \<noteq> pa @ q2a) \<Longrightarrow>
+       \<exists>pa. pa @ [[Tick]\<^sub>E] \<in> P \<and> filter_tocks pa \<in> f \<rightarrow>\<^sub>C Q \<and> [X]\<^sub>R # [Tock]\<^sub>E # p @ q2 = pa @ [[Tick]\<^sub>E]"
+    apply (erule_tac x="[X]\<^sub>R # [Tock]\<^sub>E # p" in allE, auto simp add: Cons_eq_append_conv)
+    apply (erule_tac x="q2" in allE, auto)
+    unfolding PrefixTT_def
+  proof (safe, simp_all)
+    assume "Ball P ttWF" "[X]\<^sub>R # [Tock]\<^sub>E # p \<in> P"
+    then have "Tock \<notin> X"
+      by auto
+    then show "Event f \<notin> X \<Longrightarrow> filter_tocks p @ q2 \<in> tocks {x. x \<noteq> Tock \<and> x \<noteq> Event f} \<Longrightarrow>
+    \<forall>s\<in>tocks {x. x \<noteq> Tock \<and> x \<noteq> Event f}.
+       [X]\<^sub>R # [Tock]\<^sub>E # filter_tocks p @ q2 \<noteq> s \<and> (\<forall>\<sigma>\<in>Q. [X]\<^sub>R # [Tock]\<^sub>E # filter_tocks p @ q2 \<noteq> s @ [Event f]\<^sub>E # \<sigma>) \<Longrightarrow>
+    \<exists>s\<in>tocks {x. x \<noteq> Tock \<and> x \<noteq> Event f}. \<exists>Xa. Tock \<notin> Xa \<and> Event f \<notin> Xa \<and> [X]\<^sub>R # [Tock]\<^sub>E # filter_tocks p @ q2 = s @ [[Xa]\<^sub>R]"
+      apply (erule_tac x="[X]\<^sub>R # [Tock]\<^sub>E # filter_tocks p @ q2" in ballE, auto)
+      by (smt Ball_Collect tocks.tock_insert_in_tocks)
+  next
+    assume "Ball P ttWF" "[X]\<^sub>R # [Tock]\<^sub>E # p \<in> P"
+    then have "Tock \<notin> X"
+      by auto
+    then show "Event f \<notin> X \<Longrightarrow> filter_tocks p @ q2 \<in> tocks {x. x \<noteq> Tock \<and> x \<noteq> Event f} \<Longrightarrow>
+    \<forall>s\<in>tocks {x. x \<noteq> Tock \<and> x \<noteq> Event f}.
+       [X]\<^sub>R # [Tock]\<^sub>E # filter_tocks p @ q2 \<noteq> s \<and> (\<forall>\<sigma>\<in>Q. [X]\<^sub>R # [Tock]\<^sub>E # filter_tocks p @ q2 \<noteq> s @ [Event f]\<^sub>E # \<sigma>) \<Longrightarrow>
+    \<exists>s\<in>tocks {x. x \<noteq> Tock \<and> x \<noteq> Event f}. \<exists>Xa. Tock \<notin> Xa \<and> Event f \<notin> Xa \<and> [X]\<^sub>R # [Tock]\<^sub>E # filter_tocks p @ q2 = s @ [[Xa]\<^sub>R]"
+      apply (erule_tac x="[X]\<^sub>R # [Tock]\<^sub>E # filter_tocks p @ q2" in ballE, auto)
+      by (smt Ball_Collect tocks.tock_insert_in_tocks)
+  next
+    fix s
+    assume "Ball P ttWF" "[X]\<^sub>R # [Tock]\<^sub>E # p \<in> P"
+    then have "Tock \<notin> X"
+      by auto
+    then show "Event f \<notin> X \<Longrightarrow> s \<in> tocks {x. x \<noteq> Tock \<and> x \<noteq> Event f} \<Longrightarrow> [X]\<^sub>R # [Tock]\<^sub>E # s \<in> tocks {x. x \<noteq> Tock \<and> x \<noteq> Event f}"
+      by (smt Ball_Collect tocks.tock_insert_in_tocks)
+  next
+    fix s \<sigma>
+    assume "\<forall>x\<in>P. ttWF x" "[X]\<^sub>R # [Tock]\<^sub>E # p \<in> P"
+    then have "Tock \<notin> X"
+      by auto
+    then show "Event f \<notin> X \<Longrightarrow>  s \<in> tocks {x. x \<noteq> Tock \<and> x \<noteq> Event f} \<Longrightarrow> \<sigma> \<in> Q \<Longrightarrow> filter_tocks p @ q2 = s @ [Event f]\<^sub>E # \<sigma> \<Longrightarrow>
+          \<forall>sa\<in>tocks {x. x \<noteq> Tock \<and> x \<noteq> Event f}.
+              [X]\<^sub>R # [Tock]\<^sub>E # s @ [Event f]\<^sub>E # \<sigma> \<noteq> sa \<and> (\<forall>\<sigma>'\<in>Q. [X]\<^sub>R # [Tock]\<^sub>E # s @ [Event f]\<^sub>E # \<sigma> \<noteq> sa @ [Event f]\<^sub>E # \<sigma>') \<Longrightarrow>
+          \<exists>sa\<in>tocks {x. x \<noteq> Tock \<and> x \<noteq> Event f}. \<exists>Xa. Tock \<notin> Xa \<and> Event f \<notin> Xa \<and> [X]\<^sub>R # [Tock]\<^sub>E # s @ [Event f]\<^sub>E # \<sigma> = sa @ [[Xa]\<^sub>R]"
+      by (erule_tac x="[X]\<^sub>R # [Tock]\<^sub>E # s" in ballE, auto, smt Ball_Collect tocks.tock_insert_in_tocks)
+  qed
+qed
+
+lemma TimeSyncInterruptTT_PrefixTT_init_tock_any_refusal_subset:
+  "\<forall>x\<in>P. ttWF x \<Longrightarrow> Event f \<notin> X \<Longrightarrow> {t. \<exists>X. [X]\<^sub>R # [Tock]\<^sub>E # t \<in> P \<triangle>\<^sub>T f \<rightarrow>\<^sub>C Q} \<subseteq> {t. \<exists>X. [X]\<^sub>R # [Tock]\<^sub>E # t \<in> P} \<triangle>\<^sub>T f \<rightarrow>\<^sub>C Q"
+proof auto
+  fix x Xa
+  show "\<forall>x\<in>P. ttWF x \<Longrightarrow> Event f \<notin> X \<Longrightarrow> [Xa]\<^sub>R # [Tock]\<^sub>E # x \<in> P \<triangle>\<^sub>T f \<rightarrow>\<^sub>C Q \<Longrightarrow> x \<in> {t. \<exists>X. [X]\<^sub>R # [Tock]\<^sub>E # t \<in> P} \<triangle>\<^sub>T f \<rightarrow>\<^sub>C Q"
+    unfolding TimeSyncInterruptTT_def apply safe
+  proof simp_all
+    fix p
+    assume "[Xa]\<^sub>R # [Tock]\<^sub>E # x = p @ [[Tick]\<^sub>E]"
+    then obtain p' where "p = [Xa]\<^sub>R # [Tock]\<^sub>E # p' \<and> x = p' @ [[Tick]\<^sub>E]"
+      by (case_tac p rule:ttWF.cases, simp_all)
+    then show "p @ [[Tick]\<^sub>E] \<in> P \<Longrightarrow> filter_tocks p \<in> f \<rightarrow>\<^sub>C Q \<Longrightarrow>
+        \<exists>p. (\<exists>X. [X]\<^sub>R # [Tock]\<^sub>E # p @ [[Tick]\<^sub>E] \<in> P) \<and> filter_tocks p \<in> f \<rightarrow>\<^sub>C Q \<and> x = p @ [[Tick]\<^sub>E]"
+      unfolding PrefixTT_def apply auto
+      apply (meson list.inject list.simps(3) tocks.simps)
+      apply (metis end_refusal_notin_tocks filter_tocks.simps(1) filter_tocks_in_tocks)
+      apply (meson list.inject list.simps(3) tocks.simps)
+      by (metis append.left_neutral append_Cons filter_tocks.simps(1) filter_tocks_in_tocks mid_event_notin_tocks)
+  next
+    fix p Xb Y Z
+    assume case_assms: "Event f \<notin> X" "p @ [[Xb]\<^sub>R] \<in> P" "filter_tocks p @ [[Y]\<^sub>R] \<in> f \<rightarrow>\<^sub>C Q" "Z \<subseteq> Xb \<union> Y"
+      "{e \<in> Xb. e \<noteq> Tock} = {e \<in> Y. e \<noteq> Tock}"
+    assume "[Xa]\<^sub>R # [Tock]\<^sub>E # x = p @ [[Z]\<^sub>R]"
+    then obtain p' where p_def: "p = [Xa]\<^sub>R # [Tock]\<^sub>E # p' \<and> x = p' @ [[Z]\<^sub>R]"
+      by (case_tac p rule:ttWF.cases, simp_all)
+    have 1: "[Xa]\<^sub>R # [Tock]\<^sub>E # p' @ [[Xb]\<^sub>R] \<in> P"
+      using case_assms(2) p_def by auto
+    have 2: "filter_tocks p' @ [[Y]\<^sub>R] \<in> f \<rightarrow>\<^sub>C Q"
+      using case_assms(3) p_def unfolding PrefixTT_def using tocks.cases apply auto
+      apply (simp add: Cons_eq_append_conv filter_tocks_refusal_no_mid_event)
+      apply (metis append_Cons filter_tocks.simps(1) filter_tocks_refusal_no_mid_event)
+      by (metis append_Cons filter_tocks.simps(1) filter_tocks_refusal_no_mid_event)
+    show "\<forall>p X. (\<forall>Xa. [Xa]\<^sub>R # [Tock]\<^sub>E # p @ [[X]\<^sub>R] \<notin> P) \<or>
+             (\<forall>Y. {e \<in> X. e \<noteq> Tock} = {e \<in> Y. e \<noteq> Tock} \<longrightarrow> filter_tocks p @ [[Y]\<^sub>R] \<in> f \<rightarrow>\<^sub>C Q \<longrightarrow> (\<forall>Z\<subseteq>X \<union> Y. x \<noteq> p @ [[Z]\<^sub>R])) \<Longrightarrow>
+      \<exists>p. (\<exists>X. [X]\<^sub>R # [Tock]\<^sub>E # p @ [[Tick]\<^sub>E] \<in> P) \<and> filter_tocks p \<in> f \<rightarrow>\<^sub>C Q \<and> x = p @ [[Tick]\<^sub>E]"
+      using 1 2 case_assms(4) case_assms(5) p_def apply (erule_tac x=p' in allE, erule_tac x=Xb in allE, safe, simp_all)
+      by (erule_tac x=Y in allE, safe, blast)
+  next
+    fix p q2
+    assume case_assms: "Event f \<notin> X" "p \<in> P" "\<forall>p'. p \<noteq> p' @ [[Tick]\<^sub>E]" "\<forall>p' Y. p \<noteq> p' @ [[Y]\<^sub>R]"
+      "filter_tocks p @ q2 \<in> f \<rightarrow>\<^sub>C Q" "\<forall>q' Y. q2 \<noteq> [Y]\<^sub>R # q'"
+    assume "[Xa]\<^sub>R # [Tock]\<^sub>E # x = p @ q2"
+    then obtain p' where p_def: "p = [Xa]\<^sub>R # [Tock]\<^sub>E # p' \<and> x = p' @ q2"
+      using case_assms(4) case_assms(6) by (cases p rule:ttWF.cases, auto)
+    have 1: "[Xa]\<^sub>R # [Tock]\<^sub>E # p' \<in> P"
+      using p_def case_assms(2) by auto
+    have 2: "\<forall>p'. p \<noteq> p' @ [[Tick]\<^sub>E]"
+      using case_assms(3) by blast
+    have 3: "\<forall>p' Y. p \<noteq> p' @ [[Y]\<^sub>R]"
+      using case_assms(4) by blast
+    have 4: "filter_tocks p' @ q2 \<in> f \<rightarrow>\<^sub>C Q"
+      using p_def case_assms(5) unfolding PrefixTT_def apply auto
+         apply (meson list.inject neq_Nil_conv tocks.simps)
+      apply (case_tac s rule:ttWF.cases, auto)
+      apply (metis (no_types, lifting) list.inject list.simps(3) tocks.simps)
+      apply (meson list.inject list.simps(3) tocks.simps)
+      apply (case_tac s rule:ttWF.cases, auto)
+      by (metis (no_types, lifting) list.distinct(1) list.inject tocks.simps)
+    have 5: "\<forall>q' Y. q2 \<noteq> [Y]\<^sub>R # q'"
+      using case_assms(6) by blast
+
+    show "\<forall>p. (\<forall>X. [X]\<^sub>R # [Tock]\<^sub>E # p \<notin> P) \<or> (\<exists>p'. p = p' @ [[Tick]\<^sub>E]) \<or> (\<exists>p' Y. p = p' @ [[Y]\<^sub>R]) \<or>
+        (\<forall>q2. filter_tocks p @ q2 \<in> f \<rightarrow>\<^sub>C Q \<longrightarrow> (\<exists>q' Y. q2 = [Y]\<^sub>R # q') \<or> x \<noteq> p @ q2) \<Longrightarrow>
+      \<exists>p. (\<exists>X. [X]\<^sub>R # [Tock]\<^sub>E # p @ [[Tick]\<^sub>E] \<in> P) \<and> filter_tocks p \<in> f \<rightarrow>\<^sub>C Q \<and> x = p @ [[Tick]\<^sub>E]"
+      using 1 2 3 4 5 p_def by (erule_tac x=p' in allE, auto)
+  qed
+qed
+
+lemma ttWF_priTT_imp_ttWF1: "\<And>\<sigma> Q. ttWF x \<Longrightarrow> priTT p x y \<sigma> Q \<Longrightarrow> ttWF y"
+  by (induct x y rule:ttWF2.induct, auto, unfold prirefTT_def, auto, (case_tac \<rho> rule:ttWF.cases, auto)+)
+
+lemma ttWF_priTT_imp_ttWF2: "\<And>\<sigma> Q. ttWF y \<Longrightarrow> priTT p x y \<sigma> Q \<Longrightarrow> ttWF x"
+  by (induct x y rule:ttWF2.induct, auto, (case_tac \<sigma> rule:ttWF.cases, auto)+)
+
+lemma PriTT_wf: 
+  "\<forall>x\<in>P. ttWF x \<Longrightarrow> \<forall>x\<in>PriTT p P. ttWF x"
+  unfolding PriTT_def using ttWF_priTT_imp_ttWF2 by blast
+
+lemma priTT_init_event_eq:
+  "\<And>\<sigma>. ttWF x \<Longrightarrow> ttWF y \<Longrightarrow> x priTT\<^sub>[\<^sub>p\<^sub>,\<^sub>[Event e]\<^sub>E # \<sigma>\<^sub>,\<^sub>P\<^sub>] y = x priTT\<^sub>[\<^sub>p\<^sub>,\<^sub>\<sigma>\<^sub>,\<^sub>{\<sigma>. [Event e]\<^sub>E # \<sigma> \<in> P}\<^sub>] y"
+  by (induct x y rule:ttWF2.induct, auto, unfold prirefTT_def, auto)
+
+lemma priTT_prefix_eq: 
+  "\<And>\<rho> \<sigma> P. ttWF y \<Longrightarrow> x priTT\<^sub>[\<^sub>p\<^sub>,\<^sub>\<sigma> @ \<rho>\<^sub>,\<^sub>P\<^sub>] y = x priTT\<^sub>[\<^sub>p\<^sub>,\<^sub>\<rho>\<^sub>,\<^sub>{t. \<sigma> @ t \<in> P}\<^sub>] y"
+  apply (induct x y rule:ttWF2.induct, auto simp add: prirefTT_def)
+  apply (case_tac \<sigma> rule:ttWF.cases, auto)
+  using ttWF.simps(10) ttWF_priTT_imp_ttWF2 apply blast
+  using ttWF.simps(6) ttWF_priTT_imp_ttWF2 by blast+
+
+lemma PriTT_init_event:
+  "\<forall>x\<in>P. ttWF x \<Longrightarrow> maximal(p,Event e) \<Longrightarrow> {t. [Event e]\<^sub>E # t \<in> PriTT p P} = PriTT p {t. [Event e]\<^sub>E # t \<in> P}"
+  unfolding PriTT_def apply auto
+  apply (case_tac s rule:ttWF.cases, auto, metis priTT_init_event_eq ttWF.simps(4) ttWF_priTT_imp_ttWF2)
+  by (rule_tac x="[Event e]\<^sub>E # s" in exI, auto, metis priTT_init_event_eq ttWF.simps(4) ttWF_priTT_imp_ttWF2)
+
+lemma prirefTT_subset: "P \<subseteq> Q \<Longrightarrow> prirefTT p \<sigma> P X \<subseteq> prirefTT p \<sigma> Q X"
+  unfolding prirefTT_def by auto
+
+lemma maximal_notin_prirefTT: "maximal(p, e) \<Longrightarrow> e \<notin> X \<Longrightarrow> e \<notin> prirefTT p \<sigma> P X"
+  unfolding prirefTT_def by (auto simp add: some_higher_not_maximal)
+
+lemma tt_prefix_subset_priTT: "\<And>P  \<rho>' t. ttWF \<rho> \<Longrightarrow> ttWF \<sigma> \<Longrightarrow> \<rho>' \<lesssim>\<^sub>C \<rho> \<Longrightarrow> \<rho> priTT\<^sub>[\<^sub>p\<^sub>,\<^sub>t\<^sub>,\<^sub>P\<^sub>] \<sigma> \<Longrightarrow> \<exists>\<sigma>'. \<rho>' priTT\<^sub>[\<^sub>p\<^sub>,\<^sub>t\<^sub>,\<^sub>P\<^sub>] \<sigma>' \<and> \<sigma>' \<lesssim>\<^sub>C \<sigma>"
+  apply (induct \<rho> \<sigma> rule:ttWF2.induct, auto)
+  using priTT.simps(1) tt_prefix_subset.simps(1) tt_prefix_subset_antisym apply blast
+  apply (case_tac \<rho>' rule:ttWF.cases, auto)
+  using priTT.simps(1) tt_prefix_subset.simps(1) apply blast
+  apply (meson dual_order.trans priTT.simps(2) tt_prefix_subset_refl)
+  apply (case_tac \<rho>' rule:ttWF.cases, auto)
+  using priTT.simps(1) tt_prefix_subset.simps(1) apply blast
+  using priTT.simps(1) priTT.simps(4) tt_prefix_subset_refl apply blast
+  apply (case_tac \<rho>' rule:ttWF.cases, auto)
+  using priTT.simps(1) tt_prefix_subset.simps(1) apply blast
+  apply (meson priTT.simps(4) tt_prefix_subset.simps(3))
+  apply (case_tac \<rho>' rule:ttWF.cases, auto)
+  using priTT.simps(1) tt_prefix_subset.simps(1) apply blast
+  apply (meson priTT.simps(4) tt_prefix_subset.simps(3) ttevent.distinct(3))
+  apply (case_tac \<rho>' rule:ttWF.cases, auto)
+  using priTT.simps(1) tt_prefix_subset.simps(1) apply blast
+  apply (meson equalityD1 order_trans priTT.simps(2) tt_prefix_subset.simps(1) tt_prefix_subset.simps(2))
+  by (meson dual_order.trans equalityE priTT.simps(3) tt_prefix_subset.simps(2) tt_prefix_subset.simps(3))
+
+lemma TT1_PriTT: "\<forall>x\<in>P. ttWF x \<Longrightarrow> TT1 P \<Longrightarrow> TT1 (PriTT p P)"
+  unfolding PriTT_def TT1_def
+proof auto
+  fix \<rho> \<sigma> s
+  assume P_wf: "\<forall>x\<in>P. ttWF x"
+  assume TT1_P: "\<forall>\<rho>. (\<exists>\<sigma>. \<rho> \<lesssim>\<^sub>C \<sigma> \<and> \<sigma> \<in> P) \<longrightarrow> \<rho> \<in> P"
+  assume s_in_P: "s \<in> P"
+  assume \<sigma>_priTT_s: "\<sigma> priTT\<^sub>[\<^sub>p\<^sub>,\<^sub>[]\<^sub>,\<^sub>P\<^sub>] s"
+  assume \<rho>_tt_prefix_subset_\<sigma>: "\<rho> \<lesssim>\<^sub>C \<sigma>"
+
+  have s_wf: "ttWF s"
+    using P_wf s_in_P by blast
+  have \<sigma>_wf: "ttWF \<sigma>"
+    using P_wf \<sigma>_priTT_s s_in_P ttWF_priTT_imp_ttWF2 by blast
+  obtain s' where "\<rho> priTT\<^sub>[\<^sub>p\<^sub>,\<^sub>[]\<^sub>,\<^sub>P\<^sub>] s' \<and> s' \<lesssim>\<^sub>C s"
+    using \<rho>_tt_prefix_subset_\<sigma> \<sigma>_priTT_s \<sigma>_wf s_wf tt_prefix_subset_priTT by blast
+  then show "\<exists>s. \<rho> priTT\<^sub>[\<^sub>p\<^sub>,\<^sub>[]\<^sub>,\<^sub>P\<^sub>] s \<and> s \<in> P"
+    using TT1_P s_in_P by blast
+qed
+
+lemma hide_trace_end_refusal:
+  "\<And>x. x @ [[X]\<^sub>R] \<in> hide_trace H y \<Longrightarrow> \<exists>y' Y. y = y' @ [[Y]\<^sub>R] \<and> X \<subseteq> Y \<and> H \<subseteq> Y"
+proof (induct H y rule:hide_trace.induct, auto)
+  fix e \<sigma> x Xa
+  assume ind_hyp: "\<And>x. x @ [[X]\<^sub>R] \<in> hide_trace Xa \<sigma> \<Longrightarrow> \<exists>y' Y. \<sigma> = y' @ [[Y]\<^sub>R] \<and> X \<subseteq> Y \<and> Xa \<subseteq> Y"
+  assume "x @ [[X]\<^sub>R] \<in> hide_trace Xa \<sigma>"
+  then have "\<exists>y' Y. \<sigma> = y' @ [[Y]\<^sub>R] \<and> X \<subseteq> Y \<and> Xa \<subseteq> Y"
+    using ind_hyp by auto
+  then show "\<exists>y' Y. [Event e]\<^sub>E # \<sigma> = y' @ [[Y]\<^sub>R] \<and> X \<subseteq> Y \<and> Xa \<subseteq> Y"
+    by auto
+next
+  fix e \<sigma> x s' Xa
+  assume ind_hyp: "\<And>x. x @ [[X]\<^sub>R] \<in> hide_trace Xa \<sigma> \<Longrightarrow> \<exists>y' Y. \<sigma> = y' @ [[Y]\<^sub>R] \<and> X \<subseteq> Y \<and> Xa \<subseteq> Y"
+  assume s'_in_hide_trace_\<sigma>: "s' \<in> hide_trace Xa \<sigma>" and x_X_eq_e_s': "x @ [[X]\<^sub>R] = [Event e]\<^sub>E # s'"
+  obtain x' where x'_def: "s' = x' @ [[X]\<^sub>R] \<and> x = [Event e]\<^sub>E # x'"
+    using x_X_eq_e_s' by (induct x rule:ttWF.induct, auto)
+  then have "\<exists>y' Y. \<sigma> = y' @ [[Y]\<^sub>R] \<and> X \<subseteq> Y \<and> Xa \<subseteq> Y"
+    using ind_hyp s'_in_hide_trace_\<sigma> by blast
+  then show "\<exists>y' Y. [Event e]\<^sub>E # \<sigma> = y' @ [[Y]\<^sub>R] \<and> X \<subseteq> Y \<and> Xa \<subseteq> Y"
+    by auto
+next
+  fix Xa Y s x
+  assume ind_hyp: "\<And>x. x @ [[X]\<^sub>R] \<in> hide_trace Xa s \<Longrightarrow> \<exists>y' Y. s = y' @ [[Y]\<^sub>R] \<and> X \<subseteq> Y \<and> Xa \<subseteq> Y"
+  assume "x @ [[X]\<^sub>R] \<in> hide_trace Xa s"
+  then have "\<exists>y' Y. s = y' @ [[Y]\<^sub>R] \<and> X \<subseteq> Y \<and> Xa \<subseteq> Y"
+    using ind_hyp by blast
+  then show "\<exists>y' Ya. [Y]\<^sub>R # [Tock]\<^sub>E # s = y' @ [[Ya]\<^sub>R] \<and> X \<subseteq> Ya \<and> Xa \<subseteq> Ya"
+    by auto
+next
+  fix Xa Y s x s' Z
+  assume ind_hyp: "\<And>x. x @ [[X]\<^sub>R] \<in> hide_trace Xa s \<Longrightarrow> \<exists>y' Y. s = y' @ [[Y]\<^sub>R] \<and> X \<subseteq> Y \<and> Xa \<subseteq> Y"
+  assume x_X_eq_Z_Tock_s': "x @ [[X]\<^sub>R] = [Z]\<^sub>R # [Tock]\<^sub>E # s'" and s'_in_hide_trace_\<sigma>': "s' \<in> hide_trace Xa s"
+  obtain x' where x'_def: "s' = x' @ [[X]\<^sub>R] \<and> x = [Z]\<^sub>R # [Tock]\<^sub>E # x'"
+    using x_X_eq_Z_Tock_s' by (induct x rule:ttWF.induct, auto)
+  then have "\<exists>y' Y. s = y' @ [[Y]\<^sub>R] \<and> X \<subseteq> Y \<and> Xa \<subseteq> Y"
+    using ind_hyp s'_in_hide_trace_\<sigma>' by auto
+  then show "\<exists>y' Ya. [Y]\<^sub>R # [Tock]\<^sub>E # s = y' @ [[Ya]\<^sub>R] \<and> X \<subseteq> Ya \<and> Xa \<subseteq> Ya"
+    by auto
+qed
+
+lemma priTT_end_refusal:
+  "(x @ [[X]\<^sub>R]) priTT\<^sub>[\<^sub>p\<^sub>,\<^sub>\<sigma>\<^sub>,\<^sub>Q\<^sub>] y \<Longrightarrow> \<exists>y' Y. y = y' @ [[Y]\<^sub>R] \<and> X \<subseteq> prirefTT p (\<sigma> @ y') Q Y"
+proof (induct p x y \<sigma> Q rule:priTT.induct, auto)
+  fix p v va \<sigma> Q
+  assume "[[X]\<^sub>R] priTT\<^sub>[\<^sub>p\<^sub>,\<^sub>\<sigma>\<^sub>,\<^sub>Q\<^sub>] (v # va)"
+  then have "\<exists>Y. [[X]\<^sub>R] priTT\<^sub>[\<^sub>p\<^sub>,\<^sub>\<sigma>\<^sub>,\<^sub>Q\<^sub>] [[Y]\<^sub>R] \<and> v = [Y]\<^sub>R \<and> va = []"
+    by (cases v, auto, (cases va, auto)+)
+  then show "\<exists>y' Y. v # va = y' @ [[Y]\<^sub>R] \<and> X \<subseteq> prirefTT p (\<sigma> @ y') Q Y"
+    by auto
+qed
+
+thm TimeSyncInterruptTT_def
+
+lemma TimeSyncInterruptTT_PrefixTT_end_refusal:
+  assumes Q_wf: "\<forall>x\<in>Q. ttWF x"
+  shows "x @ [[X]\<^sub>R] \<in> P \<triangle>\<^sub>T (e \<rightarrow>\<^sub>C Q) \<Longrightarrow>
+    (\<exists> x'. x' @ [[X]\<^sub>R] \<in> Q) 
+    \<or> (\<exists>Xa. x @ [[Xa]\<^sub>R] \<in> P \<and> Event e \<notin> Xa \<and> X \<subseteq> Xa)"
+  unfolding TimeSyncInterruptTT_def
+proof (safe, simp_all)
+  fix Xa Y
+  assume case_assms: "x @ [[Xa]\<^sub>R] \<in> P" "filter_tocks x @ [[Y]\<^sub>R] \<in> e \<rightarrow>\<^sub>C Q" "X \<subseteq> Xa \<union> Y" "{e \<in> Xa. e \<noteq> Tock} = {e \<in> Y. e \<noteq> Tock}"
+  have "Tock \<notin> Y \<and> Event e \<notin> Y"
+    using case_assms(2) unfolding PrefixTT_def by (auto simp add: notin_tocks filter_tocks_refusal_no_mid_event)
+  then have "X \<subseteq> Xa \<and> Event e \<notin> Xa"
+    using case_assms(3) case_assms(4) by blast
+  then show "\<forall>Xa. x @ [[Xa]\<^sub>R] \<in> P \<longrightarrow> Event e \<in> Xa \<or> \<not> X \<subseteq> Xa \<Longrightarrow> \<exists>x'. x' @ [[X]\<^sub>R] \<in> Q"
+    using case_assms(1) by blast
+next
+  fix p q2
+  assume case_assms: "\<forall>p' Y. p \<noteq> p' @ [[Y]\<^sub>R]" "filter_tocks p @ q2 \<in> e \<rightarrow>\<^sub>C Q" "\<forall>q' Y. q2 \<noteq> [Y]\<^sub>R # q'" "x @ [[X]\<^sub>R] = p @ q2"
+  have q2_wf: "ttWF q2"
+    using PrefixTT_wf assms case_assms(2) filter_tocks_in_tocks tocks_append_wf2 by fastforce
+  have "\<exists>q'. q2 = q' @ [[X]\<^sub>R]"
+    using case_assms apply - apply (induct x p rule:ttWF2.induct, auto,  fastforce)
+    by (metis append_Nil2 append_butlast_last_id case_assms(1) case_assms(4) last_appendR last_snoc)+
+  then have "\<exists>q''. q2 = [Event e]\<^sub>E # q'' @ [[X]\<^sub>R]"
+    using case_assms(2) case_assms(3) q2_wf apply auto
+    apply (case_tac q' rule:ttWF.cases, auto)
+    unfolding PrefixTT_def apply auto
+    using mid_event_notin_tocks apply force+
+  proof -
+    fix ea \<sigma> s \<sigma>'
+    show "\<And>p. filter_tocks p @ [Event ea]\<^sub>E # \<sigma> @ [[X]\<^sub>R] = s @ [Event e]\<^sub>E # \<sigma>' \<Longrightarrow> s \<in> tocks {x. x \<noteq> Tock \<and> x \<noteq> Event e}
+      \<Longrightarrow> ea = e"
+      apply (induct s rule:ttWF.induct, auto simp add: notin_tocks)
+      apply (case_tac p rule:ttWF.cases, auto)
+      apply (metis (no_types, lifting) append_eq_Cons_conv filter_tocks_in_tocks list.inject start_event_notin_tocks ttevent.inject ttobs.inject(1))
+      apply (metis (no_types, lifting) append_eq_Cons_conv filter_tocks_in_tocks list.inject start_event_notin_tocks ttevent.inject ttobs.inject(1))
+      apply (metis (no_types, lifting) append_eq_Cons_conv filter_tocks_in_tocks list.inject start_event_notin_tocks ttevent.inject ttobs.inject(1))
+      apply (metis (no_types, lifting) append_eq_Cons_conv filter_tocks_in_tocks list.inject start_event_notin_tocks ttevent.inject ttobs.inject(1))
+      apply (metis (no_types, lifting) append_eq_Cons_conv filter_tocks_in_tocks list.inject start_event_notin_tocks ttevent.inject ttobs.inject(1))
+      apply (metis (no_types, lifting) append_eq_Cons_conv filter_tocks_in_tocks list.inject start_event_notin_tocks ttevent.inject ttobs.inject(1))
+      apply (metis (no_types, lifting) append_eq_Cons_conv filter_tocks_in_tocks list.inject start_event_notin_tocks ttevent.inject ttobs.inject(1))
+      apply (metis (no_types, lifting) append_eq_Cons_conv filter_tocks_in_tocks list.inject start_event_notin_tocks ttevent.inject ttobs.inject(1))
+    proof (metis (no_types, lifting) append_eq_Cons_conv filter_tocks_in_tocks list.inject start_event_notin_tocks ttevent.inject ttobs.inject(1))
+      fix Xa \<sigma>'' p
+      show "(\<And>p. filter_tocks p @ [Event ea]\<^sub>E # \<sigma> @ [[X]\<^sub>R] = \<sigma>'' @ [Event e]\<^sub>E # \<sigma>' \<Longrightarrow> \<sigma>'' \<in> tocks {x. x \<noteq> Tock \<and> x \<noteq> Event e} \<Longrightarrow> ea = e) \<Longrightarrow>
+       filter_tocks p @ [Event ea]\<^sub>E # \<sigma> @ [[X]\<^sub>R] = [Xa]\<^sub>R # [Tock]\<^sub>E # \<sigma>'' @ [Event e]\<^sub>E # \<sigma>' \<Longrightarrow>
+       [Xa]\<^sub>R # [Tock]\<^sub>E # \<sigma>'' \<in> tocks {x. x \<noteq> Tock \<and> x \<noteq> Event e} \<Longrightarrow> ea = e"
+        apply (induct p rule:filter_tocks.induct, auto)
+        by (metis (no_types, lifting) list.distinct(1) list.inject tocks.simps)
+    qed
+  qed
+  then show "\<exists>x'. x' @ [[X]\<^sub>R] \<in> Q"
+    using case_assms(2) unfolding PrefixTT_def apply auto
+    using mid_event_notin_tocks apply force+
+    by (metis (no_types, lifting) append_butlast_last_id append_is_Nil_conv last.simps last_appendR list.distinct(1) ttobs.simps(4))
+qed
+
+section \<open>Timelock Freedom\<close>
+
+fun timelock_free_trace :: "'e tttrace \<Rightarrow> bool" where
+  "timelock_free_trace [] = True" |
+  "timelock_free_trace ([e]\<^sub>E # \<rho>) = timelock_free_trace \<rho>" |
+  "timelock_free_trace ([X]\<^sub>R # \<rho>) = (Tock \<notin> X \<and> timelock_free_trace \<rho>)"
+
+definition timelock_free :: "'e ttprocess \<Rightarrow> bool" where
+  "timelock_free P = (\<forall>t\<in>P. timelock_free_trace t)"
+
+lemma tt_prefix_subset_timelock_free:
+  "\<rho> \<lesssim>\<^sub>C \<sigma> \<Longrightarrow> timelock_free_trace \<sigma> \<Longrightarrow> timelock_free_trace \<rho>"
+  by (induct \<rho> \<sigma> rule:tt_prefix_subset.induct, auto)
+
+lemma TT2_timelock_free_contains_tock: 
+  assumes TT2_P: "TT2 P" and timelock_free_P: "timelock_free P" and s_X_in_P: "s @ [[X]\<^sub>R] \<in> P"
+  shows "s @ [[X]\<^sub>R, [Tock]\<^sub>E] \<in> P"
+proof -
+  have "timelock_free_trace (s @ [[X]\<^sub>R]) \<Longrightarrow> Tock \<notin> X"
+    by (induct s rule:timelock_free_trace.induct, auto)
+  have "s @ [[X]\<^sub>R, [Tock]\<^sub>E] \<notin> P \<Longrightarrow> s @ [[X \<union> {Tock}]\<^sub>R] \<in> P"
+    using TT2_P s_X_in_P unfolding TT2_def apply (auto)
+    by (erule_tac x=s in allE, erule_tac x="[]" in allE, erule_tac x=X in allE, erule_tac x="{Tock}" in allE, auto)
+  also have "timelock_free_trace (s @ [[X \<union> {Tock}]\<^sub>R]) \<Longrightarrow> False"
+    by (induct s rule:timelock_free_trace.induct, auto)
+  then show "s @ [[X]\<^sub>R, [Tock]\<^sub>E] \<in> P"
+    using s_X_in_P timelock_free_P calculation unfolding timelock_free_def by auto
+qed
+
+lemma timelock_free_refusal_implies_tock:
+  "timelock_free P \<Longrightarrow> TT2 P \<Longrightarrow> t @ [[Z]\<^sub>R] \<in> P \<Longrightarrow> t @ [[Z]\<^sub>R, [Tock]\<^sub>E] \<in> P"
+  unfolding TT2_def timelock_free_def
+proof (erule_tac x="t" in allE, erule_tac x="[]" in allE, auto, erule_tac x=Z in allE, erule_tac x="{Tock}" in allE, auto)
+  assume "\<forall>x\<in>P. timelock_free_trace x" "t @ [[insert Tock Z]\<^sub>R] \<in> P"
+  then have "timelock_free_trace (t @ [[insert Tock Z]\<^sub>R])"
+    by auto
+  then have "False"
+    by (induct t rule:timelock_free_trace.induct, auto)
+  then show "t @ [[Z]\<^sub>R, [Tock]\<^sub>E] \<in> P"
+    by auto
+qed
+
+lemma timelock_free_StopTT: "timelock_free STOP\<^sub>C"
+  unfolding timelock_free_def StopTT_def
+proof auto
+  fix s :: "'a tttrace"
+  show "s \<in> tocks {x. x \<noteq> Tock} \<Longrightarrow> timelock_free_trace s"
+    by (induct s rule:tocks.induct, auto)
+next
+  fix s :: "'a tttrace" and X
+  show "s \<in> tocks {x. x \<noteq> Tock} \<Longrightarrow> Tock \<notin> X \<Longrightarrow> timelock_free_trace (s @ [[X]\<^sub>R])"
+    by (induct s rule:tocks.induct, auto)
+qed
+
+lemma RenamingTT_timelock_free:
+  "\<forall>x\<in>P. ttWF x \<Longrightarrow> timelock_free P \<Longrightarrow> timelock_free (RenamingTT P f)"
+  unfolding timelock_free_def RenamingTT_def
+proof auto
+  fix x
+  have "\<And>xa P. ttWF x \<Longrightarrow> \<forall>x\<in>P. timelock_free_trace x \<Longrightarrow> xa \<in> P \<Longrightarrow> x \<in> rename_trace f xa \<Longrightarrow> timelock_free_trace x"
+    apply (induct x rule:ttWF.induct, auto, case_tac xa rule:ttWF.cases, auto)
+    apply (case_tac xa rule:ttWF.cases, auto, metis insertI1 singletonD timelock_free_trace.simps(2))
+    by (case_tac xa rule:ttWF.cases, auto, metis insertI1 singletonD timelock_free_trace.simps(2) timelock_free_trace.simps(3))
+  then show "\<And>xa. \<forall>x\<in>P. ttWF x \<Longrightarrow> \<forall>x\<in>P. timelock_free_trace x \<Longrightarrow> xa \<in> P \<Longrightarrow> x \<in> rename_trace f xa \<Longrightarrow> timelock_free_trace x"
+    using rename_trace_ttWF by blast
+qed
+
+lemma PrefixTT_timelock_free:
+  "timelock_free P \<Longrightarrow> timelock_free (e \<rightarrow>\<^sub>C P)"
+  unfolding timelock_free_def PrefixTT_def
+proof auto
+  fix s
+  show "s \<in> tocks {x. x \<noteq> Tock \<and> x \<noteq> Event e} \<Longrightarrow> timelock_free_trace s"
+    apply (induct s rule:ttWF.induct, auto simp add: notin_tocks)
+    apply (metis (mono_tags, lifting) mem_Collect_eq tocks_wf ttWF.simps(5))
+    using tocks.simps by auto
+next
+  fix s X
+  show "s \<in> tocks {x. x \<noteq> Tock \<and> x \<noteq> Event e} \<Longrightarrow> Tock \<notin> X \<Longrightarrow> timelock_free_trace (s @ [[X]\<^sub>R])"
+    apply (induct s rule:ttWF.induct, auto simp add: notin_tocks)
+    apply (metis (mono_tags, lifting) mem_Collect_eq tocks_wf ttWF.simps(5))
+    using tocks.simps by auto
+next
+  fix s
+  show "s \<in> tocks {x. x \<noteq> Tock \<and> x \<noteq> Event e} \<Longrightarrow> timelock_free_trace s"
+    apply (induct s rule:ttWF.induct, auto simp add: notin_tocks)
+    apply (metis (mono_tags, lifting) mem_Collect_eq tocks_wf ttWF.simps(5))
+    using tocks.simps by auto
+next
+  fix s \<sigma>
+  show "\<forall>x\<in>P. timelock_free_trace x \<Longrightarrow> s \<in> tocks {x. x \<noteq> Tock \<and> x \<noteq> Event e} \<Longrightarrow> \<sigma> \<in> P \<Longrightarrow> timelock_free_trace (s @ [Event e]\<^sub>E # \<sigma>)"
+    apply (induct s rule:ttWF.induct, auto simp add: notin_tocks)
+    apply (metis (mono_tags, lifting) mem_Collect_eq tocks_wf ttWF.simps(5))
+    using tocks.cases by auto
+qed
+
+lemma StrictTimedInterruptTT_timelock_free:
+  "timelock_free P \<Longrightarrow> timelock_free Q \<Longrightarrow> timelock_free (P \<triangle>\<^bsub>n\<^esub> Q)"
+  unfolding StrictTimedInterruptTT_def timelock_free_def
+proof auto
+  fix p q
+  assume "\<forall>x\<in>P. timelock_free_trace x" "\<forall>x\<in>Q. timelock_free_trace x" "p \<in> P" "q \<in> Q"
+  then have "timelock_free_trace p \<and> timelock_free_trace q"
+    by auto
+  then show "timelock_free_trace (p @ q)"
+    by (induct p rule:timelock_free_trace.induct, auto)
+qed
+
+lemma TimeSyncInterruptTT_timelock_free:
+  "timelock_free P \<Longrightarrow> timelock_free Q \<Longrightarrow> timelock_free (P \<triangle>\<^sub>T Q)"
+  unfolding timelock_free_def TimeSyncInterruptTT_def
+proof (safe, simp_all)
+  fix p X Y Z
+  assume "Ball Q timelock_free_trace" "filter_tocks p @ [[Y]\<^sub>R] \<in> Q"
+  then have "timelock_free_trace (filter_tocks p @ [[Y]\<^sub>R])"
+    by blast
+  then have "Tock \<notin> Y"
+    by (induct p rule:filter_tocks.induct, auto)
+  then have "Z \<subseteq> X \<union> Y \<Longrightarrow> {e \<in> X. e \<noteq> Tock} = {e \<in> Y. e \<noteq> Tock} \<Longrightarrow> Z \<subseteq> X"
+    by blast
+  also assume "Ball P timelock_free_trace" "p @ [[X]\<^sub>R] \<in> P"
+  then have "timelock_free_trace (p @ [[X]\<^sub>R])"
+    by blast
+  then show "Z \<subseteq> X \<union> Y \<Longrightarrow> {e \<in> X. e \<noteq> Tock} = {e \<in> Y. e \<noteq> Tock} \<Longrightarrow>
+      timelock_free_trace (p @ [[Z]\<^sub>R])"
+    using calculation by (induct p rule:timelock_free_trace.induct, auto)
+next
+  fix p q2
+  assume "Ball P timelock_free_trace" "Ball Q timelock_free_trace" "p \<in> P" "filter_tocks p @ q2 \<in> Q"
+  then have "timelock_free_trace p \<and> timelock_free_trace (filter_tocks p @ q2)"
+    by blast
+  then show "timelock_free_trace (p @ q2)"
+    by (induct p rule:timelock_free_trace.induct, auto, case_tac \<rho> rule:ttWF.cases, auto)
+qed
+
+
+lemma PrefixTT_refusal_implies_tock: "[[Z]\<^sub>R] \<in> e \<rightarrow>\<^sub>C P \<Longrightarrow> [[Z]\<^sub>R, [Tock]\<^sub>E] \<in> e \<rightarrow>\<^sub>C P"
+  unfolding PrefixTT_def using tocks.simps by (auto simp add: notin_tocks Cons_eq_append_conv)
+
+lemma timelock_free_TimeSyncInterruptTT_PrefixTT_refusal_implies_tock:
+  assumes TT1_P: "TT1 P" and TT2_P: "TT2 P" and P_timelock_free: "timelock_free P"
+  assumes e_notin_Z: "Event e \<notin> Z"
+  shows "[[Z]\<^sub>R] \<in> P \<triangle>\<^sub>T e \<rightarrow>\<^sub>C Q \<Longrightarrow> [[Z]\<^sub>R, [Tock]\<^sub>E] \<in> P \<triangle>\<^sub>T e \<rightarrow>\<^sub>C Q"
+proof -
+  assume "[[Z]\<^sub>R] \<in> P \<triangle>\<^sub>T e \<rightarrow>\<^sub>C Q"
+  then obtain X Y where "[[X]\<^sub>R] \<in> P \<and> [[Y]\<^sub>R] \<in> e \<rightarrow>\<^sub>C Q \<and> Z \<subseteq> X \<union> Y \<and> {e \<in> X. e \<noteq> Tock} = {e \<in> Y. e \<noteq> Tock}"
+    unfolding TimeSyncInterruptTT_def by (auto, metis (no_types, lifting) append_eq_Cons_conv append_is_Nil_conv)
+  then have "Tock \<notin> X \<and> Tock \<notin> Y \<and> [[X]\<^sub>R] \<in> P \<and> [[Y]\<^sub>R] \<in> e \<rightarrow>\<^sub>C Q \<and> Z \<subseteq> X \<and> X = Y"
+    unfolding PrefixTT_def apply (safe, simp_all add: notin_tocks Cons_eq_append_conv)
+    using P_timelock_free timelock_free_def timelock_free_trace.simps(3) by fastforce+
+  then have "Tock \<notin> X \<and> Tock \<notin> Y \<and> [[X]\<^sub>R, [Tock]\<^sub>E] \<in> P \<and> [[Y]\<^sub>R, [Tock]\<^sub>E] \<in> e \<rightarrow>\<^sub>C Q \<and> Z \<subseteq> X \<and> X = Y"
+    by (metis P_timelock_free PrefixTT_refusal_implies_tock TT2_P append.left_neutral timelock_free_refusal_implies_tock)
+  then show "[[Z]\<^sub>R, [Tock]\<^sub>E] \<in> P \<triangle>\<^sub>T e \<rightarrow>\<^sub>C Q"
+    unfolding TimeSyncInterruptTT_def apply (auto, rule_tac x="[[Z]\<^sub>R, [Tock]\<^sub>E]" in exI, auto)
+    using TT1_P TT1_def tt_prefix_subset.simps(2) tt_prefix_subset_refl apply blast
+    by (smt PrefixTT_def PrefixTT_refusal_implies_tock Un_iff append_Nil e_notin_Z mem_Collect_eq subsetCE tocks.empty_in_tocks)
+qed
+
+subsection \<open>Timed Chaos\<close>
+
+definition TChaosTT :: "'a ttprocess" where
+  "TChaosTT = {t. ttWF t \<and> timelock_free_trace t}"
+
+lemma TChaos_wf:
+  "\<forall>x\<in>TChaosTT. ttWF x"
+  unfolding TChaosTT_def by auto
+
+lemma TT0_TChaos:
+  "TT0 TChaosTT"
+  unfolding TChaosTT_def TT0_def by (auto, rule_tac x="[]" in exI, auto)
+
+lemma TT1_TChaos:
+  "TT1 TChaosTT"
+  unfolding TChaosTT_def TT1_def apply auto
+  using tt_prefix_subset_ttWF apply blast
+  using tt_prefix_subset_timelock_free by blast
+
+lemma TT2_TChaos:
+  "TT2 TChaosTT"
+  unfolding TT2_def
+proof auto
+  fix \<rho> \<sigma> :: "'a tttrace" and X Y
+  assume \<rho>_X_\<sigma>_in_TChaos: "\<rho> @ [X]\<^sub>R # \<sigma> \<in> TChaosTT"
+  assume Y_disjoint: "Y \<inter> {e. e \<noteq> Tock \<and> \<rho> @ [[e]\<^sub>E] \<in> TChaosTT \<or> e = Tock \<and> \<rho> @ [[X]\<^sub>R, [e]\<^sub>E] \<in> TChaosTT} = {}"
+
+  have "\<rho> @ [[X]\<^sub>R, [Tock]\<^sub>E] \<in> TChaosTT"
+    using \<rho>_X_\<sigma>_in_TChaos unfolding TChaosTT_def by (simp, induct \<rho> rule:ttWF.induct, auto)
+  then have "Tock \<notin> Y"
+    using Y_disjoint by blast
+  then show "\<rho> @ [X \<union> Y]\<^sub>R # \<sigma> \<in> TChaosTT"
+    using \<rho>_X_\<sigma>_in_TChaos unfolding TChaosTT_def
+    by (simp, induct \<rho> rule:ttWF.induct, auto, cases \<sigma> rule:ttWF.cases, auto)
+qed
+
+lemma TChaos_timelock_free:
+  "timelock_free TChaosTT"
+  unfolding TChaosTT_def timelock_free_def by auto
+
+section \<open>Timelock event and partial ordering\<close>
+
+datatype 'e timelock_event = Timelock | OtherEvent 'e
+
+fun timelock_ordering :: "'e timelock_event ttevent \<Rightarrow> 'e timelock_event ttevent \<Rightarrow> bool" where
+  "timelock_ordering (Event Timelock) Tock = True" |
+  "timelock_ordering a b = (a=b)"
+
+lemma timelock_ordering_is_order: "timelock_ordering \<in> {x. class.order x (Event_Priority.less x)}"
+  unfolding class.order_def class.preorder_def class.order_axioms_def apply auto
+  by (case_tac x, auto, case_tac x, auto, case_tac y, auto, case_tac x, auto)
+
+lemma timelock_ordering_porder_cancel: "porder2f (f2porder timelock_ordering) = timelock_ordering"
+   using timelock_ordering_is_order by (subst f2porder_inverse[where y = timelock_ordering], auto)
+
+lemma Timelock_not_maximal: "\<not> maximal(f2porder timelock_ordering, Event Timelock)"
+  unfolding maximal_def my_le_def by (auto, rule_tac x="Tock" in exI, auto simp add: timelock_ordering_porder_cancel)
+
+lemma Tock_maximal: "maximal(f2porder timelock_ordering, Tock)"
+  unfolding maximal_def my_le_def by (auto simp add: timelock_ordering_porder_cancel)
+
+lemma Tick_maximal: "maximal(f2porder timelock_ordering, Tick)"
+  unfolding maximal_def my_le_def by (auto simp add: timelock_ordering_porder_cancel)
+
+lemma OtherEvent_maximal: "maximal(f2porder timelock_ordering, Event (OtherEvent e))"
+  unfolding maximal_def my_le_def by (auto simp add: timelock_ordering_porder_cancel)
+
+subsection \<open>Lemmas related to prioritisation using timelock_ordering\<close>
+
+lemma timelock_ordering_prirefTT: "TT2 P \<Longrightarrow> timelock_free P \<Longrightarrow> \<sigma> @ [[X]\<^sub>R] \<in> P \<Longrightarrow>
+  prirefTT (f2porder timelock_ordering) \<sigma> P X = X \<union> {Event Timelock}"
+  unfolding prirefTT_def my_le_def my_lt_def apply (auto simp add: timelock_ordering_porder_cancel)
+  using timelock_ordering.elims(2) apply blast+
+  using timelock_free_refusal_implies_tock by blast
+
+lemma PriTT_timelock_ordering_init_tock:
+  "\<forall>x\<in>P. ttWF x \<Longrightarrow> TT1 P \<Longrightarrow> TT2 P \<Longrightarrow> timelock_free P \<Longrightarrow>
+    {t. [X]\<^sub>R # [Tock]\<^sub>E # t \<in> PriTT (f2porder timelock_ordering) P}
+      = PriTT (f2porder timelock_ordering) {t. [{e\<in>X. e \<noteq> Event Timelock}]\<^sub>R # [Tock]\<^sub>E # t \<in> P}"
+  unfolding PriTT_def
+proof auto
+  fix x s
+  assume P_wf: "\<forall>x\<in>P. ttWF x" and TT1_P: "TT1 P" and TT2_P: "TT2 P" and P_timelock_free: "timelock_free P"
+  assume s_in_P: "s \<in> P"
+  
+  assume "([X]\<^sub>R # [Tock]\<^sub>E # x) priTT\<^sub>[\<^sub>f2porder timelock_ordering\<^sub>,\<^sub>[]\<^sub>,\<^sub>P\<^sub>] s"
+  then obtain Y y where x_priTT_y: "x priTT\<^sub>[\<^sub>f2porder timelock_ordering\<^sub>,\<^sub>[[Y]\<^sub>R, [Tock]\<^sub>E]\<^sub>,\<^sub>P\<^sub>] y" and
+      s_def: "s = [Y]\<^sub>R # [Tock]\<^sub>E # y" and
+      X_subset_prirefTT_Y: "X \<subseteq> prirefTT (f2porder timelock_ordering) [] P Y"
+    by (cases s rule:ttWF.cases, auto)
+
+  have ttWF_y: "ttWF y"
+    using P_wf s_def s_in_P ttWF.simps(5) by blast
+  have ttWF_x: "ttWF x"
+    using ttWF_priTT_imp_ttWF2 ttWF_y x_priTT_y by blast
+
+  have 1: "x priTT\<^sub>[\<^sub>f2porder timelock_ordering\<^sub>,\<^sub>[]\<^sub>,\<^sub>{t. [Y]\<^sub>R # [Tock]\<^sub>E # t \<in> P}\<^sub>] y"
+    using ttWF_y priTT_prefix_eq[where \<sigma>="[[Y]\<^sub>R, [Tock]\<^sub>E]", where \<rho>="[]"] x_priTT_y by auto
+
+  have "{e\<in>prirefTT (f2porder timelock_ordering) [] P Y. e \<noteq> Event Timelock} = {e\<in>Y. e \<noteq> Event Timelock}"
+    unfolding prirefTT_def apply auto
+    by (metis OtherEvent_maximal Tick_maximal Tock_maximal some_higher_not_maximal timelock_event.exhaust ttevent.exhaust)+
+  then have 2: "{e\<in>X. e \<noteq> Event Timelock} \<subseteq> Y"
+    using X_subset_prirefTT_Y by auto
+  then have "{t. [Y]\<^sub>R # [Tock]\<^sub>E # t \<in> P} \<subseteq> {t. [{e\<in>X. e \<noteq> Event Timelock}]\<^sub>R # [Tock]\<^sub>E # t \<in> P}"
+    apply auto using TT1_P TT1_def tt_prefix_subset.simps(2) tt_prefix_subset_refl by blast
+  then have "\<And>\<sigma>. x priTT\<^sub>[\<^sub>f2porder timelock_ordering\<^sub>,\<^sub>\<sigma>\<^sub>,\<^sub>{t. [Y]\<^sub>R # [Tock]\<^sub>E # t \<in> P}\<^sub>] y \<Longrightarrow>
+      x priTT\<^sub>[\<^sub>f2porder timelock_ordering\<^sub>,\<^sub>\<sigma>\<^sub>,\<^sub>{t. [{e\<in>X. e \<noteq> Event Timelock}]\<^sub>R # [Tock]\<^sub>E # t \<in> P}\<^sub>] y"
+    using ttWF_y ttWF_x apply -
+  proof (induct x y rule:ttWF2.induct, auto)
+    fix Xa Ya \<sigma> x
+    show "Xa \<subseteq> prirefTT (f2porder timelock_ordering) \<sigma> {t. [Y]\<^sub>R # [Tock]\<^sub>E # t \<in> P} Ya \<Longrightarrow>
+        {t. [Y]\<^sub>R # [Tock]\<^sub>E # t \<in> P} \<subseteq> {t. [{e \<in> X. e \<noteq> Event Timelock}]\<^sub>R # [Tock]\<^sub>E # t \<in> P} \<Longrightarrow>
+        x \<in> Xa \<Longrightarrow> x \<in> prirefTT (f2porder timelock_ordering) \<sigma> {t. [{e \<in> X. e \<noteq> Event Timelock}]\<^sub>R # [Tock]\<^sub>E # t \<in> P} Ya"
+      by (meson prirefTT_subset subset_iff)
+  next
+    fix \<rho> f \<sigma> \<sigma>' Z
+    assume Z_in_P: "[Y]\<^sub>R # [Tock]\<^sub>E # \<sigma>' @ [[Z]\<^sub>R] \<in> P"
+    assume f_in_prirefTT_Z: "Event f \<notin> prirefTT (f2porder timelock_ordering) \<sigma>' {t. [Y]\<^sub>R # [Tock]\<^sub>E # t \<in> P} Z"
+
+    show "maximal(f2porder timelock_ordering,Event f)"
+    proof (cases f, auto simp add: OtherEvent_maximal)
+      have "timelock_free_trace ([Y]\<^sub>R # [Tock]\<^sub>E # \<sigma>' @ [[Z]\<^sub>R])"
+        using Z_in_P P_timelock_free unfolding timelock_free_def by auto
+      then have "Tock \<notin> Z"
+        by (auto, induct \<sigma>' rule:timelock_free_trace.induct, auto)
+      then have 1: "[Y]\<^sub>R # [Tock]\<^sub>E # \<sigma>' @ [[Z]\<^sub>R, [Tock]\<^sub>E] \<in> P"
+        using TT2_P Z_in_P unfolding TT2_def apply auto
+        apply (erule_tac x="[Y]\<^sub>R # [Tock]\<^sub>E # \<sigma>'" in allE, erule_tac x="[]" in allE)
+      proof (erule_tac x="Z" in allE, erule_tac x="{Tock}" in allE, auto)
+        assume "[Y]\<^sub>R # [Tock]\<^sub>E # \<sigma>' @ [[insert Tock Z]\<^sub>R] \<in> P"
+        then have "timelock_free_trace ([Y]\<^sub>R # [Tock]\<^sub>E # \<sigma>' @ [[insert Tock Z]\<^sub>R])"
+          using P_timelock_free unfolding timelock_free_def by auto
+        then have "False"
+          by (induct \<sigma>' rule:timelock_free_trace.induct, auto)
+        then show "[Y]\<^sub>R # [Tock]\<^sub>E # \<sigma>' @ [[Z]\<^sub>R, [Tock]\<^sub>E] \<in> P"
+          by auto
+      qed
+
+      assume "f  = Timelock"
+      then have 2: "[Y]\<^sub>R # [Tock]\<^sub>E # \<sigma>' @ [[Z]\<^sub>R, [Tock]\<^sub>E] \<notin> P"
+        using f_in_prirefTT_Z unfolding prirefTT_def my_lt_def my_le_def by (auto simp add: timelock_ordering_porder_cancel)
+
+      show "maximal(f2porder timelock_ordering,Event Timelock)"
+        using 1 2 by auto
+    qed
+  next
+    fix Xa \<rho> Ya \<sigma> \<sigma>' x
+    show "{t. [Y]\<^sub>R # [Tock]\<^sub>E # t \<in> P} \<subseteq> {t. [{e \<in> X. e \<noteq> Event Timelock}]\<^sub>R # [Tock]\<^sub>E # t \<in> P} \<Longrightarrow>
+        Xa \<subseteq> prirefTT (f2porder timelock_ordering) \<sigma>' {t. [Y]\<^sub>R # [Tock]\<^sub>E # t \<in> P} Ya \<Longrightarrow>
+        x \<in> Xa \<Longrightarrow> x \<in> prirefTT (f2porder timelock_ordering) \<sigma>' {t. [{e \<in> X. e \<noteq> Event Timelock}]\<^sub>R # [Tock]\<^sub>E # t \<in> P} Ya"
+      by (meson prirefTT_subset subset_iff)
+  next
+    fix Xa \<rho> Ya \<sigma> \<sigma>'
+    show "Tock \<in> prirefTT (f2porder timelock_ordering) \<sigma>' {t. [{e \<in> X. e \<noteq> Event Timelock}]\<^sub>R # [Tock]\<^sub>E # t \<in> P} Ya \<Longrightarrow> 
+        Tock \<notin> Ya \<Longrightarrow> False"
+      using Tock_maximal maximal_notin_prirefTT by blast
+  qed
+  then have 3: "x priTT\<^sub>[\<^sub>f2porder timelock_ordering\<^sub>,\<^sub>[]\<^sub>,\<^sub>{t. [{e\<in>X. e \<noteq> Event Timelock}]\<^sub>R # [Tock]\<^sub>E # t \<in> P}\<^sub>] y"
+    using "1" by blast
+
+  have 4: "[{e \<in> X. e \<noteq> Event Timelock}]\<^sub>R # [Tock]\<^sub>E # y \<in> P"
+    using "2" TT1_P TT1_def s_def s_in_P tt_prefix_subset.simps(2) tt_prefix_subset_refl by blast
+
+  show "\<exists>s. x priTT\<^sub>[\<^sub>(f2porder timelock_ordering)\<^sub>,\<^sub>[]\<^sub>,\<^sub>{t. [{e \<in> X. e \<noteq> Event Timelock}]\<^sub>R # [Tock]\<^sub>E # t \<in> P}\<^sub>] s \<and> [{e \<in> X. e \<noteq> Event Timelock}]\<^sub>R # [Tock]\<^sub>E # s \<in> P"
+    using 3 4 by (rule_tac x="y" in exI, auto)
+next
+  fix x s
+  assume P_wf: "\<forall>x\<in>P. ttWF x" and TT1_P: "TT1 P" and TT2_P: "TT2 P" and P_timelock_free: "timelock_free P"
+  assume x_priTT_s: "x priTT\<^sub>[\<^sub>f2porder timelock_ordering\<^sub>,\<^sub>[]\<^sub>,\<^sub>{t. [{e \<in> X. e \<noteq> Event Timelock}]\<^sub>R # [Tock]\<^sub>E # t \<in> P}\<^sub>] s"
+  assume tock_s_in_P: "[{e \<in> X. e \<noteq> Event Timelock}]\<^sub>R # [Tock]\<^sub>E # s \<in> P"
+  then have 1: "prirefTT (f2porder timelock_ordering) [] P {e \<in> X. e \<noteq> Event Timelock} = X \<union> {Event Timelock}"
+    unfolding prirefTT_def my_lt_def my_le_def apply safe apply (simp_all add: timelock_ordering_porder_cancel)
+    apply (case_tac x, auto, case_tac x1, auto)
+    using timelock_ordering.elims(2) apply blast
+    apply (meson TT1_P TT1_def subset_iff tt_prefix_subset.simps(1) tt_prefix_subset.simps(2) tt_prefix_subset.simps(3))
+    apply (meson TT1_P TT1_def tt_prefix_subset.simps(1) tt_prefix_subset.simps(2) tt_prefix_subset.simps(3) tt_prefix_subset_refl)
+    by (meson TT1_P TT1_def equalityE tt_prefix_subset.simps(1) tt_prefix_subset.simps(2) tt_prefix_subset.simps(3))
+
+  have ttWF_s: "ttWF s"
+    using P_wf tock_s_in_P ttWF.simps(5) by blast
+  have ttWF_x: "ttWF x"
+    using ttWF_priTT_imp_ttWF2 ttWF_s x_priTT_s by blast
+
+  have 2: "x priTT\<^sub>[\<^sub>f2porder timelock_ordering\<^sub>,\<^sub>[[{e \<in> X. e \<noteq> Event Timelock}]\<^sub>R, [Tock]\<^sub>E]\<^sub>,\<^sub>P\<^sub>] s"
+    using x_priTT_s ttWF_s priTT_prefix_eq[where \<sigma>="[[{e \<in> X. e \<noteq> Event Timelock}]\<^sub>R, [Tock]\<^sub>E]"] by fastforce 
+  
+  show "x priTT\<^sub>[\<^sub>f2porder timelock_ordering\<^sub>,\<^sub>[]\<^sub>,\<^sub>{t. [{e \<in> X. e \<noteq> Event Timelock}]\<^sub>R # [Tock]\<^sub>E # t \<in> P}\<^sub>] s \<Longrightarrow>
+      \<exists>s. ([X]\<^sub>R # [Tock]\<^sub>E # x) priTT\<^sub>[\<^sub>f2porder timelock_ordering\<^sub>,\<^sub>[]\<^sub>,\<^sub>P\<^sub>] s \<and> s \<in> P"
+    using tock_s_in_P P_wf 1 2 by (rule_tac x="[{e \<in> X. e \<noteq> Event Timelock}]\<^sub>R # [Tock]\<^sub>E # s" in exI, auto)
+qed
+
+fun tttrace_contains_event :: "'a ttevent \<Rightarrow> 'a tttrace \<Rightarrow> bool" where
+  "tttrace_contains_event x [] = False" |
+  "tttrace_contains_event x ([X]\<^sub>R # \<rho>) = tttrace_contains_event x \<rho>" |
+  "tttrace_contains_event x ([e]\<^sub>E # \<rho>) = (x = e \<or> tttrace_contains_event x \<rho>)"
+
+fun tttrace_refusal_contains_event :: "'a ttevent \<Rightarrow> 'a tttrace \<Rightarrow> bool" where
+  "tttrace_refusal_contains_event x [] = False" |
+  "tttrace_refusal_contains_event x ([X]\<^sub>R # \<rho>) = (x \<in> X \<or> tttrace_refusal_contains_event x \<rho>)" |
+  "tttrace_refusal_contains_event x ([e]\<^sub>E # \<rho>) = tttrace_refusal_contains_event x \<rho>"
+
+fun tttrace_insert_event_refusal :: "'a ttevent \<Rightarrow> 'a tttrace \<Rightarrow> 'a tttrace" where
+  "tttrace_insert_event_refusal x [] = []" |
+  "tttrace_insert_event_refusal x ([X]\<^sub>R # \<rho>) = [insert x X]\<^sub>R # tttrace_insert_event_refusal x \<rho>" |
+  "tttrace_insert_event_refusal x ([e]\<^sub>E # \<rho>) = [e]\<^sub>E # tttrace_insert_event_refusal x \<rho>"
+
+
+lemma timelock_ordering_priTT_reflexive:
+  "\<And>P \<sigma>. \<not> tttrace_contains_event (Event Timelock) \<rho> \<Longrightarrow> ttWF \<rho> \<Longrightarrow> \<rho> priTT\<^sub>[\<^sub>f2porder timelock_ordering\<^sub>,\<^sub>\<sigma>\<^sub>,\<^sub>P\<^sub>] \<rho>"
+  apply (induct \<rho> rule:ttWF.induct, auto)
+  unfolding prirefTT_def apply auto
+  using Tick_maximal apply blast
+  apply (metis OtherEvent_maximal timelock_event.exhaust)
+  by (meson Tock_maximal some_higher_not_maximal)
+
+section \<open>Function to add undefined behaviour after a deadline miss to a specification\<close>
+
+definition remove_timelock_spec :: "'e ttprocess \<Rightarrow> 'e timelock_event ttprocess" where
+  "remove_timelock_spec P =
+    (PriTT (f2porder timelock_ordering) ((RenamingTT P OtherEvent) \<triangle>\<^sub>T (Timelock \<rightarrow>\<^sub>C (STOP\<^sub>C \<triangle>\<^bsub>1\<^esub> TChaosTT))) \<setminus>\<^sub>C {Event Timelock})"
+
+lemma Timelock_prefix_deadline_miss_wf:
+  "\<forall>x\<in>(Timelock \<rightarrow>\<^sub>C (STOP\<^sub>C \<triangle>\<^bsub>Suc 0\<^esub> TChaosTT)). ttWF x"
+  by (metis (no_types, hide_lams) PrefixTT_wf StopTT_wf StrictTimedInterruptTT_wf TChaos_wf)
+
+lemma Timelock_prefix_deadline_miss_ttWFx:
+  "ttWFx (Timelock \<rightarrow>\<^sub>C (STOP\<^sub>C \<triangle>\<^bsub>Suc 0\<^esub> TChaosTT))"
+  using Timelock_prefix_deadline_miss_wf ttWF_is_ttWFw_ttWFx ttWFx_def by blast
+
+lemma unprioiritised_remove_timelock_spec_wf:
+  "\<forall>x\<in>P. ttWF x \<Longrightarrow> \<forall>x\<in>(RenamingTT P OtherEvent \<triangle>\<^sub>T Timelock \<rightarrow>\<^sub>C (STOP\<^sub>C \<triangle>\<^bsub>Suc 0\<^esub> TChaosTT)). ttWF x"
+  by (smt RenamingTT_wf TimeSyncInterruptTT_wf Timelock_prefix_deadline_miss_wf)
+
+lemma Timelock_prefix_deadline_miss_TT1:
+  "TT1 (Timelock \<rightarrow>\<^sub>C (STOP\<^sub>C \<triangle>\<^bsub>Suc 0\<^esub> TChaosTT))"
+  by (simp add: TT1_Prefix TT1_Stop TT1_StrictTimedInterrupt TT1_TChaos)
+
+lemma unprioiritised_remove_timelock_spec_TT1:
+  "\<forall>x\<in>P. ttWF x \<Longrightarrow> TT1 P \<Longrightarrow> TT1 (RenamingTT P OtherEvent \<triangle>\<^sub>T Timelock \<rightarrow>\<^sub>C (STOP\<^sub>C \<triangle>\<^bsub>Suc 0\<^esub> TChaosTT))"
+  by (simp add: RenamingTT_wf TT1_Renaming TT1_TimeSyncInterrupt Timelock_prefix_deadline_miss_TT1 Timelock_prefix_deadline_miss_wf)
+
+lemma Timelock_prefix_deadline_miss_TT2:
+  "TT2 (Timelock \<rightarrow>\<^sub>C (STOP\<^sub>C \<triangle>\<^bsub>Suc 0\<^esub> TChaosTT))"
+  by (simp add: TT0_Stop TT0_StrictTimedInterrupt TT0_TChaos TT1_Stop TT1_StrictTimedInterrupt TT1_TChaos
+        TT2_Prefix TT2_Stop TT2_StrictTimedInterrupt TT2_TChaos)
+
+lemma Renaming_ttWFx:
+  "\<forall>x\<in>P. ttWF x \<Longrightarrow> ttWFx (RenamingTT P OtherEvent)"
+  using ttWF_is_ttWFw_ttWFx ttWFx_def RenamingTT_wf by blast
+
+lemma unprioiritised_remove_timelock_spec_TT2:
+  "\<forall>x\<in>P. ttWF x \<Longrightarrow> TT1 P \<Longrightarrow> TT2 P \<Longrightarrow> TT2 (RenamingTT P OtherEvent \<triangle>\<^sub>T Timelock \<rightarrow>\<^sub>C (STOP\<^sub>C \<triangle>\<^bsub>Suc 0\<^esub> TChaosTT))"
+  by (simp add: RenamingTT_wf Renaming_ttWFx TT1_Renaming TT2_Renaming TT2_TimeSyncInterrupt Timelock_prefix_deadline_miss_TT1
+        Timelock_prefix_deadline_miss_TT2 Timelock_prefix_deadline_miss_ttWFx Timelock_prefix_deadline_miss_wf)
+
+lemma Timelock_prefix_deadline_miss_timelock_free:
+  "timelock_free (Timelock \<rightarrow>\<^sub>C (STOP\<^sub>C \<triangle>\<^bsub>Suc 0\<^esub> TChaosTT))"
+  by (simp add: PrefixTT_timelock_free StrictTimedInterruptTT_timelock_free TChaos_timelock_free timelock_free_StopTT)
+
+lemma unprioiritised_remove_timelock_spec_timelock_free:
+  "\<forall>x\<in>P. ttWF x \<Longrightarrow> timelock_free P \<Longrightarrow> timelock_free (RenamingTT P OtherEvent \<triangle>\<^sub>T Timelock \<rightarrow>\<^sub>C (STOP\<^sub>C \<triangle>\<^bsub>Suc 0\<^esub> TChaosTT))"
+  by (simp add: RenamingTT_timelock_free TimeSyncInterruptTT_timelock_free Timelock_prefix_deadline_miss_timelock_free)
+
+lemma unhidden_remove_timelock_spec_init_event:
+  assumes P_wf: "\<forall>x\<in>P. ttWF x"
+  shows "{t. [Event (OtherEvent e')]\<^sub>E # t \<in> PriTT (f2porder timelock_ordering) (RenamingTT P OtherEvent \<triangle>\<^sub>T Timelock \<rightarrow>\<^sub>C (STOP\<^sub>C \<triangle>\<^bsub>Suc 0\<^esub> TChaosTT))}
+    = PriTT (f2porder timelock_ordering) (RenamingTT {t. [Event e']\<^sub>E # t \<in> P} OtherEvent \<triangle>\<^sub>T Timelock \<rightarrow>\<^sub>C (STOP\<^sub>C \<triangle>\<^bsub>Suc 0\<^esub> TChaosTT))"
+  (is "?lhs = ?rhs")
+proof -
+  have "?lhs = PriTT (f2porder timelock_ordering) {t. [Event (OtherEvent e')]\<^sub>E # t \<in> RenamingTT P OtherEvent \<triangle>\<^sub>T Timelock \<rightarrow>\<^sub>C (STOP\<^sub>C \<triangle>\<^bsub>Suc 0\<^esub> TChaosTT)}"
+    by (metis OtherEvent_maximal P_wf PriTT_init_event unprioiritised_remove_timelock_spec_wf)
+  also have "... = PriTT (f2porder timelock_ordering) ({t. [Event (OtherEvent e')]\<^sub>E # t \<in> RenamingTT P OtherEvent} \<triangle>\<^sub>T Timelock \<rightarrow>\<^sub>C (STOP\<^sub>C \<triangle>\<^bsub>Suc 0\<^esub> TChaosTT))"
+    by (simp add: TimeSyncInterruptTT_PrefixTT_init_event)
+  also have "... = ?rhs"
+    by (simp add: RenamingTT_init_event inj_def)
+  then show ?thesis
+    using calculation by auto
+qed
+
+lemma unhidden_remove_timelock_spec_init_tock:
+  assumes P_wf: "\<forall>x\<in>P. ttWF x" and TT1_P: "TT1 P" and TT2_P: "TT2 P" and P_timelock_free: "timelock_free P"
+  shows "{t. [X']\<^sub>R # [Tock]\<^sub>E # t \<in> PriTT (f2porder timelock_ordering) (RenamingTT P OtherEvent \<triangle>\<^sub>T Timelock \<rightarrow>\<^sub>C (STOP\<^sub>C \<triangle>\<^bsub>Suc 0\<^esub> TChaosTT))}
+      = PriTT (f2porder timelock_ordering) (RenamingTT {t. [(lift_renaming_func OtherEvent) -` X']\<^sub>R # [Tock]\<^sub>E # t \<in> P} OtherEvent \<triangle>\<^sub>T Timelock \<rightarrow>\<^sub>C (STOP\<^sub>C \<triangle>\<^bsub>Suc 0\<^esub> TChaosTT))"
+proof -
+  have 1: "{t. [X']\<^sub>R # [Tock]\<^sub>E # t \<in> PriTT (f2porder timelock_ordering) (RenamingTT P OtherEvent \<triangle>\<^sub>T Timelock \<rightarrow>\<^sub>C (STOP\<^sub>C \<triangle>\<^bsub>Suc 0\<^esub> TChaosTT))}
+    = PriTT (f2porder timelock_ordering) {t. [{e \<in> X'. e \<noteq> Event Timelock}]\<^sub>R # [Tock]\<^sub>E # t \<in> RenamingTT P OtherEvent \<triangle>\<^sub>T Timelock \<rightarrow>\<^sub>C (STOP\<^sub>C \<triangle>\<^bsub>Suc 0\<^esub> TChaosTT)}"
+    using PriTT_timelock_ordering_init_tock[where P="RenamingTT P OtherEvent \<triangle>\<^sub>T Timelock \<rightarrow>\<^sub>C (STOP\<^sub>C \<triangle>\<^bsub>Suc 0\<^esub> TChaosTT)", where X=X']
+      P_timelock_free P_wf TT1_P TT2_P unprioiritised_remove_timelock_spec_TT1 unprioiritised_remove_timelock_spec_TT2
+      unprioiritised_remove_timelock_spec_timelock_free unprioiritised_remove_timelock_spec_wf by fastforce
+  have 2: "{t. [{e \<in> X'. e \<noteq> Event Timelock}]\<^sub>R # [Tock]\<^sub>E # t \<in> RenamingTT P OtherEvent \<triangle>\<^sub>T Timelock \<rightarrow>\<^sub>C (STOP\<^sub>C \<triangle>\<^bsub>Suc 0\<^esub> TChaosTT)}
+    = {t. [{e \<in> X'. e \<noteq> Event Timelock}]\<^sub>R # [Tock]\<^sub>E # t \<in> RenamingTT P OtherEvent} \<triangle>\<^sub>T Timelock \<rightarrow>\<^sub>C (STOP\<^sub>C \<triangle>\<^bsub>Suc 0\<^esub> TChaosTT)"
+    apply (subst TimeSyncInterruptTT_PrefixTT_init_tock[where X="{e \<in> X'. e \<noteq> Event Timelock}", where P="RenamingTT P OtherEvent", where Q="STOP\<^sub>C \<triangle>\<^bsub>Suc 0\<^esub> TChaosTT", where f=Timelock])
+    using P_wf RenamingTT_wf by auto
+  have 3: "{t. [{e \<in> X'. e \<noteq> Event Timelock}]\<^sub>R # [Tock]\<^sub>E # t \<in> RenamingTT P OtherEvent}
+    = {t. [X']\<^sub>R # [Tock]\<^sub>E # t \<in> RenamingTT P OtherEvent}"
+    unfolding RenamingTT_def apply auto
+    apply (case_tac xa rule:ttWF.cases, auto)
+    apply (rule_tac x="[{y. lift_renaming_func OtherEvent y \<in> X' \<and> lift_renaming_func OtherEvent y \<noteq> Event Timelock}]\<^sub>R # [Tock]\<^sub>E # \<sigma>" in bexI, auto)
+    apply (case_tac xa, auto)
+    apply (case_tac xa rule:ttWF.cases, auto)
+    apply (rule_tac x="[lift_renaming_func OtherEvent -` X']\<^sub>R # [Tock]\<^sub>E # \<sigma>" in bexI, auto)
+    apply (case_tac xa, auto)
+    done
+  have 4: "{t. [X']\<^sub>R # [Tock]\<^sub>E # t \<in> RenamingTT P OtherEvent}
+    = RenamingTT {t. [(lift_renaming_func OtherEvent) -` X']\<^sub>R # [Tock]\<^sub>E # t \<in> P} OtherEvent"
+    by (simp add: RenamingTT_init_tock)
+  show ?thesis
+    by (simp add: "1" "2" "3" "4")
+qed
+
+lemma unhidden_remove_timelock_spec_timelock_free_no_init_Timelock:
+  assumes P_wf: "\<forall>x\<in>P. ttWF x" and TT1_P: "TT1 P" and TT2_P: "TT2 P"
+  assumes P_timelock_free: "timelock_free P"
+  shows "[Event Timelock]\<^sub>E # \<sigma> \<notin> PriTT (f2porder timelock_ordering) (RenamingTT P OtherEvent \<triangle>\<^sub>T Timelock \<rightarrow>\<^sub>C (STOP\<^sub>C \<triangle>\<^bsub>Suc 0\<^esub> TChaosTT))"
+proof auto
+  assume "[Event Timelock]\<^sub>E # \<sigma> \<in> PriTT (f2porder timelock_ordering) (RenamingTT P OtherEvent \<triangle>\<^sub>T Timelock \<rightarrow>\<^sub>C (STOP\<^sub>C \<triangle>\<^bsub>Suc 0\<^esub> TChaosTT))"
+  then have "(\<exists> \<sigma>'. [Event Timelock]\<^sub>E # \<sigma>' \<in> (RenamingTT P OtherEvent \<triangle>\<^sub>T Timelock \<rightarrow>\<^sub>C (STOP\<^sub>C \<triangle>\<^bsub>Suc 0\<^esub> TChaosTT))
+    \<and> (\<exists>Z. [[Z]\<^sub>R] \<in> (RenamingTT P OtherEvent \<triangle>\<^sub>T Timelock \<rightarrow>\<^sub>C (STOP\<^sub>C \<triangle>\<^bsub>Suc 0\<^esub> TChaosTT))
+        \<and> Event Timelock \<notin> prirefTT (f2porder timelock_ordering) [] (RenamingTT P OtherEvent \<triangle>\<^sub>T Timelock \<rightarrow>\<^sub>C (STOP\<^sub>C \<triangle>\<^bsub>Suc 0\<^esub> TChaosTT)) Z))"
+    unfolding PriTT_def using Timelock_not_maximal by (safe, (case_tac s rule:ttWF.cases, auto)+)
+  then obtain \<sigma>' Z where 
+    Timelock_at_start: "[Event Timelock]\<^sub>E # \<sigma>' \<in> (RenamingTT P OtherEvent \<triangle>\<^sub>T Timelock \<rightarrow>\<^sub>C (STOP\<^sub>C \<triangle>\<^bsub>Suc 0\<^esub> TChaosTT))" and
+    refusal_at_start: "[[Z]\<^sub>R] \<in> (RenamingTT P OtherEvent \<triangle>\<^sub>T Timelock \<rightarrow>\<^sub>C (STOP\<^sub>C \<triangle>\<^bsub>Suc 0\<^esub> TChaosTT))" and
+    Timelock_not_eliminated: "Event Timelock \<notin> prirefTT (f2porder timelock_ordering) [] (RenamingTT P OtherEvent \<triangle>\<^sub>T Timelock \<rightarrow>\<^sub>C (STOP\<^sub>C \<triangle>\<^bsub>Suc 0\<^esub> TChaosTT)) Z"
+    by auto
+
+  have Tock_Timelock_notin_Z: "Tock \<notin> Z \<and> Event Timelock \<notin> Z"
+    using refusal_at_start unfolding TimeSyncInterruptTT_def
+  proof (safe, simp_all)
+    fix X Y Za :: "'a timelock_event ttevent set"
+    assume X_in_Renaming_P: "[[X]\<^sub>R] \<in> RenamingTT P OtherEvent"
+    assume Y_in_Timelock_Prefix: "[[Y]\<^sub>R] \<in> Timelock \<rightarrow>\<^sub>C (STOP\<^sub>C \<triangle>\<^bsub>Suc 0\<^esub> TChaosTT)"
+    assume Za_subset_X_Y: "Za \<subseteq> X \<union> Y"
+    assume Tock_in_Za: "Tock \<in> Za"
+
+    have "Tock \<in> X \<or> Tock \<in> Y"
+      using Tock_in_Za Za_subset_X_Y by auto
+    then show False
+    proof(auto)
+      assume Tock_in_X: "Tock \<in> X"
+      then have "\<exists> X'. Tock \<in> X' \<and> [[X']\<^sub>R] \<in> P"
+        using X_in_Renaming_P unfolding RenamingTT_def apply auto
+        apply (case_tac x rule:ttWF.cases, simp_all)
+        using lift_renaming_func.simps(2) by blast
+      then show False
+        using P_timelock_free unfolding timelock_free_def by auto
+    next
+      assume Tock_in_Y: "Tock \<in> Y"
+      then show "False"
+        using Y_in_Timelock_Prefix unfolding PrefixTT_def by (auto simp add: notin_tocks Cons_eq_append_conv)
+    qed
+  next
+    fix X Y Za :: "'a timelock_event ttevent set"
+    assume X_in_Renaming_P: "[[X]\<^sub>R] \<in> RenamingTT P OtherEvent"
+    assume Y_in_Timelock_Prefix: "[[Y]\<^sub>R] \<in> Timelock \<rightarrow>\<^sub>C (STOP\<^sub>C \<triangle>\<^bsub>Suc 0\<^esub> TChaosTT)"
+    assume Za_subset_X_Y: "Za \<subseteq> X \<union> Y"
+    assume X_Y_same_events: "{e \<in> X. e \<noteq> Tock} = {e \<in> Y. e \<noteq> Tock}"
+    assume Timelock_in_Za: "Event Timelock \<in> Za"
+     
+    have "Event Timelock \<in> X \<and> Event Timelock \<in> Y"
+      using Timelock_in_Za Za_subset_X_Y X_Y_same_events by auto
+    then show False
+      using Y_in_Timelock_Prefix unfolding PrefixTT_def by (auto simp add: notin_tocks Cons_eq_append_conv)
+  next
+    fix p q2 :: "'a timelock_event tttrace"
+    assume p_not_refusal: "\<forall>p' Y. p \<noteq> p' @ [[Y]\<^sub>R]"
+    assume q2_not_refusal: "\<forall>q' Y. q2 \<noteq> [Y]\<^sub>R # q'"
+    assume Z_eq_p_q2: "[[Z]\<^sub>R] = p @ q2"
+
+    have "p = [[Z]\<^sub>R] \<or> q2 = [[Z]\<^sub>R]"
+      by (metis Z_eq_p_q2 append_is_Nil_conv butlast.simps(2) butlast_append self_append_conv self_append_conv2)
+    then show False
+      using p_not_refusal q2_not_refusal by auto
+  next
+    fix p q2 :: "'a timelock_event tttrace"
+    assume p_not_refusal: "\<forall>p' Y. p \<noteq> p' @ [[Y]\<^sub>R]"
+    assume q2_not_refusal: "\<forall>q' Y. q2 \<noteq> [Y]\<^sub>R # q'"
+    assume Z_eq_p_q2: "[[Z]\<^sub>R] = p @ q2"
+
+    have "p = [[Z]\<^sub>R] \<or> q2 = [[Z]\<^sub>R]"
+      by (metis Z_eq_p_q2 append_is_Nil_conv butlast.simps(2) butlast_append self_append_conv self_append_conv2)
+    then show False
+      using p_not_refusal q2_not_refusal by auto
+  qed        
+
+  have "[[Z]\<^sub>R, [Tock]\<^sub>E] \<notin> (RenamingTT P OtherEvent \<triangle>\<^sub>T Timelock \<rightarrow>\<^sub>C (STOP\<^sub>C \<triangle>\<^bsub>Suc 0\<^esub> TChaosTT))"
+    using Timelock_not_eliminated unfolding prirefTT_def my_lt_def my_le_def by (auto simp add: timelock_ordering_porder_cancel)
+  then have "[[Z]\<^sub>R, [Tock]\<^sub>E] \<notin> RenamingTT P OtherEvent"
+    unfolding TimeSyncInterruptTT_def PrefixTT_def apply auto
+    apply (erule_tac x="[[Z]\<^sub>R, [Tock]\<^sub>E]" in allE, auto, erule_tac x="[]" in allE, auto)
+    apply (erule_tac x="[[Z]\<^sub>R, [Tock]\<^sub>E]" in ballE, auto)
+    by (metis (mono_tags, lifting) Tock_Timelock_notin_Z mem_Collect_eq subsetI tocks.empty_in_tocks tocks.tock_insert_in_tocks)
+  then have "\<exists>Z'. [[Z']\<^sub>R, [Tock]\<^sub>E] \<notin> P \<and> Z' = lift_renaming_func OtherEvent -` Z"
+    unfolding RenamingTT_def by auto
+  then obtain Z' where Z'_Tock_notin_P: "[[Z']\<^sub>R, [Tock]\<^sub>E] \<notin> P" and Z'_def: "Z' = lift_renaming_func OtherEvent -` Z"
+    by auto
+
+  have "[[Z]\<^sub>R] \<in> RenamingTT P OtherEvent"
+    using refusal_at_start unfolding TimeSyncInterruptTT_def
+  proof (safe, simp_all)
+    fix X Y Za and p :: "'b timelock_event tttrace"
+    assume X_in_Renaming_P:"[[X]\<^sub>R] \<in> RenamingTT P OtherEvent"
+    assume Za_subset_X_Y: "Za \<subseteq> X \<union> Y"
+    assume X_Y_same_events: "{e \<in> X. e \<noteq> Tock} = {e \<in> Y. e \<noteq> Tock}"
+    assume Z_eq_Za: "[] = p \<and> Z = Za"
+
+    have "Za \<subseteq> X"
+    proof auto
+      fix x
+      assume "x \<in> Za"
+      then have "(x \<in> X \<or> x \<in> Y) \<and> x \<noteq> Tock"
+        using Za_subset_X_Y Tock_Timelock_notin_Z Z_eq_Za by auto
+      then show "x \<in> X"
+        using X_Y_same_events by auto
+    qed
+    also have "TT1 (RenamingTT P OtherEvent)"
+      using TT1_Renaming TT1_P by blast
+    then show "[[Za]\<^sub>R] \<in> RenamingTT P OtherEvent"
+      using calculation X_in_Renaming_P unfolding TT1_def apply auto by (erule_tac x="[[Za]\<^sub>R]" in allE, auto)
+  next
+    fix p q2 :: "'a timelock_event tttrace"
+    assume p_not_refusal: "\<forall>p' Y. p \<noteq> p' @ [[Y]\<^sub>R]"
+    assume q_not_refusal: "\<forall>q' Y. q2 \<noteq> [Y]\<^sub>R # q'"
+    assume Z_eq_p_q: "[[Z]\<^sub>R] = p @ q2"
+
+    have "p = [[Z]\<^sub>R] \<or> q2 = [[Z]\<^sub>R]"
+      by (metis Z_eq_p_q append_Nil append_is_Nil_conv butlast_append butlast_snoc)
+    then show "p @ q2 \<in> RenamingTT P OtherEvent"
+      using p_not_refusal q_not_refusal by auto
+  qed
+  then have Z'_in_P: "[[Z']\<^sub>R] \<in> P"
+    unfolding RenamingTT_def by (auto, case_tac x rule:ttWF.cases, auto simp add: Z'_def)
+  then have "[[Z' \<union> {Tock}]\<^sub>R] \<in> P"
+    using TT2_P Z'_Tock_notin_P unfolding TT2_def 
+    apply (erule_tac x="[]" in allE, erule_tac x="[]" in allE)
+    by (erule_tac x="Z'" in allE, erule_tac x="{Tock}" in allE, auto)
+  then show False
+    using P_timelock_free timelock_free_def by fastforce
+qed
+
+lemma remove_timelock_spec_init_event:
+  assumes P_wf: "\<forall>x\<in>P. ttWF x"
+  shows "{t. [Event (OtherEvent e')]\<^sub>E # t \<in> remove_timelock_spec P}
+    = remove_timelock_spec {t. [Event e']\<^sub>E # t \<in> P}"
+  unfolding remove_timelock_spec_def HidingTT_def
+proof auto
+  fix p x
+  assume p_in_PriTT: "p \<in> PriTT (f2porder timelock_ordering) (RenamingTT P OtherEvent \<triangle>\<^sub>T Timelock \<rightarrow>\<^sub>C (STOP\<^sub>C \<triangle>\<^bsub>Suc 0\<^esub> TChaosTT))"
+  assume e'_x_in_hide_trace_p: "[Event (OtherEvent e')]\<^sub>E # x \<in> hide_trace {Event Timelock} p"
+
+  have "\<exists>p'. p = [Event (OtherEvent e')]\<^sub>E # p'"
+    using p_in_PriTT e'_x_in_hide_trace_p
+  proof (cases p rule:ttWF.cases, auto, case_tac \<sigma> rule:ttWF.cases, auto)
+    fix \<sigma>'
+    assume "[Event Timelock]\<^sub>E # [Event Timelock]\<^sub>E # \<sigma>'
+        \<in> PriTT (f2porder timelock_ordering) (RenamingTT P OtherEvent \<triangle>\<^sub>T Timelock \<rightarrow>\<^sub>C (STOP\<^sub>C \<triangle>\<^bsub>Suc 0\<^esub> TChaosTT))"
+    then have "\<exists>s.  [Event Timelock]\<^sub>E # [Event Timelock]\<^sub>E # s \<in> RenamingTT P OtherEvent \<triangle>\<^sub>T Timelock \<rightarrow>\<^sub>C (STOP\<^sub>C \<triangle>\<^bsub>Suc 0\<^esub> TChaosTT)"
+      unfolding PriTT_def apply (auto, case_tac s rule:ttWF.cases, auto simp add: Timelock_not_maximal)
+      by (case_tac \<sigma> rule:ttWF.cases, auto simp add: Timelock_not_maximal)
+    then show "False"
+      unfolding TimeSyncInterruptTT_def apply safe apply simp_all
+    proof -
+      fix s p :: "'a timelock_event tttrace"
+      assume "[Event Timelock]\<^sub>E # [Event Timelock]\<^sub>E # s = p @ [[Tick]\<^sub>E]"
+      then show "p @ [[Tick]\<^sub>E] \<in> RenamingTT P OtherEvent \<Longrightarrow> False"
+        unfolding RenamingTT_def by (cases p rule:ttWF.cases, auto, case_tac x rule:ttWF.cases, auto)
+    next
+      fix s p :: "'a timelock_event tttrace" and X Y Z
+      assume "[Event Timelock]\<^sub>E # [Event Timelock]\<^sub>E # s = p @ [[Z]\<^sub>R]"
+      then show "p @ [[X]\<^sub>R] \<in> RenamingTT P OtherEvent \<Longrightarrow> False"
+        unfolding RenamingTT_def by (cases p rule:ttWF.cases, auto, case_tac x rule:ttWF.cases, auto)
+    next
+      fix s p q2 :: "'a timelock_event tttrace"
+      assume p_in_P_renaming: "p \<in> RenamingTT P OtherEvent"
+      assume q2_in_Timelock_prefix: "filter_tocks p @ q2 \<in> Timelock \<rightarrow>\<^sub>C (STOP\<^sub>C \<triangle>\<^bsub>Suc 0\<^esub> TChaosTT)"
+      assume "[Event Timelock]\<^sub>E # [Event Timelock]\<^sub>E # s = p @ q2"
+      then have "(\<exists>p'. p = [Event Timelock]\<^sub>E # p') \<or> (p = [] \<and> q2 = [Event Timelock]\<^sub>E # [Event Timelock]\<^sub>E # s)"
+        by (induct p rule:ttWF.induct, auto)
+      then have "p = [] \<and> q2 = [Event Timelock]\<^sub>E # [Event Timelock]\<^sub>E # s"
+        using p_in_P_renaming unfolding RenamingTT_def by (auto, (case_tac x rule:ttWF.cases, auto)+)
+      then show "False"
+        using q2_in_Timelock_prefix unfolding PrefixTT_def apply (auto simp add: notin_tocks)
+         apply (metis (no_types, lifting) butlast.simps(2) butlast_snoc start_event_notin_tocks)
+        apply (case_tac sa rule:tocks.cases, auto)
+        unfolding StopTT_def StrictTimedInterruptTT_def apply (auto simp add: notin_tocks)
+        apply (metis butlast.simps(2) butlast_snoc last.simps last_snoc start_event_notin_tocks ttobs.simps(4))
+        by (metis (no_types, lifting) filter.simps(1) length_0_conv n_not_Suc_n tocks.simps tt_prefix.simps(2) tt_prefix_concat ttobs.simps(4))
+    qed
+  next  
+    fix \<sigma>'
+    assume "[Event Timelock]\<^sub>E # [Event (OtherEvent e')]\<^sub>E # \<sigma>'
+        \<in> PriTT (f2porder timelock_ordering) (RenamingTT P OtherEvent \<triangle>\<^sub>T Timelock \<rightarrow>\<^sub>C (STOP\<^sub>C \<triangle>\<^bsub>Suc 0\<^esub> TChaosTT))"
+    then have "\<exists>s.  [Event Timelock]\<^sub>E # [Event (OtherEvent e')]\<^sub>E # s \<in> RenamingTT P OtherEvent \<triangle>\<^sub>T Timelock \<rightarrow>\<^sub>C (STOP\<^sub>C \<triangle>\<^bsub>Suc 0\<^esub> TChaosTT)"
+      unfolding PriTT_def apply (auto, case_tac s rule:ttWF.cases, auto simp add: Timelock_not_maximal)
+      by (case_tac \<sigma> rule:ttWF.cases, auto simp add: Timelock_not_maximal)
+    then show "False"
+      unfolding TimeSyncInterruptTT_def apply safe apply simp_all
+    proof -
+      fix s p :: "'a timelock_event tttrace"
+      assume "[Event Timelock]\<^sub>E # [Event (OtherEvent e')]\<^sub>E # s = p @ [[Tick]\<^sub>E]"
+      then show "p @ [[Tick]\<^sub>E] \<in> RenamingTT P OtherEvent \<Longrightarrow> False"
+        unfolding RenamingTT_def by (cases p rule:ttWF.cases, auto, case_tac x rule:ttWF.cases, auto)
+    next
+      fix s p :: "'a timelock_event tttrace" and X Y Z
+      assume "[Event Timelock]\<^sub>E # [Event (OtherEvent e')]\<^sub>E # s = p @ [[Z]\<^sub>R]"
+      then show "p @ [[X]\<^sub>R] \<in> RenamingTT P OtherEvent \<Longrightarrow> False"
+        unfolding RenamingTT_def by (cases p rule:ttWF.cases, auto, case_tac x rule:ttWF.cases, auto)
+    next
+      fix s p q2 :: "'a timelock_event tttrace"
+      assume p_in_P_renaming: "p \<in> RenamingTT P OtherEvent"
+      assume q2_in_Timelock_prefix: "filter_tocks p @ q2 \<in> Timelock \<rightarrow>\<^sub>C (STOP\<^sub>C \<triangle>\<^bsub>Suc 0\<^esub> TChaosTT)"
+      assume "[Event Timelock]\<^sub>E # [Event (OtherEvent e')]\<^sub>E # s = p @ q2"
+      then have "(\<exists>p'. p = [Event Timelock]\<^sub>E # p') \<or> (p = [] \<and> q2 = [Event Timelock]\<^sub>E # [Event (OtherEvent e')]\<^sub>E # s)"
+        by (induct p rule:ttWF.induct, auto)
+      then have "p = [] \<and> q2 = [Event Timelock]\<^sub>E # [Event (OtherEvent e')]\<^sub>E # s"
+        using p_in_P_renaming unfolding RenamingTT_def by (auto, (case_tac x rule:ttWF.cases, auto)+)
+      then show "False"
+        using q2_in_Timelock_prefix unfolding PrefixTT_def apply (auto simp add: notin_tocks)
+         apply (metis (no_types, lifting) butlast.simps(2) butlast_snoc start_event_notin_tocks)
+        apply (case_tac sa rule:tocks.cases, auto)
+        unfolding StopTT_def StrictTimedInterruptTT_def apply (auto simp add: notin_tocks)
+        apply (metis butlast.simps(2) butlast_snoc last.simps last_snoc start_event_notin_tocks ttobs.simps(4))
+        by (metis (no_types, lifting) filter.simps(1) length_0_conv n_not_Suc_n tocks.simps tt_prefix.simps(2) tt_prefix_concat ttobs.simps(4))
+    qed
+  qed
+  then show "\<exists>xa. (\<exists>p. xa = hide_trace {Event Timelock} p \<and>
+                     p \<in> PriTT (f2porder timelock_ordering)
+                           (RenamingTT {t. [Event e']\<^sub>E # t \<in> P} OtherEvent \<triangle>\<^sub>T Timelock \<rightarrow>\<^sub>C (STOP\<^sub>C \<triangle>\<^bsub>Suc 0\<^esub> TChaosTT))) \<and>
+                x \<in> xa"
+    apply (auto, rule_tac x="hide_trace {Event Timelock} p'" in exI, auto, rule_tac x="p'" in exI, auto)
+    using P_wf p_in_PriTT unhidden_remove_timelock_spec_init_event apply fastforce
+    using e'_x_in_hide_trace_p by auto
+next
+  fix x p
+  assume p_in_PriTT: "p \<in> PriTT (f2porder timelock_ordering)
+      (RenamingTT {t. [Event e']\<^sub>E # t \<in> P} OtherEvent \<triangle>\<^sub>T Timelock \<rightarrow>\<^sub>C (STOP\<^sub>C \<triangle>\<^bsub>Suc 0\<^esub> TChaosTT))"
+  assume x_in_hide_trace_p: "x \<in> hide_trace {Event Timelock} p"
+
+  show "\<exists>xa. (\<exists>p. xa = hide_trace {Event Timelock} p \<and>
+                     p \<in> PriTT (f2porder timelock_ordering) (RenamingTT P OtherEvent \<triangle>\<^sub>T Timelock \<rightarrow>\<^sub>C (STOP\<^sub>C \<triangle>\<^bsub>Suc 0\<^esub> TChaosTT))) \<and>
+                [Event (OtherEvent e')]\<^sub>E # x \<in> xa"
+    apply (rule_tac x="hide_trace {Event Timelock} ([Event (OtherEvent e')]\<^sub>E # p)" in exI, auto)
+    apply (rule_tac x="[Event (OtherEvent e')]\<^sub>E # p" in exI, auto simp add: x_in_hide_trace_p)
+    using P_wf p_in_PriTT unhidden_remove_timelock_spec_init_event by fastforce
+qed
+
+lemma remove_timelock_spec_init_tock:
+  assumes P_wf: "\<forall>x\<in>P. ttWF x" and TT1_P: "TT1 P" and TT2_P: "TT2 P"
+  assumes P_timelock_free: "timelock_free P"
+  shows "{t. [X]\<^sub>R # [Tock]\<^sub>E # t \<in> remove_timelock_spec P}
+    = remove_timelock_spec {t. [lift_renaming_func OtherEvent -` X]\<^sub>R # [Tock]\<^sub>E # t \<in> P}"
+  (is "?lhs = ?rhs")
+proof -
+  have "?lhs = {t. [X]\<^sub>R # [Tock]\<^sub>E # t \<in> PriTT (f2porder timelock_ordering) (RenamingTT P OtherEvent \<triangle>\<^sub>T Timelock \<rightarrow>\<^sub>C (STOP\<^sub>C \<triangle>\<^bsub>1\<^esub> TChaosTT))} \<setminus>\<^sub>C {Event Timelock}"
+    unfolding remove_timelock_spec_def HidingTT_def
+  proof auto
+    fix x p
+    show "[X]\<^sub>R # [Tock]\<^sub>E # x \<in> hide_trace {Event Timelock} p \<Longrightarrow>
+           p \<in> PriTT (f2porder timelock_ordering) (RenamingTT P OtherEvent \<triangle>\<^sub>T Timelock \<rightarrow>\<^sub>C (STOP\<^sub>C \<triangle>\<^bsub>Suc 0\<^esub> TChaosTT)) \<Longrightarrow>
+           \<exists>xa. (\<exists>p. xa = hide_trace {Event Timelock} p \<and>
+                     [X]\<^sub>R # [Tock]\<^sub>E # p
+                     \<in> PriTT (f2porder timelock_ordering) (RenamingTT P OtherEvent \<triangle>\<^sub>T Timelock \<rightarrow>\<^sub>C (STOP\<^sub>C \<triangle>\<^bsub>Suc 0\<^esub> TChaosTT))) \<and>
+                x \<in> xa"
+      apply (case_tac p rule:ttWF.cases, auto)
+      apply (simp add: P_timelock_free P_wf TT1_P TT2_P unhidden_remove_timelock_spec_timelock_free_no_init_Timelock)
+      apply (rule_tac x="hide_trace {Event Timelock} \<sigma>" in exI, auto, rule_tac x=\<sigma> in exI, auto)
+      by (meson P_wf TT1_P TT1_PriTT TT1_def tt_prefix_subset.simps(2) tt_prefix_subset_refl unprioiritised_remove_timelock_spec_TT1 unprioiritised_remove_timelock_spec_wf)
+  next
+    fix x p
+    assume "[X]\<^sub>R # [Tock]\<^sub>E # p \<in> PriTT (f2porder timelock_ordering) (RenamingTT P OtherEvent \<triangle>\<^sub>T Timelock \<rightarrow>\<^sub>C (STOP\<^sub>C \<triangle>\<^bsub>Suc 0\<^esub> TChaosTT))"
+    then have "[X \<union> {Event Timelock}]\<^sub>R # [Tock]\<^sub>E # p \<in> PriTT (f2porder timelock_ordering) (RenamingTT P OtherEvent \<triangle>\<^sub>T Timelock \<rightarrow>\<^sub>C (STOP\<^sub>C \<triangle>\<^bsub>Suc 0\<^esub> TChaosTT))"
+      unfolding PriTT_def apply auto
+      apply (case_tac s rule:ttWF.cases, auto)
+    proof (rule_tac x="[Xa]\<^sub>R # [Tock]\<^sub>E # \<sigma>" in exI, auto)
+      fix Xa \<sigma>
+      assume "[Xa]\<^sub>R # [Tock]\<^sub>E # \<sigma> \<in> RenamingTT P OtherEvent \<triangle>\<^sub>T Timelock \<rightarrow>\<^sub>C (STOP\<^sub>C \<triangle>\<^bsub>Suc 0\<^esub> TChaosTT)"
+      then have "[[Xa]\<^sub>R, [Tock]\<^sub>E] \<in> RenamingTT P OtherEvent \<triangle>\<^sub>T Timelock \<rightarrow>\<^sub>C (STOP\<^sub>C \<triangle>\<^bsub>Suc 0\<^esub> TChaosTT)"
+        by (meson P_wf TT1_P TT1_def subsetI tt_prefix_subset.simps(1) tt_prefix_subset.simps(2) tt_prefix_subset.simps(3) unprioiritised_remove_timelock_spec_TT1)
+      then show "Event Timelock \<in> prirefTT (f2porder timelock_ordering) [] (RenamingTT P OtherEvent \<triangle>\<^sub>T Timelock \<rightarrow>\<^sub>C (STOP\<^sub>C \<triangle>\<^bsub>Suc 0\<^esub> TChaosTT)) Xa"
+        unfolding prirefTT_def my_le_def my_lt_def by (auto simp add: timelock_ordering_porder_cancel)
+    qed
+    then show "x \<in> hide_trace {Event Timelock} p \<Longrightarrow>
+           \<exists>xa. (\<exists>p. xa = hide_trace {Event Timelock} p \<and>
+                     p \<in> PriTT (f2porder timelock_ordering) (RenamingTT P OtherEvent \<triangle>\<^sub>T Timelock \<rightarrow>\<^sub>C (STOP\<^sub>C \<triangle>\<^bsub>Suc 0\<^esub> TChaosTT))) \<and>
+                [X]\<^sub>R # [Tock]\<^sub>E # x \<in> xa"
+      apply (rule_tac x="hide_trace {Event Timelock} ([X \<union> {Event Timelock}]\<^sub>R # [Tock]\<^sub>E # p)" in exI, auto)
+      by (rule_tac x="[X \<union> {Event Timelock}]\<^sub>R # [Tock]\<^sub>E # p" in exI, auto)
+  qed
+  also have "... = ?rhs"
+    by (simp add: P_timelock_free P_wf TT1_P TT2_P remove_timelock_spec_def unhidden_remove_timelock_spec_init_tock)
+  then show ?thesis
+    using calculation by auto
+qed
+
+lemma timelock_ordering_PriTT_init_tock_any_refusal_subset:
+  assumes P_wf: "\<forall>x\<in>P. ttWF x"
+  shows "PriTT (f2porder timelock_ordering) {t. [X]\<^sub>R # [Tock]\<^sub>E # t \<in> P}
+      \<subseteq> {t. \<exists>X. [X]\<^sub>R # [Tock]\<^sub>E # t \<in> PriTT (f2porder timelock_ordering) P}"
+  unfolding PriTT_def apply (auto, rule_tac x="{}" in exI, rule_tac x="[X]\<^sub>R # [Tock]\<^sub>E # s" in exI, auto)
+  unfolding prirefTT_def using assms ttWF.simps(5) apply auto
+  apply (meson Tock_maximal some_higher_not_maximal)
+  using assms ttWF.simps(5) priTT_prefix_eq[where \<rho>="[]", where \<sigma>="[[X]\<^sub>R, [Tock]\<^sub>E]"] by auto
+
+lemma remove_timelock_spec_init_tock_any_refusal_subset:
+  assumes P_wf: "\<forall>x\<in>P. ttWF x" and TT1_P: "TT1 P"
+  shows "remove_timelock_spec {t. [X]\<^sub>R # [Tock]\<^sub>E # t \<in> P}
+      \<subseteq> {t. \<exists>X. [X]\<^sub>R # [Tock]\<^sub>E # t \<in> remove_timelock_spec P}"
+  (is "?lhs \<subseteq> ?rhs")
+proof -
+  have "?lhs \<subseteq> PriTT (f2porder timelock_ordering) ({t. [lift_renaming_func OtherEvent ` X]\<^sub>R # [Tock]\<^sub>E # t \<in> RenamingTT P OtherEvent} \<triangle>\<^sub>T Timelock \<rightarrow>\<^sub>C (STOP\<^sub>C \<triangle>\<^bsub>1\<^esub> TChaosTT)) \<setminus>\<^sub>C {Event Timelock}"
+    unfolding remove_timelock_spec_def by (auto simp add: RenamingTT_init_tock2 inj_def)
+  also have "... \<subseteq> PriTT (f2porder timelock_ordering) {t. [lift_renaming_func OtherEvent ` X]\<^sub>R # [Tock]\<^sub>E # t \<in> RenamingTT P OtherEvent \<triangle>\<^sub>T Timelock \<rightarrow>\<^sub>C (STOP\<^sub>C \<triangle>\<^bsub>1\<^esub> TChaosTT)} \<setminus>\<^sub>C {Event Timelock}"    
+    using RenamingTT_wf assms by (subst TimeSyncInterruptTT_PrefixTT_init_tock, auto, case_tac x, auto)
+  also have "... \<subseteq> {t. \<exists>X. [X]\<^sub>R # [Tock]\<^sub>E # t \<in> PriTT (f2porder timelock_ordering) (RenamingTT P OtherEvent \<triangle>\<^sub>T Timelock \<rightarrow>\<^sub>C (STOP\<^sub>C \<triangle>\<^bsub>1\<^esub> TChaosTT)) \<setminus>\<^sub>C {Event Timelock}}"
+    unfolding HidingTT_def PriTT_def
+  proof auto
+    fix x p s
+    assume p_priTT_s: "p priTT\<^sub>[\<^sub>f2porder
+                  timelock_ordering\<^sub>,\<^sub>[]\<^sub>,\<^sub>{t. [lift_renaming_func OtherEvent ` X]\<^sub>R # [Tock]\<^sub>E # t
+                                               \<in> RenamingTT P OtherEvent \<triangle>\<^sub>T Timelock \<rightarrow>\<^sub>C (STOP\<^sub>C \<triangle>\<^bsub>Suc 0\<^esub> TChaosTT)}\<^sub>] s"
+    assume x_in_hide_trace_p: "x \<in> hide_trace {Event Timelock} p"
+    assume tock_S_in_TimeSyncInterrupt:
+      "[lift_renaming_func OtherEvent ` X]\<^sub>R # [Tock]\<^sub>E # s
+        \<in> RenamingTT P OtherEvent \<triangle>\<^sub>T Timelock \<rightarrow>\<^sub>C (STOP\<^sub>C \<triangle>\<^bsub>Suc 0\<^esub> TChaosTT)"
+
+    have ttWF_s: "ttWF s"
+      by (meson assms tock_S_in_TimeSyncInterrupt ttWF.simps(5) unprioiritised_remove_timelock_spec_wf)
+    have ttWF_p: "ttWF p"
+      using p_priTT_s ttWF_priTT_imp_ttWF2 ttWF_s by blast
+
+    have p_priTT_s: "p priTT\<^sub>[\<^sub>f2porder timelock_ordering\<^sub>,\<^sub>[[lift_renaming_func OtherEvent ` X]\<^sub>R, [Tock]\<^sub>E]\<^sub>,\<^sub>RenamingTT P OtherEvent \<triangle>\<^sub>T Timelock \<rightarrow>\<^sub>C (STOP\<^sub>C \<triangle>\<^bsub>Suc 0\<^esub> TChaosTT)\<^sub>] s"
+      using ttWF_s priTT_prefix_eq[where \<sigma>="[[lift_renaming_func OtherEvent ` X]\<^sub>R, [Tock]\<^sub>E]"] p_priTT_s by auto
+
+    have rename_X_in_TimeSyncInterruptTT: "[[lift_renaming_func OtherEvent ` X]\<^sub>R] \<in> RenamingTT P OtherEvent \<triangle>\<^sub>T Timelock \<rightarrow>\<^sub>C (STOP\<^sub>C \<triangle>\<^bsub>Suc 0\<^esub> TChaosTT)"
+      by (meson P_wf TT1_P TT1_def subset_iff tock_S_in_TimeSyncInterrupt tt_prefix_subset.simps(1) tt_prefix_subset.simps(2) unprioiritised_remove_timelock_spec_TT1)
+      
+    show "\<exists>X xa. (\<exists>p. xa = hide_trace {Event Timelock} p \<and>
+      (\<exists>s. p priTT\<^sub>[\<^sub>f2porder timelock_ordering\<^sub>,\<^sub>[]\<^sub>,\<^sub>RenamingTT P OtherEvent \<triangle>\<^sub>T Timelock \<rightarrow>\<^sub>C (STOP\<^sub>C \<triangle>\<^bsub>Suc 0\<^esub> TChaosTT)\<^sub>] s \<and>
+        s \<in> RenamingTT P OtherEvent \<triangle>\<^sub>T Timelock \<rightarrow>\<^sub>C (STOP\<^sub>C \<triangle>\<^bsub>Suc 0\<^esub> TChaosTT))) \<and> [X]\<^sub>R # [Tock]\<^sub>E # x \<in> xa"
+    proof (cases "Event Timelock \<in> prirefTT (f2porder timelock_ordering) [] (RenamingTT P OtherEvent \<triangle>\<^sub>T Timelock \<rightarrow>\<^sub>C (STOP\<^sub>C \<triangle>\<^bsub>Suc 0\<^esub> TChaosTT)) (lift_renaming_func OtherEvent ` X)") 
+      assume "Event Timelock \<in> prirefTT (f2porder timelock_ordering) [] (RenamingTT P OtherEvent \<triangle>\<^sub>T Timelock \<rightarrow>\<^sub>C (STOP\<^sub>C \<triangle>\<^bsub>Suc 0\<^esub> TChaosTT)) (lift_renaming_func OtherEvent ` X)"
+      then have "([{Event Timelock}]\<^sub>R # [Tock]\<^sub>E # p)
+        priTT\<^sub>[\<^sub>f2porder timelock_ordering\<^sub>,\<^sub>[]\<^sub>,\<^sub>RenamingTT P OtherEvent \<triangle>\<^sub>T Timelock \<rightarrow>\<^sub>C (STOP\<^sub>C \<triangle>\<^bsub>Suc 0\<^esub> TChaosTT)\<^sub>]
+          ([lift_renaming_func OtherEvent ` X]\<^sub>R # [Tock]\<^sub>E # s)"
+        using p_priTT_s apply auto
+        by (meson Tock_maximal assms maximal_notin_prirefTT tock_S_in_TimeSyncInterrupt
+            ttWF.simps(5) unprioiritised_remove_timelock_spec_wf)
+      then show ?thesis
+        apply (rule_tac x="{Event Timelock}" in exI, auto)
+        apply (rule_tac x="hide_trace {Event Timelock} ([{Event Timelock}]\<^sub>R # [Tock]\<^sub>E # p)" in exI, auto)
+        apply (rule_tac x="[{Event Timelock}]\<^sub>R # [Tock]\<^sub>E # p" in exI, auto)
+        apply (rule_tac x="[lift_renaming_func OtherEvent ` X]\<^sub>R # [Tock]\<^sub>E # s" in exI)
+        by (auto simp add: tock_S_in_TimeSyncInterrupt  x_in_hide_trace_p)
+    next
+      assume inner_assm: "Event Timelock
+        \<notin> prirefTT (f2porder timelock_ordering) [] (RenamingTT P OtherEvent \<triangle>\<^sub>T Timelock \<rightarrow>\<^sub>C (STOP\<^sub>C \<triangle>\<^bsub>Suc 0\<^esub> TChaosTT))
+          (lift_renaming_func OtherEvent ` X)"
+      then have "[[lift_renaming_func OtherEvent ` X]\<^sub>R, [Tock]\<^sub>E] \<notin> RenamingTT P OtherEvent \<triangle>\<^sub>T Timelock \<rightarrow>\<^sub>C (STOP\<^sub>C \<triangle>\<^bsub>Suc 0\<^esub> TChaosTT)"
+        unfolding prirefTT_def my_le_def my_lt_def by (auto simp add: timelock_ordering_porder_cancel)
+      also have "TT1 (RenamingTT P OtherEvent \<triangle>\<^sub>T Timelock \<rightarrow>\<^sub>C (STOP\<^sub>C \<triangle>\<^bsub>Suc 0\<^esub> TChaosTT))"
+        using P_wf TT1_P unprioiritised_remove_timelock_spec_TT1 by blast
+      then have "[[lift_renaming_func OtherEvent ` X]\<^sub>R, [Tock]\<^sub>E] \<in> RenamingTT P OtherEvent \<triangle>\<^sub>T Timelock \<rightarrow>\<^sub>C (STOP\<^sub>C \<triangle>\<^bsub>Suc 0\<^esub> TChaosTT)"
+        unfolding TT1_def apply auto
+        by (meson subsetI tock_S_in_TimeSyncInterrupt tt_prefix_subset.simps(1) tt_prefix_subset.simps(2) tt_prefix_subset.simps(3))
+      then show "\<exists>X xa. (\<exists>p. xa = hide_trace {Event Timelock} p \<and>
+            (\<exists>s. p priTT\<^sub>[\<^sub>f2porder timelock_ordering\<^sub>,\<^sub>[]\<^sub>,\<^sub>RenamingTT P OtherEvent \<triangle>\<^sub>T Timelock \<rightarrow>\<^sub>C (STOP\<^sub>C \<triangle>\<^bsub>Suc 0\<^esub> TChaosTT)\<^sub>] s \<and>
+                 s \<in> RenamingTT P OtherEvent \<triangle>\<^sub>T Timelock \<rightarrow>\<^sub>C (STOP\<^sub>C \<triangle>\<^bsub>Suc 0\<^esub> TChaosTT))) \<and> [X]\<^sub>R # [Tock]\<^sub>E # x \<in> xa"
+        using calculation by auto
+    qed
+  qed
+  also have "... \<subseteq> ?rhs"
+    unfolding remove_timelock_spec_def by auto
+  then show ?thesis
+    using calculation by auto
+qed
+
+lemma remove_timelock_spec_wf: "\<forall>x\<in>P. ttWF x \<Longrightarrow> \<forall>x\<in>remove_timelock_spec P. ttWF x"
+  unfolding remove_timelock_spec_def apply auto
+  by (smt HidingTT_wf PriTT_wf unprioiritised_remove_timelock_spec_wf)
+
+lemma remove_timelock_spec_timelock_free:
+  assumes P_wf: "\<forall>x\<in>P. ttWF x" and TT1_P: "TT1 P"
+  shows "timelock_free (remove_timelock_spec P)"
+  unfolding timelock_free_def
+proof (auto, rule ccontr)
+  fix x :: "'a timelock_event tttrace"
+  assume x_in_remove_timelock_spec_P: "x \<in> remove_timelock_spec P"
+
+  have ttWF_x: "ttWF x"
+    using P_wf remove_timelock_spec_wf x_in_remove_timelock_spec_P by blast
+
+  assume "\<not> timelock_free_trace x"
+  then have "\<exists>x' X. x = x' @ [[X]\<^sub>R] \<and> Tock \<in> X"
+    using ttWF_x apply - by (induct x rule:ttWF.induct, auto)
+  then obtain x' X where x_end_refusal: "x = x' @ [[X]\<^sub>R] \<and> Tock \<in> X"
+    by auto
+  then obtain x'2 X2 where 2: "x'2 @ [[X2]\<^sub>R] \<in> PriTT (f2porder timelock_ordering) (RenamingTT P OtherEvent \<triangle>\<^sub>T Timelock \<rightarrow>\<^sub>C (STOP\<^sub>C \<triangle>\<^bsub>1\<^esub> TChaosTT))
+    \<and> Tock \<in> X2 \<and> Event Timelock \<in> X2"
+    using x_in_remove_timelock_spec_P hide_trace_end_refusal unfolding remove_timelock_spec_def HidingTT_def by blast
+  then obtain x'3 X3 where 3: "x'3 @ [[X3]\<^sub>R] \<in> (RenamingTT P OtherEvent \<triangle>\<^sub>T Timelock \<rightarrow>\<^sub>C (STOP\<^sub>C \<triangle>\<^bsub>1\<^esub> TChaosTT))
+    \<and> Tock \<in> X3 \<and> X2 \<subseteq> prirefTT (f2porder timelock_ordering) x'3 (RenamingTT P OtherEvent \<triangle>\<^sub>T Timelock \<rightarrow>\<^sub>C (STOP\<^sub>C \<triangle>\<^bsub>1\<^esub> TChaosTT)) X3"
+    unfolding PriTT_def using priTT_end_refusal apply auto
+    by (smt Tock_maximal append_Nil maximal_notin_prirefTT priTT_end_refusal subsetCE)
+  then have "(\<exists>x'. x' @ [[X3]\<^sub>R] \<in> (STOP\<^sub>C \<triangle>\<^bsub>1\<^esub> TChaosTT)) \<or> (\<exists>Xa. x'3 @ [[Xa]\<^sub>R] \<in> RenamingTT P OtherEvent \<and> Event Timelock \<notin> Xa \<and> X3 \<subseteq> Xa)"
+    by (smt StopTT_wf StrictTimedInterruptTT_wf TChaos_wf TimeSyncInterruptTT_PrefixTT_end_refusal)
+  then show False
+  proof auto
+    fix x'
+    assume "x' @ [[X3]\<^sub>R] \<in> STOP\<^sub>C \<triangle>\<^bsub>Suc 0\<^esub> TChaosTT"
+    then have "x' @ [[X3]\<^sub>R] \<in> STOP\<^sub>C \<or> (\<exists>x''. x'' @ [[X3]\<^sub>R] \<in> TChaosTT)"
+      unfolding StrictTimedInterruptTT_def apply - apply (induct x' rule:ttWF.induct, auto)
+      apply (metis Nil_is_append_conv append_Nil butlast_append butlast_snoc)
+      apply (metis append_Nil2 append_butlast_last_id last.simps last_appendR)
+      apply (metis append_Nil2 append_butlast_last_id last.simps last_appendR)
+      apply (metis append_Nil2 last.simps last_appendR snoc_eq_iff_butlast)
+      apply (metis append_Nil2 last.simps last_appendR list.distinct(1) snoc_eq_iff_butlast)
+      apply (metis append_Nil2 last.simps last_appendR snoc_eq_iff_butlast)
+      by (metis append_Nil2 last.simps last_appendR list.distinct(1) snoc_eq_iff_butlast)+
+    then  show "False"
+      unfolding StopTT_def TChaosTT_def
+    proof (auto simp add: notin_tocks)
+      show "Tock \<notin> X3 \<Longrightarrow> False"
+        using 3 by blast
+    next
+      fix x''
+      assume "timelock_free_trace (x'' @ [[X3]\<^sub>R])"
+      then have "Tock \<notin> X3"
+        by (induct x'' rule:timelock_free_trace.induct, auto)
+      then show False
+        using 3 by blast
+    qed
+  next
+    fix Xa
+    assume x'3_Xa_in_P_renaming: "x'3 @ [[Xa]\<^sub>R] \<in> RenamingTT P OtherEvent"
+    assume Timelock_notin_Xa: "Event Timelock \<notin> Xa"
+    assume X3_subset_Xa: "X3 \<subseteq> Xa"
+
+    have Timelock_notin_X3: "Event Timelock \<notin> X3"
+      using Timelock_notin_Xa X3_subset_Xa by blast
+    have x'3_tock_notin_TimeSyncInterruptTT: "x'3 @ [[X3]\<^sub>R, [Tock]\<^sub>E] \<notin> (RenamingTT P OtherEvent \<triangle>\<^sub>T Timelock \<rightarrow>\<^sub>C (STOP\<^sub>C \<triangle>\<^bsub>1\<^esub> TChaosTT))"
+      using "3" P_wf ttWF_dist_cons_refusal unprioiritised_remove_timelock_spec_wf by fastforce
+
+    have Timelock_in_prirefTT_X3: 
+      "Event Timelock \<in> prirefTT (f2porder timelock_ordering) x'3 (RenamingTT P OtherEvent \<triangle>\<^sub>T Timelock \<rightarrow>\<^sub>C (STOP\<^sub>C \<triangle>\<^bsub>1\<^esub> TChaosTT)) X3"
+      using "2" "3" by blast
+    have Timelock_notin_prirefTT_X3: 
+      "Event Timelock \<notin> prirefTT (f2porder timelock_ordering) x'3 (RenamingTT P OtherEvent \<triangle>\<^sub>T Timelock \<rightarrow>\<^sub>C (STOP\<^sub>C \<triangle>\<^bsub>1\<^esub> TChaosTT)) X3"
+      using Timelock_notin_X3 x'3_tock_notin_TimeSyncInterruptTT unfolding prirefTT_def apply auto
+      unfolding my_le_def my_lt_def by (auto simp add: timelock_ordering_porder_cancel, case_tac b, auto)
+
+    show False
+      using Timelock_notin_prirefTT_X3 Timelock_in_prirefTT_X3 by blast
+  qed
+qed
+
+lemma remove_timelock_spec_timelock_free_no_effect:
+  assumes P_wf: "\<forall>x\<in>P. ttWF x" and TT1_P: "TT1 P" and TT2_P: "TT2 P"
+  assumes P_timelock_free: "timelock_free P" 
+  shows "remove_timelock_spec P = RenamingTT P OtherEvent"
+proof auto
+  fix x
+  assume x_in_remove_timelock_spec: "x \<in> remove_timelock_spec P"
+
+  have 1:  "\<And>P. \<forall>x\<in>P. ttWF x \<Longrightarrow> TT1 P \<Longrightarrow> TT2 P \<Longrightarrow> timelock_free P \<Longrightarrow> ttWF x \<Longrightarrow>
+    x \<in> remove_timelock_spec P \<Longrightarrow> x \<in> PriTT (f2porder timelock_ordering) (RenamingTT P OtherEvent \<triangle>\<^sub>T Timelock \<rightarrow>\<^sub>C (STOP\<^sub>C \<triangle>\<^bsub>1\<^esub> TChaosTT))"
+    unfolding remove_timelock_spec_def HidingTT_def
+  proof (auto, induct x rule:ttWF.induct, auto)
+    fix p and P :: "'b ttprocess"
+    assume P_wf: "\<forall>x\<in>P. ttWF x" and TT1_P: "TT1 P" and TT2_P: "TT2 P"
+    assume P_timelock_free: "timelock_free P"
+    assume p_in_PriTT: "p \<in> PriTT (f2porder timelock_ordering) (RenamingTT P OtherEvent \<triangle>\<^sub>T Timelock \<rightarrow>\<^sub>C (STOP\<^sub>C \<triangle>\<^bsub>Suc 0\<^esub> TChaosTT))"
+    assume empty_in_p_hiding: "[] \<in> hide_trace {Event Timelock} p"
+    then have "p = [] \<or> (\<exists>p'. p = [Event Timelock]\<^sub>E # p')"
+      by (cases p rule:ttWF.cases, auto)
+    then have "p = []"
+      using P_timelock_free P_wf TT1_P TT2_P unhidden_remove_timelock_spec_timelock_free_no_init_Timelock p_in_PriTT by blast
+    then show "[] \<in> PriTT (f2porder timelock_ordering) (RenamingTT P OtherEvent \<triangle>\<^sub>T Timelock \<rightarrow>\<^sub>C (STOP\<^sub>C \<triangle>\<^bsub>Suc 0\<^esub> TChaosTT))"
+      using p_in_PriTT by blast
+  next
+    fix X p and P :: "'b ttprocess"
+    assume P_wf: "\<forall>x\<in>P. ttWF x" and TT1_P: "TT1 P" and TT2_P: "TT2 P"
+    assume P_timelock_free: "timelock_free P"
+    assume p_in_PriTT: "p \<in> PriTT (f2porder timelock_ordering) (RenamingTT P OtherEvent \<triangle>\<^sub>T Timelock \<rightarrow>\<^sub>C (STOP\<^sub>C \<triangle>\<^bsub>Suc 0\<^esub> TChaosTT))"
+    assume X_in_p_hiding: "[[X]\<^sub>R] \<in> hide_trace {Event Timelock} p"
+    then have "\<exists>Y. p = [[Y]\<^sub>R] \<and> X \<subseteq> Y \<and> Event Timelock \<in> Y"
+      using P_timelock_free P_wf TT1_P TT2_P unhidden_remove_timelock_spec_timelock_free_no_init_Timelock p_in_PriTT by (cases p rule:ttWF.cases, auto)
+    then obtain Y where "p = [[Y]\<^sub>R] \<and> X \<subseteq> Y \<and> Event Timelock \<in> Y"
+      by auto
+    also have Timelock_prefix_wf: "\<forall>x\<in>(Timelock \<rightarrow>\<^sub>C (STOP\<^sub>C \<triangle>\<^bsub>Suc 0\<^esub> TChaosTT)). ttWF x"
+      using Timelock_prefix_deadline_miss_wf by blast
+    have TimeSyncInterruptTT_wf: "\<forall>x\<in>(RenamingTT P OtherEvent \<triangle>\<^sub>T Timelock \<rightarrow>\<^sub>C (STOP\<^sub>C \<triangle>\<^bsub>Suc 0\<^esub> TChaosTT)). ttWF x"
+      by (smt P_wf RenamingTT_wf TimeSyncInterruptTT_wf Timelock_prefix_wf)
+    have TT1_Timelock_prefix: "TT1 (Timelock \<rightarrow>\<^sub>C (STOP\<^sub>C \<triangle>\<^bsub>Suc 0\<^esub> TChaosTT))"
+      using Timelock_prefix_deadline_miss_TT1 by blast
+    then have "TT1 (Timelock \<rightarrow>\<^sub>C (STOP\<^sub>C \<triangle>\<^bsub>Suc 0\<^esub> TChaosTT))"
+      by (smt PrefixTT_wf StopTT_wf StrictTimedInterruptTT_wf mem_Collect_eq)
+    then have "TT1 (RenamingTT P OtherEvent \<triangle>\<^sub>T Timelock \<rightarrow>\<^sub>C (STOP\<^sub>C \<triangle>\<^bsub>Suc 0\<^esub> TChaosTT))"
+      by (metis P_wf RenamingTT_wf TT1_P TT1_Renaming TT1_TimeSyncInterrupt Timelock_prefix_wf)
+    then have "TT1  (PriTT (f2porder timelock_ordering) (RenamingTT P OtherEvent \<triangle>\<^sub>T Timelock \<rightarrow>\<^sub>C (STOP\<^sub>C \<triangle>\<^bsub>Suc 0\<^esub> TChaosTT)))"
+      by (simp add: TT1_PriTT TimeSyncInterruptTT_wf)
+    then show "[[X]\<^sub>R] \<in> PriTT (f2porder timelock_ordering) (RenamingTT P OtherEvent \<triangle>\<^sub>T Timelock \<rightarrow>\<^sub>C (STOP\<^sub>C \<triangle>\<^bsub>Suc 0\<^esub> TChaosTT))"
+      by (metis TT1_def calculation p_in_PriTT tt_prefix_subset.simps(1) tt_prefix_subset.simps(2))
+  next
+    fix p :: "'b timelock_event tttrace" and P :: "'b ttprocess"
+    assume P_wf: "\<forall>x\<in>P. ttWF x" and TT1_P: "TT1 P" and TT2_P: "TT2 P"
+    assume P_timelock_free: "timelock_free P"
+    assume "[[Tick]\<^sub>E] \<in> hide_trace {Event Timelock} p" "p \<in> PriTT (f2porder timelock_ordering) (RenamingTT P OtherEvent \<triangle>\<^sub>T Timelock \<rightarrow>\<^sub>C (STOP\<^sub>C \<triangle>\<^bsub>Suc 0\<^esub> TChaosTT))"
+    then have "p = [[Tick]\<^sub>E]"
+      by (cases p rule:ttWF.cases, auto simp add: P_timelock_free P_wf TT1_P TT2_P unhidden_remove_timelock_spec_timelock_free_no_init_Timelock)
+    then show "p \<in> PriTT (f2porder timelock_ordering) (RenamingTT P OtherEvent \<triangle>\<^sub>T Timelock \<rightarrow>\<^sub>C (STOP\<^sub>C \<triangle>\<^bsub>Suc 0\<^esub> TChaosTT)) \<Longrightarrow>
+        [[Tick]\<^sub>E] \<in> PriTT (f2porder timelock_ordering) (RenamingTT P OtherEvent \<triangle>\<^sub>T Timelock \<rightarrow>\<^sub>C (STOP\<^sub>C \<triangle>\<^bsub>Suc 0\<^esub> TChaosTT))"
+      by blast
+  next
+    fix e and \<sigma> p :: "'b timelock_event tttrace" and P :: "'b ttprocess"
+    assume P_wf: "\<forall>x\<in>P. ttWF x" and TT1_P: "TT1 P" and TT2_P: "TT2 P"
+    assume P_timelock_free: "timelock_free P"
+    assume e_\<sigma>_in_hide_trace_p: "[Event e]\<^sub>E # \<sigma> \<in> hide_trace {Event Timelock} p"
+    assume p_in_PriTT: "p \<in> PriTT (f2porder timelock_ordering) (RenamingTT P OtherEvent \<triangle>\<^sub>T Timelock \<rightarrow>\<^sub>C (STOP\<^sub>C \<triangle>\<^bsub>Suc 0\<^esub> TChaosTT))"
+    assume ind_hyp: "\<And>P p. \<forall>x\<in>P. ttWF x \<Longrightarrow> TT1 P \<Longrightarrow> TT2 P \<Longrightarrow> timelock_free P \<Longrightarrow> \<sigma> \<in> hide_trace {Event Timelock} p \<Longrightarrow>
+      p \<in> PriTT (f2porder timelock_ordering) (RenamingTT P OtherEvent \<triangle>\<^sub>T Timelock \<rightarrow>\<^sub>C (STOP\<^sub>C \<triangle>\<^bsub>Suc 0\<^esub> TChaosTT)) \<Longrightarrow>
+      \<sigma> \<in> PriTT (f2porder timelock_ordering) (RenamingTT P OtherEvent \<triangle>\<^sub>T Timelock \<rightarrow>\<^sub>C (STOP\<^sub>C \<triangle>\<^bsub>Suc 0\<^esub> TChaosTT))"
+
+    obtain p' e' where 1: "p = [Event e]\<^sub>E # p' \<and> \<sigma> \<in> hide_trace {Event Timelock} p' \<and> e = OtherEvent e'"
+      using e_\<sigma>_in_hide_trace_p apply (cases p rule:ttWF.cases, auto)
+      using P_timelock_free P_wf TT1_P TT2_P unhidden_remove_timelock_spec_timelock_free_no_init_Timelock p_in_PriTT by (blast, meson timelock_event.exhaust)
+    have 2: "\<forall>x\<in>{t. [Event e']\<^sub>E # t \<in> P}. ttWF x"
+      using P_wf by auto
+    have 3: "TT1 {t. [Event e']\<^sub>E # t \<in> P}"
+      by (simp add: TT1_P TT1_init_event)
+    have 4: "TT2 {t. [Event e']\<^sub>E # t \<in> P}"
+      by (simp add: TT2_P TT2_init_event)
+    have 5: "timelock_free {t. [Event e']\<^sub>E # t \<in> P}"
+      by (metis (mono_tags, lifting) P_timelock_free mem_Collect_eq timelock_free_def timelock_free_trace.simps(2))
+
+    have 6: "p' \<in> PriTT (f2porder timelock_ordering) (RenamingTT {t. [Event e']\<^sub>E # t \<in> P} OtherEvent \<triangle>\<^sub>T Timelock \<rightarrow>\<^sub>C (STOP\<^sub>C \<triangle>\<^bsub>Suc 0\<^esub> TChaosTT))"
+      using "1" P_wf p_in_PriTT unhidden_remove_timelock_spec_init_event by fastforce
+
+    have "\<sigma> \<in> PriTT (f2porder timelock_ordering) (RenamingTT {t. [Event e']\<^sub>E # t \<in> P} OtherEvent \<triangle>\<^sub>T Timelock \<rightarrow>\<^sub>C (STOP\<^sub>C \<triangle>\<^bsub>Suc 0\<^esub> TChaosTT))"
+      using ind_hyp 1 2 3 4 5 6 by auto
+    then have "\<sigma> \<in> {t. [Event (OtherEvent e')]\<^sub>E # t \<in> PriTT (f2porder timelock_ordering) (RenamingTT P OtherEvent \<triangle>\<^sub>T Timelock \<rightarrow>\<^sub>C (STOP\<^sub>C \<triangle>\<^bsub>Suc 0\<^esub> TChaosTT))}"
+      by (simp add: P_wf unhidden_remove_timelock_spec_init_event)
+    then show "[Event e]\<^sub>E # \<sigma> \<in> PriTT (f2porder timelock_ordering) (RenamingTT P OtherEvent \<triangle>\<^sub>T Timelock \<rightarrow>\<^sub>C (STOP\<^sub>C \<triangle>\<^bsub>Suc 0\<^esub> TChaosTT))"
+      using "1" by blast
+  next
+    fix X and \<sigma> p :: "'b timelock_event tttrace" and P :: "'b ttprocess"
+    assume P_wf: "\<forall>x\<in>P. ttWF x" and TT1_P: "TT1 P" and TT2_P: "TT2 P"
+    assume P_timelock_free: "timelock_free P"
+    assume p_in_PriTT: "p \<in> PriTT (f2porder timelock_ordering) (RenamingTT P OtherEvent \<triangle>\<^sub>T Timelock \<rightarrow>\<^sub>C (STOP\<^sub>C \<triangle>\<^bsub>Suc 0\<^esub> TChaosTT))"
+    assume X_Tock_\<sigma>_in_hide_trace_p: "[X]\<^sub>R # [Tock]\<^sub>E # \<sigma> \<in> hide_trace {Event Timelock} p"
+    assume ttWF_\<sigma>: "ttWF \<sigma>"
+    assume Tock_notin_X: "Tock \<notin> X"
+    assume ind_hyp: "\<And>P p. \<forall>x\<in>P. ttWF x \<Longrightarrow> TT1 P \<Longrightarrow> TT2 P \<Longrightarrow> timelock_free P \<Longrightarrow> \<sigma> \<in> hide_trace {Event Timelock} p \<Longrightarrow>
+        p \<in> PriTT (f2porder timelock_ordering) (RenamingTT P OtherEvent \<triangle>\<^sub>T Timelock \<rightarrow>\<^sub>C (STOP\<^sub>C \<triangle>\<^bsub>Suc 0\<^esub> TChaosTT)) \<Longrightarrow>
+        \<sigma> \<in> PriTT (f2porder timelock_ordering) (RenamingTT P OtherEvent \<triangle>\<^sub>T Timelock \<rightarrow>\<^sub>C (STOP\<^sub>C \<triangle>\<^bsub>Suc 0\<^esub> TChaosTT))"
+
+    obtain p' X' where p_def: "p = [X']\<^sub>R # [Tock]\<^sub>E # p' \<and> X \<subseteq> X'"
+      using X_Tock_\<sigma>_in_hide_trace_p apply (cases p rule:ttWF.cases, auto)
+      using P_timelock_free P_wf TT1_P TT2_P unhidden_remove_timelock_spec_timelock_free_no_init_Timelock p_in_PriTT by blast
+
+    have 1: "\<forall>x\<in>{t. [(lift_renaming_func OtherEvent) -` X']\<^sub>R # [Tock]\<^sub>E # t \<in> P}. ttWF x"
+      using P_wf by fastforce
+    have 2: "TT1 {t. [(lift_renaming_func OtherEvent) -` X']\<^sub>R # [Tock]\<^sub>E # t \<in> P}"
+      by (simp add: TT1_P TT1_init_tock)
+    have 3: "TT2 {t. [(lift_renaming_func OtherEvent) -` X']\<^sub>R # [Tock]\<^sub>E # t \<in> P}"
+      by (simp add: TT2_P TT2_init_tock)
+    have 4: "timelock_free {t. [(lift_renaming_func OtherEvent) -` X']\<^sub>R # [Tock]\<^sub>E # t \<in> P}"
+      by (metis (no_types, lifting) P_timelock_free mem_Collect_eq timelock_free_def timelock_free_trace.simps(2) timelock_free_trace.simps(3))
+
+    have 5: "\<sigma> \<in> hide_trace {Event Timelock} p'"
+      using X_Tock_\<sigma>_in_hide_trace_p p_def by auto
+
+    have 6: "p' \<in> PriTT (f2porder timelock_ordering) (RenamingTT {t. [(lift_renaming_func OtherEvent) -` X']\<^sub>R # [Tock]\<^sub>E # t \<in> P} OtherEvent \<triangle>\<^sub>T Timelock \<rightarrow>\<^sub>C (STOP\<^sub>C \<triangle>\<^bsub>Suc 0\<^esub> TChaosTT))"
+      using P_timelock_free P_wf TT1_P TT2_P p_def p_in_PriTT unhidden_remove_timelock_spec_init_tock by fastforce
+    
+    have "\<sigma> \<in> PriTT (f2porder timelock_ordering) (RenamingTT {t. [(lift_renaming_func OtherEvent) -` X']\<^sub>R # [Tock]\<^sub>E # t \<in> P} OtherEvent \<triangle>\<^sub>T Timelock \<rightarrow>\<^sub>C (STOP\<^sub>C \<triangle>\<^bsub>Suc 0\<^esub> TChaosTT))"
+      using ind_hyp[where P="{t. [(lift_renaming_func OtherEvent) -` X']\<^sub>R # [Tock]\<^sub>E # t \<in> P}", where p=p'] 1 2 3 4 5 6 by auto
+    then have "\<sigma> \<in> {t. [X']\<^sub>R # [Tock]\<^sub>E # t \<in> PriTT (f2porder timelock_ordering) (RenamingTT P OtherEvent \<triangle>\<^sub>T Timelock \<rightarrow>\<^sub>C (STOP\<^sub>C \<triangle>\<^bsub>Suc 0\<^esub> TChaosTT))}"
+      by (simp add: P_timelock_free P_wf TT1_P TT2_P unhidden_remove_timelock_spec_init_tock)
+    also have "TT1 (PriTT (f2porder timelock_ordering) (RenamingTT P OtherEvent \<triangle>\<^sub>T Timelock \<rightarrow>\<^sub>C (STOP\<^sub>C \<triangle>\<^bsub>Suc 0\<^esub> TChaosTT)))"
+      by (meson P_wf TT1_P TT1_PriTT unprioiritised_remove_timelock_spec_TT1 unprioiritised_remove_timelock_spec_wf)
+    then show "[X]\<^sub>R # [Tock]\<^sub>E # \<sigma> \<in> PriTT (f2porder timelock_ordering) (RenamingTT P OtherEvent \<triangle>\<^sub>T Timelock \<rightarrow>\<^sub>C (STOP\<^sub>C \<triangle>\<^bsub>Suc 0\<^esub> TChaosTT))"
+      using calculation p_def tt_prefix_subset_refl unfolding TT1_def apply auto
+      by (erule_tac x="[X]\<^sub>R # [Tock]\<^sub>E # \<sigma>" in allE, auto, erule_tac x="[X']\<^sub>R # [Tock]\<^sub>E # \<sigma>" in allE, auto)
+  qed
+      
+  have 2: "\<And>P. \<forall>x\<in>P. ttWF x \<Longrightarrow> TT1 P \<Longrightarrow> TT2 P \<Longrightarrow> timelock_free P \<Longrightarrow> ttWF x \<Longrightarrow>
+    x \<in> PriTT (f2porder timelock_ordering) (RenamingTT P OtherEvent \<triangle>\<^sub>T Timelock \<rightarrow>\<^sub>C (STOP\<^sub>C \<triangle>\<^bsub>1\<^esub> TChaosTT)) \<Longrightarrow>
+    x \<in> RenamingTT P OtherEvent"
+  proof (induct x rule:ttWF.induct, auto)
+    fix P :: "'b ttprocess"
+    assume "[] \<in> PriTT (f2porder timelock_ordering) (RenamingTT P OtherEvent \<triangle>\<^sub>T Timelock \<rightarrow>\<^sub>C (STOP\<^sub>C \<triangle>\<^bsub>Suc 0\<^esub> TChaosTT))"
+    then show "[] \<in> RenamingTT P OtherEvent"
+      unfolding PriTT_def apply (auto, case_tac s rule:ttWF.cases, auto)
+      unfolding TimeSyncInterruptTT_def by auto
+  next
+    fix P :: "'b ttprocess" and X
+    assume TT1_P: "TT1 P"
+    assume "[[X]\<^sub>R] \<in> PriTT (f2porder timelock_ordering) (RenamingTT P OtherEvent \<triangle>\<^sub>T Timelock \<rightarrow>\<^sub>C (STOP\<^sub>C \<triangle>\<^bsub>Suc 0\<^esub> TChaosTT))"
+    then obtain X' where X'_assms: "X \<subseteq> X' \<union> {Event Timelock} \<and> [[X']\<^sub>R] \<in> RenamingTT P OtherEvent \<triangle>\<^sub>T Timelock \<rightarrow>\<^sub>C (STOP\<^sub>C \<triangle>\<^bsub>Suc 0\<^esub> TChaosTT)"
+      unfolding PriTT_def apply (safe, case_tac s rule:ttWF.cases, auto)
+      by (smt OtherEvent_maximal Tick_maximal Tock_maximal insertCI maximal_notin_prirefTT subset_iff timelock_event.exhaust ttevent.exhaust)
+    then have "[[X']\<^sub>R] \<in> RenamingTT P OtherEvent"
+      unfolding TimeSyncInterruptTT_def
+    proof (safe, simp_all)
+      fix p and Xa Y Z :: "'b timelock_event ttevent set"
+      assume "[[Y]\<^sub>R] \<in> Timelock \<rightarrow>\<^sub>C (STOP\<^sub>C \<triangle>\<^bsub>Suc 0\<^esub> TChaosTT)"
+      then have "Tock \<notin> Y"
+        unfolding PrefixTT_def by (auto simp add:notin_tocks Cons_eq_append_conv)
+      then have "Z \<subseteq> Xa \<union> Y \<Longrightarrow> {e \<in> Xa. e \<noteq> Tock} = {e \<in> Y. e \<noteq> Tock} \<Longrightarrow> Z \<subseteq> Xa"
+        by blast
+      then show "Z \<subseteq> Xa \<union> Y \<Longrightarrow> {e \<in> Xa. e \<noteq> Tock} = {e \<in> Y. e \<noteq> Tock} \<Longrightarrow>
+          [[Xa]\<^sub>R] \<in> RenamingTT P OtherEvent \<Longrightarrow> [[Z]\<^sub>R] \<in> RenamingTT P OtherEvent"
+        by (meson TT1_P TT1_Renaming TT1_def tt_prefix_subset.simps(1) tt_prefix_subset.simps(2))
+    next
+      fix p q2
+      assume "\<forall>p' Y. p \<noteq> p' @ [[Y]\<^sub>R]" "\<forall>q' Y. q2 \<noteq> [Y]\<^sub>R # q'" "[[X']\<^sub>R] = p @ q2"
+      then have "False"
+        by (cases p rule:ttWF.cases, auto)
+      then show "p @ q2 \<in> RenamingTT P OtherEvent"
+        by auto
+    qed
+    also have "TT1 (RenamingTT P OtherEvent)"
+      by (simp add: TT1_P TT1_Renaming)
+    then have "[[{e\<in>X. e \<noteq> Event Timelock}]\<^sub>R] \<in> RenamingTT P OtherEvent"
+      using calculation X'_assms unfolding TT1_def apply auto
+      by (erule_tac x="[[{e\<in>X. e \<noteq> Event Timelock}]\<^sub>R]" in allE, auto, erule_tac x="[[X']\<^sub>R]" in allE, auto)
+    then show "[[X]\<^sub>R] \<in> RenamingTT P OtherEvent"
+    proof (cases "Event Timelock \<in> X", auto)
+      assume "Event Timelock \<notin> X"
+      then have "{e \<in> X. e \<noteq> Event Timelock} = X"
+        by auto
+      then show "[[{e \<in> X. e \<noteq> Event Timelock}]\<^sub>R] \<in> RenamingTT P OtherEvent \<Longrightarrow> [[X]\<^sub>R] \<in> RenamingTT P OtherEvent"
+        by auto
+    next
+      show "Event Timelock \<in> X \<Longrightarrow> [[{e \<in> X. e \<noteq> Event Timelock}]\<^sub>R] \<in> RenamingTT P OtherEvent \<Longrightarrow> [[X]\<^sub>R] \<in> RenamingTT P OtherEvent"
+        unfolding RenamingTT_def apply (auto, case_tac x rule:ttWF.cases, auto)
+        apply (rule_tac x="[[{y. lift_renaming_func OtherEvent y \<in> X \<and> lift_renaming_func OtherEvent y \<noteq> Event Timelock}]\<^sub>R]" in bexI, auto)
+        by (case_tac x, auto)
+    qed
+  next
+    fix P :: "'b ttprocess"
+    assume "[[Tick]\<^sub>E] \<in> PriTT (f2porder timelock_ordering) (RenamingTT P OtherEvent \<triangle>\<^sub>T Timelock \<rightarrow>\<^sub>C (STOP\<^sub>C \<triangle>\<^bsub>Suc 0\<^esub> TChaosTT))"
+    then show "[[Tick]\<^sub>E] \<in> RenamingTT P OtherEvent"
+      unfolding PriTT_def apply auto apply (case_tac s rule:ttWF.cases, auto)
+      unfolding TimeSyncInterruptTT_def
+    proof auto
+      fix p q2 :: "'b timelock_event tttrace"
+      assume assm: "[[Tick]\<^sub>E] = p @ q2"
+      then have "(p = [[Tick]\<^sub>E] \<and> q2 = []) \<or> (p = [] \<and> q2 = [[Tick]\<^sub>E])"
+        by (case_tac p rule:ttWF.cases, simp, simp, blast, simp_all)
+      then show "p \<in> RenamingTT P OtherEvent \<Longrightarrow>
+          filter_tocks p @ q2 \<in> Timelock \<rightarrow>\<^sub>C (STOP\<^sub>C \<triangle>\<^bsub>Suc 0\<^esub> TChaosTT) \<Longrightarrow>
+          p @ q2 \<in> RenamingTT P OtherEvent"
+      unfolding PrefixTT_def apply (auto simp add: notin_tocks)
+      by (metis Nil_is_append_conv append_Nil butlast.simps(2) butlast_append last.simps list.distinct(1) ttevent.distinct(3) ttobs.inject(1))
+    qed
+  next
+    fix P :: "'b ttprocess" and e \<sigma>
+    assume P_wf: "\<forall>x\<in>P. ttWF x" and TT1_P: "TT1 P" and TT2_P: "TT2 P" and P_timelock_free: "timelock_free P"
+    assume e_\<sigma>_in_PriTT: "[Event e]\<^sub>E # \<sigma> \<in> PriTT (f2porder timelock_ordering) (RenamingTT P OtherEvent \<triangle>\<^sub>T Timelock \<rightarrow>\<^sub>C (STOP\<^sub>C \<triangle>\<^bsub>Suc 0\<^esub> TChaosTT))"
+    assume ind_hyp: "\<And>P. \<forall>x\<in>P. ttWF x \<Longrightarrow> TT1 P \<Longrightarrow> TT2 P \<Longrightarrow> timelock_free P \<Longrightarrow>
+             \<sigma> \<in> PriTT (f2porder timelock_ordering) (RenamingTT P OtherEvent \<triangle>\<^sub>T Timelock \<rightarrow>\<^sub>C (STOP\<^sub>C \<triangle>\<^bsub>Suc 0\<^esub> TChaosTT)) \<Longrightarrow>
+             \<sigma> \<in> RenamingTT P OtherEvent"
+
+    obtain e' where e_is_OtherEvent: "e = OtherEvent e'"
+      using e_\<sigma>_in_PriTT apply (cases e, auto)
+      by (simp add: P_timelock_free P_wf TT1_P TT2_P unhidden_remove_timelock_spec_timelock_free_no_init_Timelock)
+    
+    have 1: "\<forall>x\<in>{t. [Event e']\<^sub>E # t \<in> P}. ttWF x"
+      using P_wf by auto
+    have 2: "TT1 {t. [Event e']\<^sub>E # t \<in> P}"
+      by (simp add: TT1_P TT1_init_event)
+    have 3: "TT2 {t. [Event e']\<^sub>E # t \<in> P}"
+      by (simp add: TT2_P TT2_init_event)
+    have 4: "timelock_free {t. [Event e']\<^sub>E # t \<in> P}"
+      by (metis (no_types, lifting) P_timelock_free mem_Collect_eq timelock_free_def timelock_free_trace.simps(2))
+
+    have "\<sigma> \<in> PriTT (f2porder timelock_ordering) (RenamingTT {t. [Event e']\<^sub>E # t \<in> P} OtherEvent \<triangle>\<^sub>T Timelock \<rightarrow>\<^sub>C (STOP\<^sub>C \<triangle>\<^bsub>Suc 0\<^esub> TChaosTT))"
+      using P_wf e_\<sigma>_in_PriTT e_is_OtherEvent unhidden_remove_timelock_spec_init_event by fastforce
+    then have "\<sigma> \<in> RenamingTT {t. [Event e']\<^sub>E # t \<in> P} OtherEvent"
+      using "1" "2" "3" "4" ind_hyp by blast
+    then show "[Event e]\<^sub>E # \<sigma> \<in> RenamingTT P OtherEvent"
+      by (metis (mono_tags, lifting) RenamingTT_init_event e_is_OtherEvent inj_def mem_Collect_eq timelock_event.inject)
+  next
+    fix P :: "'b ttprocess" and X \<sigma>
+    assume P_wf: "\<forall>x\<in>P. ttWF x" and TT1_P: "TT1 P" and TT2_P: "TT2 P" and P_timelock_free: "timelock_free P"
+    assume X_Tock_\<sigma>_in_PriTT: "[X]\<^sub>R # [Tock]\<^sub>E # \<sigma> \<in> PriTT (f2porder timelock_ordering) (RenamingTT P OtherEvent \<triangle>\<^sub>T Timelock \<rightarrow>\<^sub>C (STOP\<^sub>C \<triangle>\<^bsub>Suc 0\<^esub> TChaosTT))"
+    assume ind_hyp: "(\<And>P. \<forall>x\<in>P. ttWF x \<Longrightarrow> TT1 P \<Longrightarrow> TT2 P \<Longrightarrow> timelock_free P \<Longrightarrow>
+             \<sigma> \<in> PriTT (f2porder timelock_ordering) (RenamingTT P OtherEvent \<triangle>\<^sub>T Timelock \<rightarrow>\<^sub>C (STOP\<^sub>C \<triangle>\<^bsub>Suc 0\<^esub> TChaosTT)) \<Longrightarrow>
+             \<sigma> \<in> RenamingTT P OtherEvent)"
+
+    have 1: "\<forall>x\<in>{\<sigma>. [lift_renaming_func OtherEvent -` X]\<^sub>R # [Tock]\<^sub>E # \<sigma> \<in> P}. ttWF x"
+      using P_wf by auto
+    have 2: "TT1 {\<sigma>. [lift_renaming_func OtherEvent -` X]\<^sub>R # [Tock]\<^sub>E # \<sigma> \<in> P}"
+      by (simp add: TT1_P TT1_init_tock)
+    have 3: "TT2 {\<sigma>. [lift_renaming_func OtherEvent -` X]\<^sub>R # [Tock]\<^sub>E # \<sigma> \<in> P}"
+      by (simp add: TT2_P TT2_init_tock)
+    have 4: "timelock_free {\<sigma>. [lift_renaming_func OtherEvent -` X]\<^sub>R # [Tock]\<^sub>E # \<sigma> \<in> P}"
+      by (metis (mono_tags, lifting) P_timelock_free mem_Collect_eq timelock_free_def timelock_free_trace.simps(2) timelock_free_trace.simps(3))
+
+    have 5: "\<sigma> \<in> PriTT (f2porder timelock_ordering) (RenamingTT {\<sigma>. [lift_renaming_func OtherEvent -` X]\<^sub>R # [Tock]\<^sub>E # \<sigma> \<in> P} OtherEvent \<triangle>\<^sub>T Timelock \<rightarrow>\<^sub>C (STOP\<^sub>C \<triangle>\<^bsub>Suc 0\<^esub> TChaosTT))"
+      using P_timelock_free P_wf TT1_P TT2_P X_Tock_\<sigma>_in_PriTT unhidden_remove_timelock_spec_init_tock by auto
+
+    have "\<sigma> \<in> RenamingTT {\<sigma>. [lift_renaming_func OtherEvent -` X]\<^sub>R # [Tock]\<^sub>E # \<sigma> \<in> P} OtherEvent"
+      using "1" "2" "3" "4" "5" ind_hyp by blast
+    then show "[X]\<^sub>R # [Tock]\<^sub>E # \<sigma> \<in> RenamingTT P OtherEvent"
+      using RenamingTT_init_tock by blast
+  qed
+
+  have x_wf: "ttWF x"
+    using P_wf remove_timelock_spec_wf x_in_remove_timelock_spec by blast
+
+  show "x \<in> RenamingTT P OtherEvent"
+    using x_in_remove_timelock_spec 1 2 x_wf assms by auto
+next
+  fix x :: "'a timelock_event tttrace"
+  have "\<And>P. \<forall>x\<in>P. ttWF x \<Longrightarrow> TT1 P \<Longrightarrow> TT2 P \<Longrightarrow> timelock_free P \<Longrightarrow> ttWF x \<Longrightarrow> x \<in> RenamingTT P OtherEvent \<Longrightarrow>
+    x \<in> remove_timelock_spec P"
+  proof (induct x rule:ttWF.induct, simp_all)
+    fix P :: "'b ttprocess"
+    assume P_wf: "\<forall>x\<in>P. ttWF x" and TT1_P: "TT1 P" and TT2_P: "TT2 P" and P_timelock_free: "timelock_free P"
+    assume "[] \<in> RenamingTT P OtherEvent"
+    then have "[] \<in> RenamingTT P OtherEvent \<triangle>\<^sub>T Timelock \<rightarrow>\<^sub>C (STOP\<^sub>C \<triangle>\<^bsub>1\<^esub> TChaosTT)"
+      unfolding TimeSyncInterruptTT_def PrefixTT_def by (auto simp add: tocks.empty_in_tocks)
+    then have "[] \<in> PriTT (f2porder timelock_ordering) (RenamingTT P OtherEvent \<triangle>\<^sub>T Timelock \<rightarrow>\<^sub>C (STOP\<^sub>C \<triangle>\<^bsub>1\<^esub> TChaosTT))"
+      unfolding PriTT_def by (auto, rule_tac x="[]" in exI, auto)
+    then show "[] \<in> remove_timelock_spec P"
+      unfolding remove_timelock_spec_def HidingTT_def by auto
+  next
+    fix P :: "'b ttprocess" and X
+    assume P_wf: "\<forall>x\<in>P. ttWF x" and TT1_P: "TT1 P" and TT2_P: "TT2 P" and P_timelock_free: "timelock_free P"
+    assume "[[X]\<^sub>R] \<in> RenamingTT P OtherEvent"
+    then have "[[{e\<in>X. e \<noteq> Event Timelock}]\<^sub>R] \<in> RenamingTT P OtherEvent"
+      by (metis (mono_tags, lifting) TT1_P TT1_Renaming TT1_def mem_Collect_eq subsetI tt_prefix_subset.simps(1) tt_prefix_subset.simps(2))
+    then have "[[{e\<in>X. e \<noteq> Event Timelock}]\<^sub>R] \<in> RenamingTT P OtherEvent \<triangle>\<^sub>T Timelock \<rightarrow>\<^sub>C (STOP\<^sub>C \<triangle>\<^bsub>1\<^esub> TChaosTT)"
+      unfolding TimeSyncInterruptTT_def PrefixTT_def apply auto
+      apply (rule_tac x="[]" in exI, rule_tac x="{e\<in>X. e \<noteq> Event Timelock}" in exI, auto)
+      by (rule_tac x="{e \<in> X. e \<noteq> Event Timelock \<and> e \<noteq> Tock}" in exI, auto simp add: tocks.empty_in_tocks)
+    then have "[[X \<union> {Event Timelock}]\<^sub>R] \<in> PriTT (f2porder timelock_ordering) (RenamingTT P OtherEvent \<triangle>\<^sub>T Timelock \<rightarrow>\<^sub>C (STOP\<^sub>C \<triangle>\<^bsub>1\<^esub> TChaosTT))"
+      unfolding PriTT_def apply auto apply (rule_tac x="[[{e \<in> X. e \<noteq> Event Timelock}]\<^sub>R]" in exI, auto)
+      apply (subst timelock_ordering_prirefTT, simp_all add: P_wf TT1_P TT2_P unprioiritised_remove_timelock_spec_TT2)
+      using P_timelock_free P_wf unprioiritised_remove_timelock_spec_timelock_free apply blast
+      using P_timelock_free P_wf TT1_P TT2_P timelock_ordering_prirefTT unprioiritised_remove_timelock_spec_TT2
+              unprioiritised_remove_timelock_spec_timelock_free by fastforce
+    then show "[[X]\<^sub>R] \<in> remove_timelock_spec P"
+      unfolding remove_timelock_spec_def HidingTT_def by auto
+  next
+    fix P :: "'b ttprocess"
+    assume P_wf: "\<forall>x\<in>P. ttWF x" and TT1_P: "TT1 P" and TT2_P: "TT2 P" and P_timelock_free: "timelock_free P"
+    assume "[[Tick]\<^sub>E] \<in> RenamingTT P OtherEvent"
+    then have "[[Tick]\<^sub>E] \<in> (RenamingTT P OtherEvent \<triangle>\<^sub>T Timelock \<rightarrow>\<^sub>C (STOP\<^sub>C \<triangle>\<^bsub>1\<^esub> TChaosTT))"
+      unfolding TimeSyncInterruptTT_def PrefixTT_def by (auto simp add: tocks.empty_in_tocks)
+    then have "[[Tick]\<^sub>E] \<in>  PriTT (f2porder timelock_ordering) (RenamingTT P OtherEvent \<triangle>\<^sub>T Timelock \<rightarrow>\<^sub>C (STOP\<^sub>C \<triangle>\<^bsub>1\<^esub> TChaosTT))"
+      unfolding PriTT_def by (auto, rule_tac x="[[Tick]\<^sub>E]" in exI, auto simp add: Tick_maximal)
+    then show "[[Tick]\<^sub>E] \<in> remove_timelock_spec P"
+      unfolding remove_timelock_spec_def HidingTT_def by auto
+  next
+    fix P :: "'b ttprocess" and e \<sigma>
+    assume P_wf: "\<forall>x\<in>P. ttWF x" and TT1_P: "TT1 P" and TT2_P: "TT2 P" and P_timelock_free: "timelock_free P"
+    assume e_\<sigma>_in_renaming_P: "[Event e]\<^sub>E # \<sigma> \<in> RenamingTT P OtherEvent"
+    assume ind_hyp: "\<And>P. \<forall>x\<in>P. ttWF x \<Longrightarrow> TT1 P \<Longrightarrow> TT2 P \<Longrightarrow> timelock_free P \<Longrightarrow> \<sigma> \<in> RenamingTT P OtherEvent \<Longrightarrow> \<sigma> \<in> remove_timelock_spec P"
+
+    obtain e' where e_OtherEvent: "e = OtherEvent e'"
+      using e_\<sigma>_in_renaming_P unfolding RenamingTT_def by (cases e, auto, case_tac x rule:ttWF.cases, auto)
+
+    have 1: "\<forall>x\<in>{t. [Event e']\<^sub>E # t \<in> P}. ttWF x"
+      using P_wf by auto
+    have 2: "TT1 {t. [Event e']\<^sub>E # t \<in> P}"
+      by (simp add: TT1_P TT1_init_event)
+    have 3: "TT2 {t. [Event e']\<^sub>E # t \<in> P}"
+      by (simp add: TT2_P TT2_init_event)
+    have 4: "timelock_free {t. [Event e']\<^sub>E # t \<in> P}"
+      by (metis (mono_tags, lifting) P_timelock_free mem_Collect_eq timelock_free_def timelock_free_trace.simps(2))
+    have 5: "\<sigma> \<in> RenamingTT {t. [Event e']\<^sub>E # t \<in> P} OtherEvent"
+      by (metis (mono_tags, lifting) RenamingTT_init_event e_OtherEvent e_\<sigma>_in_renaming_P inj_def mem_Collect_eq timelock_event.inject)
+
+    have "\<sigma> \<in> remove_timelock_spec {t. [Event e']\<^sub>E # t \<in> P}"
+      using "1" "2" "3" "4" "5" ind_hyp by blast
+    then have "\<sigma> \<in> {t. [Event (OtherEvent e')]\<^sub>E # t \<in> remove_timelock_spec P}"
+      by (simp add: P_timelock_free P_wf TT1_P TT2_P remove_timelock_spec_init_event)
+    then show "[Event e]\<^sub>E # \<sigma> \<in> remove_timelock_spec P"
+      using e_OtherEvent by blast
+  next
+    fix P :: "'b ttprocess" and X \<sigma>
+    assume P_wf: "\<forall>x\<in>P. ttWF x" and TT1_P: "TT1 P" and TT2_P: "TT2 P" and P_timelock_free: "timelock_free P"
+    assume X_Tock_\<sigma>_in_renaming_P: "[X]\<^sub>R # [Tock]\<^sub>E # \<sigma> \<in> RenamingTT P OtherEvent"
+    assume ind_hyp: "\<And>P. \<forall>x\<in>P. ttWF x \<Longrightarrow> TT1 P \<Longrightarrow> TT2 P \<Longrightarrow> timelock_free P \<Longrightarrow> \<sigma> \<in> RenamingTT P OtherEvent \<Longrightarrow> \<sigma> \<in> remove_timelock_spec P"
+
+    have 1: "\<forall>x\<in>{t. [(lift_renaming_func OtherEvent) -` X]\<^sub>R # [Tock]\<^sub>E # t \<in> P}. ttWF x"
+      using P_wf by auto
+    have 2: "TT1 {t. [(lift_renaming_func OtherEvent) -` X]\<^sub>R # [Tock]\<^sub>E # t \<in> P}"
+      by (simp add: TT1_P TT1_init_tock)
+    have 3: "TT2 {t. [(lift_renaming_func OtherEvent) -` X]\<^sub>R # [Tock]\<^sub>E # t \<in> P}"
+      by (simp add: TT2_P TT2_init_tock)
+    have 4: "timelock_free {t. [(lift_renaming_func OtherEvent) -` X]\<^sub>R # [Tock]\<^sub>E # t \<in> P}"
+      by (metis (no_types, lifting) P_timelock_free mem_Collect_eq timelock_free_def timelock_free_trace.simps(2) timelock_free_trace.simps(3))
+    have 5: "\<sigma> \<in> RenamingTT {t. [(lift_renaming_func OtherEvent) -` X]\<^sub>R # [Tock]\<^sub>E # t \<in> P} OtherEvent"
+      using RenamingTT_init_tock X_Tock_\<sigma>_in_renaming_P by blast
+
+    have "\<sigma> \<in> remove_timelock_spec {t. [(lift_renaming_func OtherEvent) -` X]\<^sub>R # [Tock]\<^sub>E # t \<in> P}"
+      using "1" "2" "3" "4" "5" ind_hyp by blast
+    then have "\<sigma> \<in> {t. [X]\<^sub>R # [Tock]\<^sub>E # t \<in> remove_timelock_spec P}"
+      by (simp add: P_timelock_free P_wf TT1_P TT2_P remove_timelock_spec_init_tock)
+    then show "[X]\<^sub>R # [Tock]\<^sub>E # \<sigma> \<in> remove_timelock_spec P"
+      by auto
+  qed
+  then show "x \<in> RenamingTT P OtherEvent \<Longrightarrow> x \<in> remove_timelock_spec P"
+    by (meson P_timelock_free P_wf RenamingTT_wf TT1_P TT2_P)
+qed
+
+section \<open>Constrained tick-tock traces refinement\<close>
+
+definition ConstrainedTracesRefinesTT :: "'a ttprocess \<Rightarrow> 'a ttprocess \<Rightarrow> bool" (infix "\<sqsubseteq>\<^sub>C\<^sub>T\<^sub>T\<^sub>T" 50) where
+  "P \<sqsubseteq>\<^sub>C\<^sub>T\<^sub>T\<^sub>T Q = (remove_timelock_spec P \<sqsubseteq>\<^sub>T\<^sub>T\<^sub>T RenamingTT Q OtherEvent)"
+    
+lemma in_traces_renaming_implies_in_traces_remove_timelock_spec:
+  assumes P_wf: "\<forall>x\<in>P. ttWF x" and TT1_P "TT1 P"
+  shows "x \<in> tracesTT (RenamingTT P OtherEvent) \<Longrightarrow> x \<in> tracesTT (remove_timelock_spec P)"
+  unfolding tracesTT_def
+proof auto
+  fix s :: "'a timelock_event tttrace"
+
+  have empty_implication: "\<And>P. [] \<in> RenamingTT P OtherEvent \<Longrightarrow> [] \<in> remove_timelock_spec P"
+  proof -
+    fix P :: "'b ttprocess"
+    assume "[] \<in> RenamingTT P OtherEvent"
+    then have "[] \<in> RenamingTT P OtherEvent \<triangle>\<^sub>T Timelock \<rightarrow>\<^sub>C (STOP\<^sub>C \<triangle>\<^bsub>1\<^esub> TChaosTT)"
+      unfolding TimeSyncInterruptTT_def PrefixTT_def by (auto simp add: tocks.empty_in_tocks)
+    then have "[] \<in> PriTT (f2porder timelock_ordering) (RenamingTT P OtherEvent \<triangle>\<^sub>T Timelock \<rightarrow>\<^sub>C (STOP\<^sub>C \<triangle>\<^bsub>1\<^esub> TChaosTT))"
+      unfolding PriTT_def by (auto, rule_tac x="[]" in exI, auto)
+    then show "[] \<in> remove_timelock_spec P"
+      unfolding remove_timelock_spec_def HidingTT_def by auto
+  qed
+
+  have "\<And>P x. ttWF s \<Longrightarrow> \<forall>x\<in>P. ttWF x \<Longrightarrow> TT1 P \<Longrightarrow> s \<in> RenamingTT P OtherEvent \<Longrightarrow> x = tttrace_to_event_trace s \<Longrightarrow>
+    \<exists>sa\<in>remove_timelock_spec P. tttrace_to_event_trace s = tttrace_to_event_trace sa"
+  proof (induct s rule:ttWF.induct, auto)
+    fix P :: "'b ttprocess"
+    show "[] \<in> RenamingTT P OtherEvent \<Longrightarrow> \<exists>sa\<in>remove_timelock_spec P. [] = tttrace_to_event_trace sa"
+      using empty_implication by (rule_tac x="[]" in bexI, auto)
+  next
+    fix P :: "'b ttprocess" and X
+    assume TT1_P: "TT1 P"
+    assume "[[X]\<^sub>R] \<in> RenamingTT P OtherEvent"
+    then have "[] \<in> RenamingTT P OtherEvent"
+      using TT1_P TT1_Renaming TT1_def tt_prefix_subset.simps(1) by blast
+    then show "\<exists>sa\<in>remove_timelock_spec P. [] = tttrace_to_event_trace sa"
+      by (rule_tac x="[]" in bexI, auto simp add: empty_implication)
+  next
+    fix P :: "'b ttprocess"
+    assume "[[Tick]\<^sub>E] \<in> RenamingTT P OtherEvent"
+    then have "[[Tick]\<^sub>E] \<in> RenamingTT P OtherEvent \<triangle>\<^sub>T Timelock \<rightarrow>\<^sub>C (STOP\<^sub>C \<triangle>\<^bsub>1\<^esub> TChaosTT)"
+      unfolding TimeSyncInterruptTT_def PrefixTT_def by (auto simp add: tocks.empty_in_tocks)
+    then have "[[Tick]\<^sub>E] \<in> PriTT (f2porder timelock_ordering) (RenamingTT P OtherEvent \<triangle>\<^sub>T Timelock \<rightarrow>\<^sub>C (STOP\<^sub>C \<triangle>\<^bsub>1\<^esub> TChaosTT))"
+      unfolding PriTT_def by (auto, rule_tac x="[[Tick]\<^sub>E]" in exI, auto simp add: Tick_maximal)
+    then have "[[Tick]\<^sub>E] \<in> remove_timelock_spec P"
+      unfolding remove_timelock_spec_def HidingTT_def by auto
+    then show "\<exists>sa\<in>remove_timelock_spec P. [Tick] = tttrace_to_event_trace sa"
+      by (rule_tac x="[[Tick]\<^sub>E]" in bexI, auto)
+  next
+    fix P :: "'b ttprocess" and e \<sigma>
+    assume P_wf: "\<forall>x\<in>P. ttWF x" and TT1_P: "TT1 P"
+    assume e_\<sigma>_in_P_renaming: "[Event e]\<^sub>E # \<sigma> \<in> RenamingTT P OtherEvent"
+    assume ind_hyp: "\<And>P x. \<forall>x\<in>P. ttWF x \<Longrightarrow> TT1 P \<Longrightarrow> \<sigma> \<in> RenamingTT P OtherEvent \<Longrightarrow> x = tttrace_to_event_trace \<sigma> \<Longrightarrow>
+      \<exists>sa\<in>remove_timelock_spec P. tttrace_to_event_trace \<sigma> = tttrace_to_event_trace sa"
+
+    obtain e' where e_OtherEvent: "e = OtherEvent e'"
+      using e_\<sigma>_in_P_renaming unfolding RenamingTT_def by (auto, case_tac x rule:ttWF.cases, auto)
+
+    have 1: "\<forall>x\<in>{t. [Event e']\<^sub>E # t \<in> P}. ttWF x"
+      using P_wf by auto
+    have 2: "TT1 {t. [Event e']\<^sub>E # t \<in> P}"
+      by (simp add: TT1_P TT1_init_event)
+    have 3: "\<sigma> \<in> RenamingTT {t. [Event e']\<^sub>E # t \<in> P} OtherEvent"
+      by (metis (mono_tags, lifting) RenamingTT_init_event e_OtherEvent e_\<sigma>_in_P_renaming inj_def mem_Collect_eq timelock_event.inject)
+
+    have "\<exists>sa\<in>remove_timelock_spec {t. [Event e']\<^sub>E # t \<in> P}. tttrace_to_event_trace \<sigma> = tttrace_to_event_trace sa"
+      using 1 2 3 ind_hyp by blast
+    then obtain sa where "sa\<in>remove_timelock_spec {t. [Event e']\<^sub>E # t \<in> P} \<and> tttrace_to_event_trace \<sigma> = tttrace_to_event_trace sa"
+      by blast
+    then have "sa \<in> {t. [Event e]\<^sub>E # t \<in> remove_timelock_spec P} \<and> tttrace_to_event_trace \<sigma> = tttrace_to_event_trace sa"
+      using P_wf e_OtherEvent remove_timelock_spec_init_event by fastforce
+    then show "\<exists>sa\<in>remove_timelock_spec P. Event e # tttrace_to_event_trace \<sigma> = tttrace_to_event_trace sa"
+      by force
+  next
+    fix P :: "'b ttprocess" and X \<sigma>
+    assume P_wf: "\<forall>x\<in>P. ttWF x" and TT1_P: "TT1 P"
+    assume X_Tock_\<sigma>_in_P_renaming: "[X]\<^sub>R # [Tock]\<^sub>E # \<sigma> \<in> RenamingTT P OtherEvent"
+    assume ind_hyp: "\<And>P x. \<forall>x\<in>P. ttWF x \<Longrightarrow> TT1 P \<Longrightarrow> \<sigma> \<in> RenamingTT P OtherEvent \<Longrightarrow>
+               x = tttrace_to_event_trace \<sigma> \<Longrightarrow> \<exists>sa\<in>remove_timelock_spec P. tttrace_to_event_trace \<sigma> = tttrace_to_event_trace sa"
+
+    have 1: "\<forall>x\<in>{t. [lift_renaming_func OtherEvent -` X]\<^sub>R # [Tock]\<^sub>E # t \<in> P}. ttWF x"
+      using P_wf by auto
+    have 2: "TT1 {t. [lift_renaming_func OtherEvent -` X]\<^sub>R # [Tock]\<^sub>E # t \<in> P}"
+      by (simp add: TT1_P TT1_init_tock)
+    have 3: "\<sigma> \<in> RenamingTT {t. [lift_renaming_func OtherEvent -` X]\<^sub>R # [Tock]\<^sub>E # t \<in> P} OtherEvent"
+      using RenamingTT_init_tock X_Tock_\<sigma>_in_P_renaming by blast
+    
+    have "\<exists>sa\<in>remove_timelock_spec {t. [lift_renaming_func OtherEvent -` X]\<^sub>R # [Tock]\<^sub>E # t \<in> P}. tttrace_to_event_trace \<sigma> = tttrace_to_event_trace sa"
+      using 1 2 3 ind_hyp by blast
+    then obtain sa where "sa \<in> remove_timelock_spec {t. [lift_renaming_func OtherEvent -` X]\<^sub>R # [Tock]\<^sub>E # t \<in> P} \<and> tttrace_to_event_trace \<sigma> = tttrace_to_event_trace sa"
+      by auto
+    then have "sa \<in> {t. \<exists>X. [X]\<^sub>R # [Tock]\<^sub>E # t \<in> remove_timelock_spec P} \<and> tttrace_to_event_trace \<sigma> = tttrace_to_event_trace sa"
+      using P_wf TT1_P remove_timelock_spec_init_tock_any_refusal_subset by blast
+    then show "\<exists>sa\<in>remove_timelock_spec P. Tock # tttrace_to_event_trace \<sigma> = tttrace_to_event_trace sa"
+      by (auto, rule_tac x="[X]\<^sub>R # [Tock]\<^sub>E # sa" in bexI, auto)
+  qed
+  then show "s \<in> RenamingTT P OtherEvent \<Longrightarrow> x = tttrace_to_event_trace s \<Longrightarrow>
+    \<exists>sa\<in>remove_timelock_spec P. tttrace_to_event_trace s = tttrace_to_event_trace sa"
+    using P_wf RenamingTT_wf assms(3) by blast
+qed
+
+lemma same_event_trace_implies_same_renamed_event_trace:
+  "\<And>y. tttrace_to_event_trace x = tttrace_to_event_trace y \<Longrightarrow> 
+    \<forall>x'\<in>rename_trace f x. \<forall>y'\<in>rename_trace f y.
+      tttrace_to_event_trace x' = tttrace_to_event_trace y'"
+proof (induct x rule:tttrace_to_event_trace.induct, simp_all)
+  fix y :: "'a tttrace"
+  show "[] = tttrace_to_event_trace y \<Longrightarrow> \<forall>y'\<in>rename_trace f y. [] = tttrace_to_event_trace y'"
+    by (induct y rule:tttrace_to_event_trace.induct, auto)
+next
+  fix X and t y :: "'a tttrace"
+  assume ind_hyp: "\<And>ya. tttrace_to_event_trace y = tttrace_to_event_trace ya \<Longrightarrow>
+    \<forall>x'\<in>rename_trace f t. \<forall>y'\<in>rename_trace f ya. tttrace_to_event_trace x' = tttrace_to_event_trace y'"
+  assume "tttrace_to_event_trace (t) = tttrace_to_event_trace y"
+  then have "\<forall>x'\<in>rename_trace f t. \<forall>y'\<in>rename_trace f y. tttrace_to_event_trace x' = tttrace_to_event_trace y'"
+    using ind_hyp by blast
+  then show "\<forall>x'. (\<exists>s' Y. x' = [Y]\<^sub>R # s' \<and> X = lift_renaming_func f -` Y \<and> s' \<in> rename_trace f t) \<longrightarrow>
+            (\<forall>y'\<in>rename_trace f y. tttrace_to_event_trace x' = tttrace_to_event_trace y')"
+    by auto
+next
+  fix e and t y :: "'a tttrace"
+  assume ind_hyp: "\<And>y. tttrace_to_event_trace t = tttrace_to_event_trace y \<Longrightarrow>
+             \<forall>x'\<in>rename_trace f t. \<forall>y'\<in>rename_trace f y. tttrace_to_event_trace x' = tttrace_to_event_trace y'"
+  assume "e # tttrace_to_event_trace t = tttrace_to_event_trace y"
+  then show "\<forall>x'. (\<exists>s'. x' = [lift_renaming_func f e]\<^sub>E # s' \<and> s' \<in> rename_trace f t) \<longrightarrow>
+            (\<forall>y'\<in>rename_trace f y. tttrace_to_event_trace x' = tttrace_to_event_trace y')"
+    using ind_hyp apply - apply (induct y rule:tttrace_to_event_trace.induct, simp_all)
+    by (metis tttrace_to_event_trace.simps(2), auto)
+qed
+
+lemma tracesTT_refinement_implies_constrained_tracesTT_refinement:
+  assumes P_wf: "\<forall>x\<in>P. ttWF x" and TT1_P: "TT1 P" and Q_wf: "\<forall>x\<in>Q. ttWF x"
+  shows "P \<sqsubseteq>\<^sub>T\<^sub>T\<^sub>T Q \<Longrightarrow> P \<sqsubseteq>\<^sub>C\<^sub>T\<^sub>T\<^sub>T Q"
+  unfolding TracesRefinementTT_def ConstrainedTracesRefinesTT_def
+proof auto
+  fix x :: "'a timelock_event ttevent list"
+  assume traces_Q_subset_traces_P: "tracesTT Q \<subseteq> tracesTT P"
+  assume x_in_traces_renaming_Q: "x \<in> tracesTT (RenamingTT Q OtherEvent)"
+  then obtain y z where "x = tttrace_to_event_trace y \<and> y \<in> rename_trace OtherEvent z \<and> z \<in> Q"
+    unfolding tracesTT_def RenamingTT_def by auto
+  then have "x = tttrace_to_event_trace y \<and> y \<in> rename_trace OtherEvent z \<and> tttrace_to_event_trace z \<in> tracesTT Q"
+    unfolding tracesTT_def using Q_wf by auto
+  then have "x = tttrace_to_event_trace y \<and> y \<in> rename_trace OtherEvent z \<and> tttrace_to_event_trace z \<in> tracesTT P"
+    using traces_Q_subset_traces_P by auto
+  then obtain w where "x = tttrace_to_event_trace y \<and> y \<in> rename_trace OtherEvent z
+      \<and> tttrace_to_event_trace z = tttrace_to_event_trace w \<and> w \<in> P"
+    unfolding tracesTT_def by auto
+  then obtain y' where "x = tttrace_to_event_trace y \<and> y \<in> rename_trace OtherEvent z
+      \<and> tttrace_to_event_trace z = tttrace_to_event_trace w \<and> w \<in> P \<and> y' \<in> rename_trace OtherEvent w"
+    using rename_trace_nonempty[where f=OtherEvent] unfolding inj_def by auto
+  then have "x = tttrace_to_event_trace y' \<and> y' \<in> rename_trace OtherEvent w \<and> w \<in> P"
+    using same_event_trace_implies_same_renamed_event_trace by blast
+  then have "x \<in> tracesTT (RenamingTT P OtherEvent)"
+    unfolding tracesTT_def RenamingTT_def by auto
+  then show "x \<in> tracesTT (remove_timelock_spec P)"
+    using P_wf TT1_P in_traces_renaming_implies_in_traces_remove_timelock_spec by blast
+qed
+
+section \<open>Constrained tick-tock refinement\<close>
+
+definition ConstrainedRefinesTT :: "'a ttprocess \<Rightarrow> 'a ttprocess \<Rightarrow> bool" (infix "\<sqsubseteq>\<^sub>C\<^sub>T\<^sub>T" 50) where
+  "P \<sqsubseteq>\<^sub>C\<^sub>T\<^sub>T Q = (P \<sqsubseteq>\<^sub>C\<^sub>T\<^sub>T\<^sub>T Q \<and> P conf\<^sub>C Q)"
+
+lemma tracesTT_refinement_implies_constrained_tt_refinement:
+  assumes P_wf: "\<forall>x\<in>P. ttWF x" and TT1_P: "TT1 P" and Q_wf: "\<forall>x\<in>Q. ttWF x"
+  shows "P \<sqsubseteq>\<^sub>C Q \<Longrightarrow> P \<sqsubseteq>\<^sub>C\<^sub>T\<^sub>T Q"
+  unfolding ConstrainedRefinesTT_def refines_eq_traces_refines_and_conf
+  using assms tracesTT_refinement_implies_constrained_tracesTT_refinement by auto
+
+section \<open>Equivalent definition using a specialised function\<close>
+
+fun add_deadline_miss_trace :: "'e tttrace \<Rightarrow> 'e tttrace set" where
+  "add_deadline_miss_trace [] = {[]}" |
+  "add_deadline_miss_trace ([e]\<^sub>E # \<rho>) = {[e]\<^sub>E # \<sigma> |\<sigma>. \<sigma> \<in> add_deadline_miss_trace \<rho>}" |
+  "add_deadline_miss_trace ([X]\<^sub>R # \<rho>) = 
+    {[X]\<^sub>R # \<sigma> |\<sigma>. Tock \<notin> X \<and> \<sigma> \<in> add_deadline_miss_trace \<rho>} \<union>
+    {t. Tock \<in> X \<and> (\<exists> X'. X' \<subseteq> {e. e \<in> X \<and> e = Tock} \<and>
+      (t = [[X']\<^sub>R] \<or> t = [[X']\<^sub>R, [Tock]\<^sub>E] \<or> (\<exists> \<sigma>. ttWF \<sigma> \<and> t = [[X']\<^sub>R, [Tock]\<^sub>E] @ \<sigma>)))}"
+
+definition add_deadline_miss :: "'e ttprocess \<Rightarrow> 'e ttprocess" where
+  "add_deadline_miss P = \<Union>{add_deadline_miss_trace t |t. t \<in> P }"
+
+lemma
+  assumes "\<forall>x\<in>P. ttWF x"
+  shows "\<forall>x\<in>(add_deadline_miss P). ttWF x"
+  using assms unfolding add_deadline_miss_def
+proof auto
